@prefix rdf: <http://www.w3.org/1999/02/22-rdf-syntax-ns#> .
@prefix dc: <http://purl.org/dc/elements/1.1/> .
@prefix reg: <http://metadataregistry.org/uri/profile/regap/> .
@prefix skos: <http://www.w3.org/2004/02/skos/core#> .

<http://iflastandards.info/ns/fr/frbr/frbrer/frbrerusertask>
    dc:title "FRBRer User Tasks" ;
    a skos:ConceptScheme ;
    skos:hasTopConcept <http://iflastandards.info/ns/fr/frbr/frbrer/frbrerusertask#T1001>, <http://iflastandards.info/ns/fr/frbr/frbrer/frbrerusertask#T1002>, <http://iflastandards.info/ns/fr/frbr/frbrer/frbrerusertask#T1003>, <http://iflastandards.info/ns/fr/frbr/frbrer/frbrerusertask#T1004> .

<http://iflastandards.info/ns/fr/frbr/frbrer/frbrerusertask#T1001>
    reg:identifier <http://metadataregistry.org/concepts/1232> ;
    reg:status <http://metadataregistry.org/uri/RegStatus/1001> ;
    a skos:Concept ;
    skos:definition "To locate either a single entity or a set of entities in a file or database as the result of a search using an attribute or relationship of the entity."@en ;
    skos:inScheme <http://iflastandards.info/ns/fr/frbr/frbrer/frbrerusertask> ;
    skos:prefLabel "find"@en ;
    skos:scopeNote "Includes only entities of interest to users of bibliographic records."@en ;
    skos:topConceptOf <http://iflastandards.info/ns/fr/frbr/frbrer/frbrerusertask> .

<http://iflastandards.info/ns/fr/frbr/frbrer/frbrerusertask#T1002>
    reg:identifier <http://metadataregistry.org/concepts/1233> ;
    reg:status <http://metadataregistry.org/uri/RegStatus/1001> ;
    a skos:Concept ;
    skos:definition "To confirm that the entity described corresponds to the entity sought, or to distinguish between two or more entities with similar characteristics."@en ;
    skos:inScheme <http://iflastandards.info/ns/fr/frbr/frbrer/frbrerusertask> ;
    skos:prefLabel "identify"@en ;
    skos:scopeNote "Includes only entities of interest to users of bibliographic records."@en ;
    skos:topConceptOf <http://iflastandards.info/ns/fr/frbr/frbrer/frbrerusertask> .

<http://iflastandards.info/ns/fr/frbr/frbrer/frbrerusertask#T1003>
    reg:identifier <http://metadataregistry.org/concepts/1234> ;
    reg:status <http://metadataregistry.org/uri/RegStatus/1001> ;
    a skos:Concept ;
    skos:definition "To choose an entity that meets the user’s requirements with respect to content, physical format, etc., or to reject an entity as being inappropriate to the user’s needs"@en ;
    skos:inScheme <http://iflastandards.info/ns/fr/frbr/frbrer/frbrerusertask> ;
    skos:prefLabel "select"@en ;
    skos:scopeNote "Includes only entities of interest to users of bibliographic records."@en ;
    skos:topConceptOf <http://iflastandards.info/ns/fr/frbr/frbrer/frbrerusertask> .

<http://iflastandards.info/ns/fr/frbr/frbrer/frbrerusertask#T1004>
    reg:identifier <http://metadataregistry.org/concepts/1235> ;
    reg:status <http://metadataregistry.org/uri/RegStatus/1001> ;
    a skos:Concept ;
    skos:definition "To acquire an entity through purchase, loan, etc., or to access an entity electronically through an online connection to a remote computer."@en ;
    skos:inScheme <http://iflastandards.info/ns/fr/frbr/frbrer/frbrerusertask> ;
    skos:prefLabel "obtain"@en ;
    skos:scopeNote "Includes only entities of interest to users of bibliographic records."@en ;
    skos:topConceptOf <http://iflastandards.info/ns/fr/frbr/frbrer/frbrerusertask> .

<http://metadataregistry.org/uri/RegStatus/1001>
    a skos:Concept ;
    skos:prefLabel "Published"@en .

