@prefix dc: <http://purl.org/dc/elements/1.1/> .
@prefix foaf: <http://xmlns.com/foaf/0.1/> .
@prefix owl: <http://www.w3.org/2002/07/owl#> .
@prefix rdf: <http://www.w3.org/1999/02/22-rdf-syntax-ns#> .
@prefix rdfs: <http://www.w3.org/2000/01/rdf-schema#> .
@prefix reg: <http://metadataregistry.org/uri/profile/regap/> .
@prefix skos: <http://www.w3.org/2004/02/skos/core#> .
@prefix xml: <http://www.w3.org/XML/1998/namespace> .
@prefix xsd: <http://www.w3.org/2001/XMLSchema#> .

<http://iflastandards.info/ns/fr/frbr/frbroo/CLP57> a rdf:Property ;
    rdfs:label "should have number of parts"@en ;
    reg:name "shouldHaveNumberOfParts"@en ;
    reg:status <http://metadataregistry.org/uri/RegStatus/1001> ;
    rdfs:comment "This property associates a publication, i.e. an instance of F3 Manifestation Product Type, with an instance of E60 Number, which denotes the number of physical units all exemplars of that publication should consist of, as long as they are recognised as complete exemplars of that publication. Typically, this property is observed on one exemplar of a publication, and extrapolated to all other exemplars of the same publication. This logical inference is an induction along the path that can be modelled as: F3 Manifestation Product Type R7B has example F5 Item P57 has number of parts E60 Number. It can happen that a given exemplar, or subset of exemplars, originally produced, or intended to be produced, with that characteristic, accidentally lacks it. This fact should be recorded as a property of F5 Item, and not of F3 Manifestation Product Type."@en ;
    rdfs:domain <http://iflastandards.info/ns/fr/frbr/frbroo/F3> ;
    rdfs:isDefinedBy <http://iflastandards.info/ns/fr/frbr/frbroo/> ;
    rdfs:range <http://www.cidoc-crm.org/cidoc-crm/E60_Number> ;
    = <http://iflastandards.info/ns/fr/frbr/frbroo/CLP57_should_have_number_of_parts> ;
    skos:definition "This property associates a publication, i.e. an instance of F3 Manifestation Product Type, with an instance of E60 Number, which denotes the number of physical units all exemplars of that publication should consist of, as long as they are recognised as complete exemplars of that publication."@en ;
    skos:scopeNote "Typically, this property is observed on one exemplar of a publication, and extrapolated to all other exemplars of the same publication. This logical inference is an induction along the path that can be modelled as: F3 Manifestation Product Type R7B has example F5 Item P57 has number of parts E60 Number. It can happen that a given exemplar, or subset of exemplars, originally produced, or intended to be produced, with that characteristic, accidentally lacks it. This fact should be recorded as a property of F5 Item, and not of F3 Manifestation Product Type."@en .

<http://iflastandards.info/ns/fr/frbr/frbroo/F10> a owl:Class ;
    rdfs:label "Person"@en ;
    reg:name "Person"@en ;
    reg:status <http://metadataregistry.org/uri/RegStatus/1001> ;
    rdfs:comment "This class comprises real persons who live or are assumed to have lived. Bibliographic identities or personae assumed by an individual or a group should be modelled as F12 Nomen and connected to the relevant person or group with an instance of F35 Nomen Use Statement, even if nothing more can be said about this person or group. In a bibliographic context, a name presented following the conventions usually employed for personal names will be assumed to correspond to an actual real person (F10 Person), unless evidence is available to indicate that this is not the case. The fact that a persona may erroneously be classified as an instance of F10 Person does not imply that the concept comprises personae."@en ;
    rdfs:isDefinedBy <http://iflastandards.info/ns/fr/frbr/frbroo/> ;
    rdfs:subClassOf <http://www.cidoc-crm.org/cidoc-crm/E21_Person> ;
    = <http://iflastandards.info/ns/fr/frbr/frbroo/F10_Person> ;
    skos:definition "This class comprises real persons who live or are assumed to have lived."@en ;
    skos:scopeNote "Bibliographic identities or personae assumed by an individual or a group should be modelled as F12 Nomen and connected to the relevant person or group with an instance of F35 Nomen Use Statement, even if nothing more can be said about this person or group. In a bibliographic context, a name presented following the conventions usually employed for personal names will be assumed to correspond to an actual real person (F10 Person), unless evidence is available to indicate that this is not the case. The fact that a persona may erroneously be classified as an instance of F10 Person does not imply that the concept comprises personae."@en .

<http://iflastandards.info/ns/fr/frbr/frbroo/F11> a owl:Class ;
    rdfs:label "Corporate Body"@en ;
    reg:name "CorporateBody"@en ;
    reg:status <http://metadataregistry.org/uri/RegStatus/1001> ;
    rdfs:comment "This class comprises organisations and groups of two or more people and/or organisations acting as a unit. To be considered an F11 Corporate Body a gathering of people needs to bear a name and exhibit organisational characteristics sufficient to allow the body as a whole to participate in the creation, modification or production of an E73 Information Object. Groups such as conferences, congresses, expeditions, exhibitions, festivals, fairs, etc. are modelled as F11 Corporate Bodies when they are named and can take collective action, such as approving a report or publishing their proceedings."@en ;
    rdfs:isDefinedBy <http://iflastandards.info/ns/fr/frbr/frbroo/> ;
    rdfs:subClassOf <http://www.cidoc-crm.org/cidoc-crm/E74_Group> ;
    = <http://iflastandards.info/ns/fr/frbr/frbroo/F11_Corporate_Body> ;
    skos:definition "This class comprises organisations and groups of two or more people and/or organisations acting as a unit. To be considered an F11 Corporate Body a gathering of people needs to bear a name and exhibit organisational characteristics sufficient to allow the body as a whole to participate in the creation, modification or production of an E73 Information Object. Groups such as conferences, congresses, expeditions, exhibitions, festivals, fairs, etc. are modelled as F11 Corporate Bodies when they are named and can take collective action, such as approving a report or publishing their proceedings."@en .

<http://iflastandards.info/ns/fr/frbr/frbroo/F17> a owl:Class ;
    rdfs:label "Aggregation Work"@en ;
    reg:name "AggregationWork"@en,
        "http://iflastandards.info/ns/fr/frbr/frbroo/F16"@en ;
    reg:status <http://metadataregistry.org/uri/RegStatus/1001> ;
    rdfs:comment "This class comprises works whose essence is the selection and/or arrangement of expressions of one or more other works. This does not make the contents of the aggregated expressions part of this work, but only part of the resulting expression. F17 Aggregation Work may include additional original parts. An expression of a work may include expressions of other works within it. For instance, an anthology of poems is regarded as a work in its own right that makes use of expressions of the individual poems that have been selected and ordered as part of an intellectual process. A new version of an aggregate work does not make the resulting complex work an aggregate work as well. The inclusion of expressions from a complex work in an aggregation work does not make the aggregation work itself complex."@en ;
    rdfs:isDefinedBy <http://iflastandards.info/ns/fr/frbr/frbroo/> ;
    rdfs:subClassOf <http://iflastandards.info/ns/fr/frbr/frbroo/F14> ;
    = <http://iflastandards.info/ns/fr/frbr/frbroo/F17_Aggregation_Work> .

<http://iflastandards.info/ns/fr/frbr/frbroo/F39> a owl:Class ;
    rdfs:label "Family"@en ;
    reg:name "Family"@en ;
    reg:status <http://metadataregistry.org/uri/RegStatus/1001> ;
    rdfs:comment "This class comprises groups of two or more persons presented as a family justified by relationships of birth, marriage, adoption, civil union, or similar social or legal status and an assumed common tradition, including examples such as royal families, dynasties, houses of nobility, etc."@en ;
    rdfs:isDefinedBy <http://iflastandards.info/ns/fr/frbr/frbroo/> ;
    rdfs:subClassOf <http://www.cidoc-crm.org/cidoc-crm/E74_Group> ;
    = <http://iflastandards.info/ns/fr/frbr/frbroo/F39_Family> ;
    skos:definition "This class comprises groups of two or more persons presented as a family justified by relationships of birth, marriage, adoption, civil union, or similar social or legal status and an assumed common tradition, including examples such as royal families, dynasties, houses of nobility, etc."@en .

<http://iflastandards.info/ns/fr/frbr/frbroo/F50> a owl:Class ;
    rdfs:label "Controlled Access Point"@en ;
    reg:name "ControlledAccessPoint"@en ;
    reg:status <http://metadataregistry.org/uri/RegStatus/1001> ;
    rdfs:comment "This class comprises identifiers that are not only designed to be unique for the thing they identify, but also to ensure, by following adequate rules based on widely known and accepted properties for their generation, that an independent agency using the same rule would create the same identifier for the same thing. F50 Controlled Access Point covers the notion of both \"preferred\" and \"variant\" forms. It does not cover the notion of \"cross references\". A cross reference may not uniquely identify one entity, but can be shared by two or more entities, regardless of whether it displays the same structural characteristics as preferred controlled access points."@en ;
    rdfs:isDefinedBy <http://iflastandards.info/ns/fr/frbr/frbroo/> ;
    rdfs:subClassOf <http://iflastandards.info/ns/fr/frbr/frbroo/F13> ;
    = <http://iflastandards.info/ns/fr/frbr/frbroo/F50_Controlled_Access_Point> ;
    skos:definition "This class comprises identifiers that are not only designed to be unique for the thing they identify, but also to ensure, by following adequate rules based on widely known and accepted properties for their generation, that an independent agency using the same rule would create the same identifier for the same thing."@en ;
    skos:scopeNote "F50 Controlled Access Point covers the notion of both \"preferred\" and \"variant\" forms. It does not cover the notion of \"cross references\". A cross reference may not uniquely identify one entity, but can be shared by two or more entities, regardless of whether it displays the same structural characteristics as preferred controlled access points."@en .

<http://iflastandards.info/ns/fr/frbr/frbroo/F6> a owl:Class ;
    rdfs:label "Concept"@en ;
    reg:name "Concept"@en ;
    reg:status <http://metadataregistry.org/uri/RegStatus/1001> ;
    rdfs:comment "An abstract notion or idea. [FRBRER] Includes fields of knowledge, disciplines, schools of thought, etc. Includes philosophies, religions, political ideologies, etc. Includes theories, processes, techniques, practices, etc. [Definition from the FRAD draft model, unchanged] This class comprises non-material products of our minds and other human produced data that have become objects of a discourse about their identity, circumstances of creation or historical implication. The production of such information may have been supported by the use of technical devices such as cameras or computers. Characteristically, instances of this class are created, invented or thought by someone, and then may be documented or communicated between persons. Instances of E28 Conceptual Object have the ability to exist on more than one particular carrier at the same time, such as paper, electronic signals, marks, audio media, paintings, photos, human memories, etc. They cannot be destroyed. They exist as long as they can be found on at least one carrier or in at least one human memory. Their existence ends when the last carrier and the last memory are lost. [Scope note for E28 Conceptual Object in CIDOC CRM version 5.0.1]"@en ;
    rdfs:isDefinedBy <http://iflastandards.info/ns/fr/frbr/frbroo/> ;
    rdfs:subClassOf <http://www.cidoc-crm.org/cidoc-crm/E28_Conceptual_Object> ;
    = <http://iflastandards.info/ns/fr/frbr/frbroo/F6_Concept> ;
    skos:definition "An abstract notion or idea."@en ;
    skos:scopeNote "Includes fields of knowledge, disciplines, schools of thought, etc. Includes philosophies, religions, political ideologies, etc. Includes theories, processes, techniques, practices, etc. [Definition from the FRAD draft model, unchanged] This class comprises non-material products of our minds and other human produced data that have become objects of a discourse about their identity, circumstances of creation or historical implication. The production of such information may have been supported by the use of technical devices such as cameras or computers. Characteristically, instances of this class are created, invented or thought by someone, and then may be documented or communicated between persons. Instances of E28 Conceptual Object have the ability to exist on more than one particular carrier at the same time, such as paper, electronic signals, marks, audio media, paintings, photos, human memories, etc. They cannot be destroyed. They exist as long as they can be found on at least one carrier or in at least one human memory. Their existence ends when the last carrier and the last memory are lost."@en .

<http://iflastandards.info/ns/fr/frbr/frbroo/F7> a owl:Class ;
    rdfs:label "Object"@en ;
    reg:name "Object"@en ;
    reg:status <http://metadataregistry.org/uri/RegStatus/1001> ;
    rdfs:comment "This class comprises all persistent physical items with a relatively stable form, man-made or natural. [This is the beginning of scope note for E18 Physical Object in CIDOC CRM version 5.0.1]"@en ;
    rdfs:isDefinedBy <http://iflastandards.info/ns/fr/frbr/frbroo/> ;
    rdfs:subClassOf <http://www.cidoc-crm.org/cidoc-crm/E18_Physical_Thing> ;
    = <http://iflastandards.info/ns/fr/frbr/frbroo/F7_Object> ;
    skos:definition "This class comprises all persistent physical items with a relatively stable form, man-made or natural."@en .

<http://iflastandards.info/ns/fr/frbr/frbroo/F8> a owl:Class ;
    rdfs:label "Event"@en ;
    reg:name "Event"@en ;
    reg:status <http://metadataregistry.org/uri/RegStatus/1001> ;
    rdfs:comment "This class comprises sets of coherent phenomena or cultural manifestations bounded in time and space. It is the social or physical coherence of these phenomena that identify an E4 Period and not the associated spatio-temporal bounds. These bounds are a mere approximation of the actual process of growth, spread and retreat. Consequently, different periods can overlap and coexist in time and space, such as when a nomadic culture exists in the same area as a sedentary culture. Typically this class is used to describe prehistoric or historic periods such as the \"Neolithic Period\", the \"Ming Dynasty\" or the \"McCarthy Era\". There are however no assumptions about the scale of the associated phenomena. In particular all events are seen as synthetic processes consisting of coherent phenomena. Therefore E4 Period is a superclass of E5 Event. For example, a modern clinical E67 Birth can be seen as both an atomic E5 Event and as an E4 Period that consists of multiple activities performed by multiple instances of E39 Actor. There are two different conceptualisations of \"artistic style\", defined either by physical features or by historical context. For example, \"Impressionism\" can be viewed as a period lasting from approximately 1870 to 1905 during which paintings with particular characteristics were produced by a group of artists that included (among others) Monet, Renoir, Pissarro, Sisley and Degas. Alternatively, it can be regarded as a style applicable to all paintings sharing the characteristics of the works produced by the Impressionist painters, regardless of historical context. The first interpretation is an E4 Period, and the second defines morphological object types that fall under E55 Type. Another specific case of an E4 Period is the set of activities and phenomena associated with a settlement, such as the populated period of Nineveh. [This is the Scope note for E4 Period in CIDOC CRM version 5.0.1] [Note that in CIDOC CRM, E12 Production, E13 Attribute Assignment, and E65 Creation are indirect subclasses of E4 Period = F8 Event; as a consequence, F8 Event is an indirect superclass of: F27 Work Conception, F28 Expression Creation, F40 Identifier Assignment, F41 Representative Manifestation Assignment, F42 Representative Expression Assignment, F32 Carrier Production Event, F33 Reproduction Event, and F30 Publication Event]"@en ;
    rdfs:isDefinedBy <http://iflastandards.info/ns/fr/frbr/frbroo/> ;
    rdfs:subClassOf <http://www.cidoc-crm.org/cidoc-crm/E4_Period> ;
    = <http://iflastandards.info/ns/fr/frbr/frbroo/F8_Event> ;
    skos:definition "This class comprises sets of coherent phenomena or cultural manifestations bounded in time and space."@en ;
    skos:scopeNote "It is the social or physical coherence of these phenomena that identify an E4 Period and not the associated spatio-temporal bounds. These bounds are a mere approximation of the actual process of growth, spread and retreat. Consequently, different periods can overlap and coexist in time and space, such as when a nomadic culture exists in the same area as a sedentary culture.  Typically this class is used to describe prehistoric or historic periods such as the \"Neolithic Period\", the \"Ming Dynasty\" or the \"McCarthy Era\". There are however no assumptions about the scale of the associated phenomena. In particular all events are seen as synthetic processes consisting of coherent phenomena. Therefore E4 Period is a superclass of E5 Event. For example, a modern clinical E67 Birth can be seen as both an atomic E5 Event and as an E4 Period that consists of multiple activities performed by multiple instances of E39 Actor. There are two different conceptualisations of \"artistic style\", defined either by physical features or by historical context. For example, \"Impressionism\" can be viewed as a period lasting from approximately 1870 to 1905 during which paintings with particular characteristics were produced by a group of artists that included (among others) Monet, Renoir, Pissarro, Sisley and Degas. Alternatively, it can be regarded as a style applicable to all paintings sharing the characteristics of the works produced by the Impressionist painters, regardless of historical context. The first interpretation is an E4 Period, and the second defines morphological object types that fall under E55 Type. Another specific case of an E4 Period is the set of activities and phenomena associated with a settlement, such as the populated period of Nineveh."@en .

<http://iflastandards.info/ns/fr/frbr/frbroo/F9> a owl:Class ;
    rdfs:label "Place"@en ;
    reg:name "Place"@en ;
    reg:status <http://metadataregistry.org/uri/RegStatus/1001> ;
    rdfs:comment "This class comprises extents in space, in particular on the surface of the earth, in the pure sense of physics: independent from temporal phenomena and matter. The instances of E53 Place are usually determined by reference to the position of immobile objects such as buildings, cities, mountains, rivers, or dedicated geodetic marks. A Place can be determined by combining a frame of reference and a location with respect to this frame. It may be identified by one or more instances of E44 Place Appellation. It is sometimes argued that instances of E53 Place are best identified by global coordinates or absolute reference systems. However, relative references are often more relevant in the context of cultural documentation and tend to be more precise. In particular, we are often interested in position in relation to large, mobile objects, such as ships. For example, the Place at which Nelson died is known with reference to a large mobile object – H.M.S Victory. A resolution of this Place in terms of absolute coordinates would require knowledge of the movements of the vessel and the precise time of death, either of which may be revised, and the result would lack historical and cultural relevance. Any object can serve as a frame of reference for E53 Place determination. The model foresees the notion of a section of an E19 Physical Object as a valid E53 Place determination. [Scope Note for E53 Place in CIDOC CRM version 5.0.1] Note that Places may be determined by the location of historical or contemporary objects, geographic features, events or geo-political units."@en ;
    rdfs:isDefinedBy <http://iflastandards.info/ns/fr/frbr/frbroo/> ;
    rdfs:subClassOf <http://www.cidoc-crm.org/cidoc-crm/E53_Place> ;
    = <http://iflastandards.info/ns/fr/frbr/frbroo/F9_Place> ;
    skos:definition "This class comprises extents in space, in particular on the surface of the earth, in the pure sense of physics: independent from temporal phenomena and matter."@en ;
    skos:scopeNote "The instances of E53 Place are usually determined by reference to the position of immobile objects such as buildings, cities, mountains, rivers, or dedicated geodetic marks. A Place can be determined by combining a frame of reference and a location with respect to this frame. It may be identified by one or more instances of E44 Place Appellation. It is sometimes argued that instances of E53 Place are best identified by global coordinates or absolute reference systems. However, relative references are often more relevant in the context of cultural documentation and tend to be more precise. In particular, we are often interested in position in relation to large, mobile objects, such as ships. For example, the Place at which Nelson died is known with reference to a large mobile object – H.M.S Victory. A resolution of this Place in terms of absolute coordinates would require knowledge of the movements of the vessel and the precise time of death, either of which may be revised, and the result would lack historical and cultural relevance. Any object can serve as a frame of reference for E53 Place determination. The model foresees the notion of a section of an E19 Physical Object as a valid E53 Place determination. Note that Places may be determined by the location of historical or contemporary objects, geographic features, events or geo-political units."@en .

<http://iflastandards.info/ns/fr/frbr/frbroo/R33> a rdf:Property ;
    rdfs:label "has content"@en ;
    reg:name "hasContent"@en ;
    reg:status <http://metadataregistry.org/uri/RegStatus/1001> ;
    rdfs:comment "This property associates an instance of F12 Nomen with one or more equivalent serialized content models for it. In digital form the symbol arrangement constituting an instance of F12 Nomen can only be represented through a particular encoding, for example ASCII or Latin1 for the Latin script. We call such a representation a content model. The property R33.1 has encoding: E55 Type allows for specifying the encoding of a particular associated content model. Together with this specification, a content model allows for unambiguously defining a nomen independently from the encoding used for representing the content."@en ;
    rdfs:domain <http://iflastandards.info/ns/fr/frbr/frbroo/F12> ;
    rdfs:isDefinedBy <http://iflastandards.info/ns/fr/frbr/frbroo/> ;
    rdfs:range rdfs:Literal ;
    rdfs:subPropertyOf <http://www.cidoc-crm.org/cidoc-crm/P3_has_note> ;
    = <http://iflastandards.info/ns/fr/frbr/frbroo/R33_has_content> ;
    skos:definition "This property associates an instance of F12 Nomen with one or more equivalent serialized content models for it."@en ;
    skos:scopeNote "In digital form the symbol arrangement constituting an instance of F12 Nomen can only be represented through a particular encoding, for example ASCII or Latin1 for the Latin script. We call such a representation a content model. The property R33.1 has encoding: E55 Type allows for specifying the encoding of a particular associated content model. Together with this specification, a content model allows for unambiguously defining a nomen independently from the encoding used for representing the content."@en .

<http://iflastandards.info/ns/fr/frbr/frbroo/CLP104> a rdf:Property ;
    rdfs:label "subject to"@en ;
    reg:name "subjectTo"@en ;
    reg:status <http://metadataregistry.org/uri/RegStatus/1001> ;
    rdfs:comment "This property associates a publication, i.e. an instance of F3 Manifestation Product Type, with an instance of E30 Right, which applies to all exemplars of that publication, as long as they are recognised as exemplars of that publication. The rights covered by this property may include: acquisition or access authorisation; terms of availability; access restrictions on the Manifestation Product Type; etc."@en ;
    rdfs:domain <http://iflastandards.info/ns/fr/frbr/frbroo/F3> ;
    rdfs:isDefinedBy <http://iflastandards.info/ns/fr/frbr/frbroo/> ;
    rdfs:range <http://www.cidoc-crm.org/cidoc-crm/E30_Right> ;
    owl:inverseOf <http://iflastandards.info/ns/fr/frbr/frbroo/CLP104i> ;
    = <http://iflastandards.info/ns/fr/frbr/frbroo/CLP104_subject_to> ;
    skos:definition "This property associates a publication, i.e. an instance of F3 Manifestation Product Type, with an instance of E30 Right, which applies to all exemplars of that publication, as long as they are recognised as exemplars of that publication."@en ;
    skos:scopeNote "The rights covered by this property may include: acquisition or access authorisation; terms of availability; access restrictions on the Manifestation Product Type; etc."@en .

<http://iflastandards.info/ns/fr/frbr/frbroo/CLP104i> a rdf:Property ;
    rdfs:label "applies to"@en ;
    reg:name "appliesTo"@en ;
    reg:status <http://metadataregistry.org/uri/RegStatus/1001> ;
    rdfs:comment "Inverse of CLP104_subject_to."@en ;
    rdfs:domain <http://www.cidoc-crm.org/cidoc-crm/E30_Right> ;
    rdfs:isDefinedBy <http://iflastandards.info/ns/fr/frbr/frbroo/> ;
    rdfs:range <http://iflastandards.info/ns/fr/frbr/frbroo/F3> ;
    owl:inverseOf <http://iflastandards.info/ns/fr/frbr/frbroo/CLP104> ;
    = <http://iflastandards.info/ns/fr/frbr/frbroo/CLP104i_applies_to> .

<http://iflastandards.info/ns/fr/frbr/frbroo/CLP105> a rdf:Property ;
    rdfs:label "right held by"@en ;
    reg:name "rightHeldBy"@en ;
    reg:status <http://metadataregistry.org/uri/RegStatus/1001> ;
    rdfs:comment "This property associates a publication, i.e. an instance of F3 Manifestation Product Type, with an instance of E39 Actor, who holds an instance of E30 Right on all exemplars of that publication, as long as they are recognised as exemplars of that publication."@en ;
    rdfs:domain <http://iflastandards.info/ns/fr/frbr/frbroo/F3> ;
    rdfs:isDefinedBy <http://iflastandards.info/ns/fr/frbr/frbroo/> ;
    rdfs:range <http://www.cidoc-crm.org/cidoc-crm/E39_Actor> ;
    owl:inverseOf <http://iflastandards.info/ns/fr/frbr/frbroo/CLP105i> ;
    = <http://iflastandards.info/ns/fr/frbr/frbroo/CLP105_right_held_by> ;
    skos:definition "This property associates a publication, i.e. an instance of F3 Manifestation Product Type, with an instance of E39 Actor, who holds an instance of E30 Right on all exemplars of that publication, as long as they are recognised as exemplars of that publication."@en .

<http://iflastandards.info/ns/fr/frbr/frbroo/CLP105i> a rdf:Property ;
    rdfs:label "right on"@en ;
    reg:name "rightOn"@en ;
    reg:status <http://metadataregistry.org/uri/RegStatus/1001> ;
    rdfs:comment "Inverse of CLP105_right_held_by."@en ;
    rdfs:domain <http://www.cidoc-crm.org/cidoc-crm/E39_Actor> ;
    rdfs:isDefinedBy <http://iflastandards.info/ns/fr/frbr/frbroo/> ;
    rdfs:range <http://iflastandards.info/ns/fr/frbr/frbroo/F3> ;
    owl:inverseOf <http://iflastandards.info/ns/fr/frbr/frbroo/CLP105> ;
    = <http://iflastandards.info/ns/fr/frbr/frbroo/CLP105i_right_on> .

<http://iflastandards.info/ns/fr/frbr/frbroo/CLP2> a rdf:Property ;
    rdfs:label "should have type"@en ;
    reg:name "shouldHaveType"@en ;
    reg:status <http://metadataregistry.org/uri/RegStatus/1001> ;
    rdfs:comment "This property associates a publication, i.e. an instance of F3 Manifestation Product Type, with an instance of E55 Type, which all exemplars of that publication should belong to, as long as they are recognised as exemplars of that publication. Typically, this property is observed on one exemplar of a publication, and extrapolated to all other exemplars of the same publication. This logical inference is an induction along the path that can be modelled as: F3 Manifestation Product Type R7B has example F5 Item P41B was classified by E17 Type Assignment P42 assigned E55 Type. It can happen that a given exemplar, or subset of exemplars, originally produced, or intended to be produced, with that characteristic, accidentally lacks it. This fact should be recorded as a property of F5 Item, and not of F3 Manifestation Product Type."@en ;
    rdfs:domain <http://iflastandards.info/ns/fr/frbr/frbroo/F3> ;
    rdfs:isDefinedBy <http://iflastandards.info/ns/fr/frbr/frbroo/> ;
    rdfs:range <http://www.cidoc-crm.org/cidoc-crm/E55_Type> ;
    owl:inverseOf <http://iflastandards.info/ns/fr/frbr/frbroo/CLP2i> ;
    = <http://iflastandards.info/ns/fr/frbr/frbroo/CLP2_should_have_type> ;
    skos:definition "This property associates a publication, i.e. an instance of F3 Manifestation Product Type, with an instance of E55 Type, which all exemplars of that publication should belong to, as long as they are recognised as exemplars of that publication."@en ;
    skos:scopeNote "Typically, this property is observed on one exemplar of a publication, and extrapolated to all other exemplars of the same publication. This logical inference is an induction along the path that can be modelled as: F3 Manifestation Product Type R7B has example F5 Item P41B was classified by E17 Type Assignment P42 assigned E55 Type. It can happen that a given exemplar, or subset of exemplars, originally produced, or intended to be produced, with that characteristic, accidentally lacks it. This fact should be recorded as a property of F5 Item, and not of F3 Manifestation Product Type."@en .

<http://iflastandards.info/ns/fr/frbr/frbroo/CLP2i> a rdf:Property ;
    rdfs:label "should be type of"@en ;
    reg:name "shouldBeTypeOf"@en ;
    reg:status <http://metadataregistry.org/uri/RegStatus/1001> ;
    rdfs:comment "Inverse of CLP2_should_have_type."@en ;
    rdfs:domain <http://www.cidoc-crm.org/cidoc-crm/E55_Type> ;
    rdfs:isDefinedBy <http://iflastandards.info/ns/fr/frbr/frbroo/> ;
    rdfs:range <http://iflastandards.info/ns/fr/frbr/frbroo/F3> ;
    owl:inverseOf <http://iflastandards.info/ns/fr/frbr/frbroo/CLP2> ;
    = <http://iflastandards.info/ns/fr/frbr/frbroo/CLP2i_should_be_type_of> .

<http://iflastandards.info/ns/fr/frbr/frbroo/CLP43> a rdf:Property ;
    rdfs:label "should have dimension"@en ;
    reg:name "shouldHaveDimension"@en ;
    reg:status <http://metadataregistry.org/uri/RegStatus/1001> ;
    rdfs:comment "This property associates a publication, i.e. an instance of F3 Manifestation Product Type, with an instance of E54 Dimension, which all exemplars of that publication should have, as long as they are recognised as exemplars of that publication. Typically, this property is observed on one exemplar of a publication, and extrapolated to all other exemplars of the same publication. This logical inference is an induction along the path that can be modelled as: F3 Manifestation Product Type R7B has example F5 Item P39B was measured by E16 Measurement P40 observed dimension E54 Dimension. It can happen that a given exemplar, or subset of exemplars, originally produced, or intended to be produced, with that characteristic, accidentally lacks it. This fact should be recorded as a property of F5 Item, and not of F3 Manifestation Product Type."@en ;
    rdfs:domain <http://iflastandards.info/ns/fr/frbr/frbroo/F3> ;
    rdfs:isDefinedBy <http://iflastandards.info/ns/fr/frbr/frbroo/> ;
    rdfs:range <http://www.cidoc-crm.org/cidoc-crm/E54_Dimension> ;
    owl:inverseOf <http://iflastandards.info/ns/fr/frbr/frbroo/CLP43i> ;
    = <http://iflastandards.info/ns/fr/frbr/frbroo/CLP43_should_have_dimension> ;
    skos:definition "This property associates a publication, i.e. an instance of F3 Manifestation Product Type, with an instance of E54 Dimension, which all exemplars of that publication should have, as long as they are recognised as exemplars of that publication."@en ;
    skos:scopeNote "Typically, this property is observed on one exemplar of a publication, and extrapolated to all other exemplars of the same publication. This logical inference is an induction along the path that can be modelled as: F3 Manifestation Product Type R7B has example F5 Item P39B was measured by E16 Measurement P40 observed dimension E54 Dimension. It can happen that a given exemplar, or subset of exemplars, originally produced, or intended to be produced, with that characteristic, accidentally lacks it. This fact should be recorded as a property of F5 Item, and not of F3 Manifestation Product Type."@en .

<http://iflastandards.info/ns/fr/frbr/frbroo/CLP43i> a rdf:Property ;
    rdfs:label "should be dimension of"@en ;
    reg:name "shouldBeDimensionOf"@en ;
    reg:status <http://metadataregistry.org/uri/RegStatus/1001> ;
    rdfs:comment "Inverse of CLP43_should_have_dimension."@en ;
    rdfs:domain <http://www.cidoc-crm.org/cidoc-crm/E54_Dimension> ;
    rdfs:isDefinedBy <http://iflastandards.info/ns/fr/frbr/frbroo/> ;
    rdfs:range <http://iflastandards.info/ns/fr/frbr/frbroo/F3> ;
    owl:inverseOf <http://iflastandards.info/ns/fr/frbr/frbroo/CLP43> ;
    = <http://iflastandards.info/ns/fr/frbr/frbroo/CLP43i_should_be_dimension_of> .

<http://iflastandards.info/ns/fr/frbr/frbroo/CLP45> a rdf:Property ;
    rdfs:label "should consist of"@en ;
    reg:name "shouldConsistOf"@en ;
    reg:status <http://metadataregistry.org/uri/RegStatus/1001> ;
    rdfs:comment "This property associates a publication, i.e. an instance of F3 Manifestation Product Type, with an instance of E57 Material, which all exemplars of that publication should consist of, as long as they are recognised as exemplars of that publication. Typically, this property is observed on one exemplar of a publication, and extrapolated to all other exemplars of the same publication. This logical inference is an induction along the path that can be modelled as: F3 Manifestation Product Type R7B has example F5 Item P41B was classified by E17 Type Assignment P42 assigned E57 Material. It can happen that a given exemplar, or subset of exemplars, originally produced, or intended to be produced, with that characteristic, accidentally lacks it. This fact should be recorded as a property of F5 Item, and not of F3 Manifestation Product Type."@en ;
    rdfs:domain <http://iflastandards.info/ns/fr/frbr/frbroo/F3> ;
    rdfs:isDefinedBy <http://iflastandards.info/ns/fr/frbr/frbroo/> ;
    rdfs:range <http://www.cidoc-crm.org/cidoc-crm/E57_Material> ;
    owl:inverseOf <http://iflastandards.info/ns/fr/frbr/frbroo/CLP45i> ;
    = <http://iflastandards.info/ns/fr/frbr/frbroo/CLP45_should_consist_of> ;
    skos:definition "This property associates a publication, i.e. an instance of F3 Manifestation Product Type, with an instance of E57 Material, which all exemplars of that publication should consist of, as long as they are recognised as exemplars of that publication."@en ;
    skos:scopeNote "Typically, this property is observed on one exemplar of a publication, and extrapolated to all other exemplars of the same publication. This logical inference is an induction along the path that can be modelled as: F3 Manifestation Product Type R7B has example F5 Item P41B was classified by E17 Type Assignment P42 assigned E57 Material. It can happen that a given exemplar, or subset of exemplars, originally produced, or intended to be produced, with that characteristic, accidentally lacks it. This fact should be recorded as a property of F5 Item, and not of F3 Manifestation Product Type."@en .

<http://iflastandards.info/ns/fr/frbr/frbroo/CLP45i> a rdf:Property ;
    rdfs:label "should be incorporated in"@en ;
    reg:name "shouldBeIncorporatedIn"@en ;
    reg:status <http://metadataregistry.org/uri/RegStatus/1001> ;
    rdfs:comment "Inverse of CLP45_should_consist_of."@en ;
    rdfs:domain <http://www.cidoc-crm.org/cidoc-crm/E57_Material> ;
    rdfs:isDefinedBy <http://iflastandards.info/ns/fr/frbr/frbroo/> ;
    rdfs:range <http://iflastandards.info/ns/fr/frbr/frbroo/F3> ;
    owl:inverseOf <http://iflastandards.info/ns/fr/frbr/frbroo/CLP45> ;
    = <http://iflastandards.info/ns/fr/frbr/frbroo/CLP45i_should_be_incorporated_in> .

<http://iflastandards.info/ns/fr/frbr/frbroo/CLP46> a rdf:Property ;
    rdfs:label "should be composed of"@en ;
    reg:name "shouldBeComposedOf"@en ;
    reg:status <http://metadataregistry.org/uri/RegStatus/1001> ;
    rdfs:comment "This property associates an instance of F3 Manifestation Product Type which prescribes that all its Items will contain as parts an Item of another instance of F3 Manifestation Product Type with that instance of F3 Manifestation Product Type."@en ;
    rdfs:domain <http://iflastandards.info/ns/fr/frbr/frbroo/F3> ;
    rdfs:isDefinedBy <http://iflastandards.info/ns/fr/frbr/frbroo/> ;
    rdfs:range <http://iflastandards.info/ns/fr/frbr/frbroo/F3> ;
    owl:inverseOf <http://iflastandards.info/ns/fr/frbr/frbroo/CLP46i> ;
    = <http://iflastandards.info/ns/fr/frbr/frbroo/CLP46_should_be_composed_of> ;
    skos:definition "This property associates an instance of F3 Manifestation Product Type which prescribes that all its Items will contain as parts an Item of another instance of F3 Manifestation Product Type with that instance of F3 Manifestation Product Type."@en .

<http://iflastandards.info/ns/fr/frbr/frbroo/CLP46i> a rdf:Property ;
    rdfs:label "may form part of"@en ;
    reg:name "mayFormPartOf"@en ;
    reg:status <http://metadataregistry.org/uri/RegStatus/1001> ;
    rdfs:comment "Inverse of CLP46_should_be_composed_of."@en ;
    rdfs:domain <http://iflastandards.info/ns/fr/frbr/frbroo/F3> ;
    rdfs:isDefinedBy <http://iflastandards.info/ns/fr/frbr/frbroo/> ;
    rdfs:range <http://iflastandards.info/ns/fr/frbr/frbroo/F3> ;
    owl:inverseOf <http://iflastandards.info/ns/fr/frbr/frbroo/CLP46> ;
    = <http://iflastandards.info/ns/fr/frbr/frbroo/CLP46i_may_form_part_of> .

<http://iflastandards.info/ns/fr/frbr/frbroo/CLR6> a rdf:Property ;
    rdfs:label "should carry"@en ;
    reg:name "shouldCarry"@en ;
    reg:status <http://metadataregistry.org/uri/RegStatus/1001> ;
    rdfs:comment "This property associates a publication, i.e. an instance of F3 Manifestation Product Type, with an instance of F24 Publication Expression, which all exemplars of that publication should carry, as long as they are recognised as complete exemplars of that publication. Typically, this property is observed on one exemplar of a publication, and extrapolated to all other exemplars of the same publication. This logical inference is an induction along the path that can be modelled as: F3 Manifestation Product Type R7B has example F5 Item R6 carries F24 Publication Expression. It can happen that a given exemplar, or a subset of exemplars, originally produced, or intended to be produced with that characteristic, accidentally lacks part of the publication expression. This fact should be recorded as a property of F5 Item, and not of F3 Manifestation Product Type."@en ;
    rdfs:domain <http://iflastandards.info/ns/fr/frbr/frbroo/F3> ;
    rdfs:isDefinedBy <http://iflastandards.info/ns/fr/frbr/frbroo/> ;
    rdfs:range <http://iflastandards.info/ns/fr/frbr/frbroo/F24> ;
    owl:inverseOf <http://iflastandards.info/ns/fr/frbr/frbroo/CLR6i> ;
    = <http://iflastandards.info/ns/fr/frbr/frbroo/CLR6_should_carry> ;
    skos:definition "This property associates a publication, i.e. an instance of F3 Manifestation Product Type, with an instance of F24 Publication Expression, which all exemplars of that publication should carry, as long as they are recognised as complete exemplars of that publication."@en ;
    skos:scopeNote "Typically, this property is observed on one exemplar of a publication, and extrapolated to all other exemplars of the same publication. This logical inference is an induction along the path that can be modelled as: F3 Manifestation Product Type R7B has example F5 Item R6 carries F24 Publication Expression. It can happen that a given exemplar, or a subset of exemplars, originally produced, or intended to be produced with that characteristic, accidentally lacks part of the publication expression. This fact should be recorded as a property of F5 Item, and not of F3 Manifestation Product Type."@en .

<http://iflastandards.info/ns/fr/frbr/frbroo/CLR6i> a rdf:Property ;
    rdfs:label "should be carried by"@en ;
    reg:name "shouldBeCarriedBy"@en ;
    reg:status <http://metadataregistry.org/uri/RegStatus/1001> ;
    rdfs:comment "Inverse of CLR6_should_carry."@en ;
    rdfs:domain <http://iflastandards.info/ns/fr/frbr/frbroo/F24> ;
    rdfs:isDefinedBy <http://iflastandards.info/ns/fr/frbr/frbroo/> ;
    rdfs:range <http://iflastandards.info/ns/fr/frbr/frbroo/F3> ;
    owl:inverseOf <http://iflastandards.info/ns/fr/frbr/frbroo/CLR6> ;
    = <http://iflastandards.info/ns/fr/frbr/frbroo/CLR6i_should_be_carried_by> .

<http://iflastandards.info/ns/fr/frbr/frbroo/R1> a rdf:Property ;
    rdfs:label "is logical successor of"@en ;
    reg:name "isLogicalSuccessorOf"@en ;
    reg:status <http://metadataregistry.org/uri/RegStatus/1001> ;
    rdfs:comment "This property associates an instance of F1 Work which logically continues the content of another instance of F1 Work with the latter."@en ;
    rdfs:domain <http://iflastandards.info/ns/fr/frbr/frbroo/F1> ;
    rdfs:isDefinedBy <http://iflastandards.info/ns/fr/frbr/frbroo/> ;
    rdfs:range <http://iflastandards.info/ns/fr/frbr/frbroo/F1> ;
    rdfs:subPropertyOf <http://www.cidoc-crm.org/cidoc-crm/P130_shows_features_of> ;
    owl:inverseOf <http://iflastandards.info/ns/fr/frbr/frbroo/R1i> ;
    = <http://iflastandards.info/ns/fr/frbr/frbroo/R1_is_logical_successor_of> ;
    skos:definition "This property associates an instance of F1 Work which logically continues the content of another instance of F1 Work with the latter."@en .

<http://iflastandards.info/ns/fr/frbr/frbroo/R10> a rdf:Property ;
    rdfs:label "has member"@en ;
    reg:name "hasMember"@en ;
    reg:status <http://metadataregistry.org/uri/RegStatus/1001> ;
    rdfs:comment "This property associates an instance of F15 Complex Work with an instance of F1 Work that forms part of it. The Work becomes complex by the fact that it has other instances of Work as members."@en ;
    rdfs:domain <http://iflastandards.info/ns/fr/frbr/frbroo/F15> ;
    rdfs:isDefinedBy <http://iflastandards.info/ns/fr/frbr/frbroo/> ;
    rdfs:range <http://iflastandards.info/ns/fr/frbr/frbroo/F1> ;
    rdfs:subPropertyOf <http://www.cidoc-crm.org/cidoc-crm/P148_has_component> ;
    owl:inverseOf <http://iflastandards.info/ns/fr/frbr/frbroo/R10i> ;
    = <http://iflastandards.info/ns/fr/frbr/frbroo/R10_has_member> .

<http://iflastandards.info/ns/fr/frbr/frbroo/R10i> a rdf:Property ;
    rdfs:label "is member of"@en ;
    reg:name "isMemberOf"@en ;
    reg:status <http://metadataregistry.org/uri/RegStatus/1001> ;
    rdfs:comment "Inverse of R10_has_member."@en ;
    rdfs:domain <http://iflastandards.info/ns/fr/frbr/frbroo/F1> ;
    rdfs:isDefinedBy <http://iflastandards.info/ns/fr/frbr/frbroo/> ;
    rdfs:range <http://iflastandards.info/ns/fr/frbr/frbroo/F15> ;
    rdfs:subPropertyOf <http://www.cidoc-crm.org/cidoc-crm/P148i_is_component_of> ;
    owl:inverseOf <http://iflastandards.info/ns/fr/frbr/frbroo/R10> ;
    = <http://iflastandards.info/ns/fr/frbr/frbroo/R10i_is_member_of> .

<http://iflastandards.info/ns/fr/frbr/frbroo/R11> a rdf:Property ;
    rdfs:label "has issuing rule"@en ;
    reg:name "hasIssuingRule"@en ;
    reg:status <http://metadataregistry.org/uri/RegStatus/1001> ;
    rdfs:comment "This property associates an instance of F18 Serial Work with the instance of E29 Design or Procedure that specifies the issuing policy planned by this Work, such as sequencing pattern, expected frequency and expected regularity. This property is a shortcut of the full path: F18 Serial Work R23B was realised through F30 Publication Event P16 used specific object E29 Design or Procedure."@en ;
    rdfs:domain <http://iflastandards.info/ns/fr/frbr/frbroo/F18> ;
    rdfs:isDefinedBy <http://iflastandards.info/ns/fr/frbr/frbroo/> ;
    rdfs:range <http://www.cidoc-crm.org/cidoc-crm/E29_Design_or_Procedure> ;
    owl:inverseOf <http://iflastandards.info/ns/fr/frbr/frbroo/R11i> ;
    = <http://iflastandards.info/ns/fr/frbr/frbroo/R11_has_issuing_rule> ;
    skos:definition """This property associates an instance of F18 Serial Work with the instance of E29 Design or Procedure that specifies the issuing policy planned by this Work, such as sequencing pattern, expected frequency and expected regularity.
"""@en ;
    skos:scopeNote "This property is a shortcut of the full path: F18 Serial Work R23B was realised through F30 Publication Event P16 used specific object E29 Design or Procedure."@en .

<http://iflastandards.info/ns/fr/frbr/frbroo/R11i> a rdf:Property ;
    rdfs:label "is issuing rule of"@en ;
    reg:name "isIssuingRuleOf"@en ;
    reg:status <http://metadataregistry.org/uri/RegStatus/1001> ;
    rdfs:comment "Inverse of R11_has_issuing_rule."@en ;
    rdfs:domain <http://www.cidoc-crm.org/cidoc-crm/E29_Design_or_Procedure> ;
    rdfs:isDefinedBy <http://iflastandards.info/ns/fr/frbr/frbroo/> ;
    rdfs:range <http://iflastandards.info/ns/fr/frbr/frbroo/F18> ;
    owl:inverseOf <http://iflastandards.info/ns/fr/frbr/frbroo/R11> ;
    = <http://iflastandards.info/ns/fr/frbr/frbroo/R11i_is_issuing_rule_of> .

<http://iflastandards.info/ns/fr/frbr/frbroo/R12> a rdf:Property ;
    rdfs:label "is realised in Performance Plan of Performance Work"@en ;
    reg:name "isRealisedInPerformancePlanOfPerformanceWork"@en ;
    reg:status <http://metadataregistry.org/uri/RegStatus/1001> ;
    rdfs:comment "This property associates an instance of F20 Performance Work with an instance of F25 Performance Plan that consists of signs (words, figures, etc.) which express the directions the instance of F20 Performance Work consists of."@en ;
    rdfs:domain <http://iflastandards.info/ns/fr/frbr/frbroo/F20> ;
    rdfs:isDefinedBy <http://iflastandards.info/ns/fr/frbr/frbroo/> ;
    rdfs:range <http://iflastandards.info/ns/fr/frbr/frbroo/F25> ;
    rdfs:subPropertyOf <http://iflastandards.info/ns/fr/frbr/frbroo/R3> ;
    owl:inverseOf <http://iflastandards.info/ns/fr/frbr/frbroo/R12i> ;
    = <http://iflastandards.info/ns/fr/frbr/frbroo/R12_is_realised_in> ;
    skos:definition "This property associates an instance of F20 Performance Work with an instance of F25 Performance Plan that consists of signs (words, figures, etc.) which express the directions the instance of F20 Performance Work consists of."@en .

<http://iflastandards.info/ns/fr/frbr/frbroo/R12i> a rdf:Property ;
    rdfs:label "realises Performance Work by Performance Plan"@en ;
    reg:name "realisesPerformanceWorkByPerformancePlan"@en ;
    reg:status <http://metadataregistry.org/uri/RegStatus/1001> ;
    rdfs:comment "Inverse of R12_is_realised_in."@en ;
    rdfs:domain <http://iflastandards.info/ns/fr/frbr/frbroo/F25> ;
    rdfs:isDefinedBy <http://iflastandards.info/ns/fr/frbr/frbroo/> ;
    rdfs:range <http://iflastandards.info/ns/fr/frbr/frbroo/F20> ;
    rdfs:subPropertyOf <http://iflastandards.info/ns/fr/frbr/frbroo/R3i> ;
    owl:inverseOf <http://iflastandards.info/ns/fr/frbr/frbroo/R12> ;
    = <http://iflastandards.info/ns/fr/frbr/frbroo/R12i_realises> .

<http://iflastandards.info/ns/fr/frbr/frbroo/R13> a rdf:Property ;
    rdfs:label "is realised in Recording of Recording Work"@en ;
    reg:name "isRealisedInRecordingOfRecordingWork"@en ;
    reg:status <http://metadataregistry.org/uri/RegStatus/1001> ;
    rdfs:comment "This property associates an instance of F21 Recording Work with an instance of F26 Recording realising the instance of F21 Recording work. This is a shortcut of the more elaborated path through R22 was realised through, F29 Recording Event and R21 created, which should be used when information about the recording event is available."@en ;
    rdfs:domain <http://iflastandards.info/ns/fr/frbr/frbroo/F21> ;
    rdfs:isDefinedBy <http://iflastandards.info/ns/fr/frbr/frbroo/> ;
    rdfs:range <http://iflastandards.info/ns/fr/frbr/frbroo/F26> ;
    rdfs:subPropertyOf <http://iflastandards.info/ns/fr/frbr/frbroo/R3> ;
    owl:inverseOf <http://iflastandards.info/ns/fr/frbr/frbroo/R13i> ;
    = <http://iflastandards.info/ns/fr/frbr/frbroo/R13_is_realised_in> ;
    skos:definition "This property associates an instance of F21 Recording Work with an instance of F26 Recording realising the instance of F21 Recording work."@en ;
    skos:scopeNote "This is a shortcut of the more elaborated path through R22 was realised through, F29 Recording Event and R21 created, which should be used when information about the recording event is available."@en .

<http://iflastandards.info/ns/fr/frbr/frbroo/R13i> a rdf:Property ;
    rdfs:label "realises Recording Work by Recording"@en ;
    reg:name "realisesRecordingWorkByRecording"@en ;
    reg:status <http://metadataregistry.org/uri/RegStatus/1001> ;
    rdfs:comment "Inverse of R13_is_realised_in."@en ;
    rdfs:domain <http://iflastandards.info/ns/fr/frbr/frbroo/F26> ;
    rdfs:isDefinedBy <http://iflastandards.info/ns/fr/frbr/frbroo/> ;
    rdfs:range <http://iflastandards.info/ns/fr/frbr/frbroo/F21> ;
    rdfs:subPropertyOf <http://iflastandards.info/ns/fr/frbr/frbroo/R3i> ;
    owl:inverseOf <http://iflastandards.info/ns/fr/frbr/frbroo/R13> ;
    = <http://iflastandards.info/ns/fr/frbr/frbroo/R13i_realises> .

<http://iflastandards.info/ns/fr/frbr/frbroo/R14> a rdf:Property ;
    rdfs:label "incorporates"@en ;
    reg:name "incorporates"@en ;
    reg:status <http://metadataregistry.org/uri/RegStatus/1001> ;
    rdfs:comment "This property associates an instance of F22 Self-Contained Expression with an instance of F2 Expression that was included in it and that is a realisation of an independent work. The incorporated expression may be self-contained or fragmentary. This property makes it possible to recognise the autonomous status of the incorporated expression, which was created in a distinct context, and can be incorporated in many distinct self-contained expressions, and to highlight the difference between structural and accidental whole-part relationships between conceptual entities. It accounts for many cultural facts that are quite frequent and significant: the inclusion of a poem in an anthology, the re-use of an operatic aria in a new opera, the use of a reproduction of a painting for a book cover or a CD booklet, the integration of textual quotations, the presence of lyrics in a song that sets those lyrics to music, the presence of the text of a play in a movie based on that play, etc."@en ;
    rdfs:domain <http://iflastandards.info/ns/fr/frbr/frbroo/F22> ;
    rdfs:isDefinedBy <http://iflastandards.info/ns/fr/frbr/frbroo/> ;
    rdfs:range <http://iflastandards.info/ns/fr/frbr/frbroo/F2> ;
    rdfs:subPropertyOf <http://www.cidoc-crm.org/cidoc-crm/P106_is_composed_of>,
        <http://www.cidoc-crm.org/cidoc-crm/P148_has_component> ;
    owl:inverseOf <http://iflastandards.info/ns/fr/frbr/frbroo/R14i> ;
    = <http://iflastandards.info/ns/fr/frbr/frbroo/R14_incorporates> ;
    skos:definition "This property associates an instance of F22 Self-Contained Expression with an instance of F2 Expression that was included in it and that is a realisation of an independent work. The incorporated expression may be self-contained or fragmentary."@en ;
    skos:scopeNote "This property makes it possible to recognise the autonomous status of the incorporated expression, which was created in a distinct context, and can be incorporated in many distinct self-contained expressions, and to highlight the difference between structural and accidental whole-part relationships between conceptual entities. It accounts for many cultural facts that are quite frequent and significant: the inclusion of a poem in an anthology, the re-use of an operatic aria in a new opera, the use of a reproduction of a painting for a book cover or a CD booklet, the integration of textual quotations, the presence of lyrics in a song that sets those lyrics to music, the presence of the text of a play in a movie based on that play, etc."@en .

<http://iflastandards.info/ns/fr/frbr/frbroo/R14i> a rdf:Property ;
    rdfs:label "is incorporated in"@en ;
    reg:name "isIncorporatedIn"@en ;
    reg:status <http://metadataregistry.org/uri/RegStatus/1001> ;
    rdfs:comment "Inverse of R14_incorporates."@en ;
    rdfs:domain <http://iflastandards.info/ns/fr/frbr/frbroo/F2> ;
    rdfs:isDefinedBy <http://iflastandards.info/ns/fr/frbr/frbroo/> ;
    rdfs:range <http://iflastandards.info/ns/fr/frbr/frbroo/F22> ;
    rdfs:subPropertyOf <http://www.cidoc-crm.org/cidoc-crm/P106i_forms_part_of> ;
    owl:inverseOf <http://iflastandards.info/ns/fr/frbr/frbroo/R14> ;
    = <http://iflastandards.info/ns/fr/frbr/frbroo/R14i_is_incorporated_in> .

<http://iflastandards.info/ns/fr/frbr/frbroo/R15> a rdf:Property ;
    rdfs:label "has fragment"@en ;
    reg:name "hasFragment"@en ;
    reg:status <http://metadataregistry.org/uri/RegStatus/1001> ;
    rdfs:comment "This property associates the fragment of an expression and the expression of which it is a fragment."@en ;
    rdfs:domain <http://iflastandards.info/ns/fr/frbr/frbroo/F2> ;
    rdfs:isDefinedBy <http://iflastandards.info/ns/fr/frbr/frbroo/> ;
    rdfs:range <http://iflastandards.info/ns/fr/frbr/frbroo/F23> ;
    rdfs:subPropertyOf <http://www.cidoc-crm.org/cidoc-crm/P106_is_composed_of> ;
    owl:inverseOf <http://iflastandards.info/ns/fr/frbr/frbroo/R15i> ;
    = <http://iflastandards.info/ns/fr/frbr/frbroo/R15_has_fragment> ;
    skos:definition "This property associates the fragment of an expression and the expression of which it is a fragment."@en .

<http://iflastandards.info/ns/fr/frbr/frbroo/R15i> a rdf:Property ;
    rdfs:label "is fragment of"@en ;
    reg:name "isFragmentOf"@en ;
    reg:status <http://metadataregistry.org/uri/RegStatus/1001> ;
    rdfs:comment "Inverse of R15_has_fragment."@en ;
    rdfs:domain <http://iflastandards.info/ns/fr/frbr/frbroo/F23> ;
    rdfs:isDefinedBy <http://iflastandards.info/ns/fr/frbr/frbroo/> ;
    rdfs:range <http://iflastandards.info/ns/fr/frbr/frbroo/F2> ;
    rdfs:subPropertyOf <http://www.cidoc-crm.org/cidoc-crm/P106i_forms_part_of> ;
    owl:inverseOf <http://iflastandards.info/ns/fr/frbr/frbroo/R15> ;
    = <http://iflastandards.info/ns/fr/frbr/frbroo/R15i_is_fragment_of> .

<http://iflastandards.info/ns/fr/frbr/frbroo/R16> a rdf:Property ;
    rdfs:label "initiated"@en ;
    reg:name "initiated"@en ;
    reg:status <http://metadataregistry.org/uri/RegStatus/1001> ;
    rdfs:comment "This property associates the first conception of a work and the work itself that ensued from a given initial idea. It is usually not recorded in cataloguing practice as it is only exceptionally documented in real life but is required in this semantic model as it marks the origin of the causality chain that results in a work's coming into existence."@en ;
    rdfs:domain <http://iflastandards.info/ns/fr/frbr/frbroo/F27> ;
    rdfs:isDefinedBy <http://iflastandards.info/ns/fr/frbr/frbroo/> ;
    rdfs:range <http://iflastandards.info/ns/fr/frbr/frbroo/F1> ;
    rdfs:subPropertyOf <http://www.cidoc-crm.org/cidoc-crm/P94_has_created> ;
    owl:inverseOf <http://iflastandards.info/ns/fr/frbr/frbroo/R16i> ;
    = <http://iflastandards.info/ns/fr/frbr/frbroo/R16_initiated> ;
    skos:definition "This property associates the first conception of a work and the work itself that ensued from a given initial idea."@en ;
    skos:scopeNote "It is usually not recorded in cataloguing practice as it is only exceptionally documented in real life but is required in this semantic model as it marks the origin of the causality chain that results in a work's coming into existence."@en .

<http://iflastandards.info/ns/fr/frbr/frbroo/R16i> a rdf:Property ;
    rdfs:label "was initiated by"@en ;
    reg:name "wasInitiatedBy"@en ;
    reg:status <http://metadataregistry.org/uri/RegStatus/1001> ;
    rdfs:comment "Inverse of R16_initiated."@en ;
    rdfs:domain <http://iflastandards.info/ns/fr/frbr/frbroo/F1> ;
    rdfs:isDefinedBy <http://iflastandards.info/ns/fr/frbr/frbroo/> ;
    rdfs:range <http://iflastandards.info/ns/fr/frbr/frbroo/F27> ;
    rdfs:subPropertyOf <http://www.cidoc-crm.org/cidoc-crm/P94i_was_created_by> ;
    owl:inverseOf <http://iflastandards.info/ns/fr/frbr/frbroo/R16> ;
    = <http://iflastandards.info/ns/fr/frbr/frbroo/R16i_was_initiated_by> .

<http://iflastandards.info/ns/fr/frbr/frbroo/R18> a rdf:Property ;
    rdfs:label "created Manifestation Singleton from Expression Creation"@en ;
    reg:name "createdManifestationSingletonFromExpressionCreation"@en ;
    reg:status <http://metadataregistry.org/uri/RegStatus/1001> ;
    rdfs:comment "This property associates an instance of F28 Expression Creation with the first physical objects in which the resulting instance of F2 Expression was embodied."@en ;
    rdfs:domain <http://iflastandards.info/ns/fr/frbr/frbroo/F28> ;
    rdfs:isDefinedBy <http://iflastandards.info/ns/fr/frbr/frbroo/> ;
    rdfs:range <http://iflastandards.info/ns/fr/frbr/frbroo/F4> ;
    rdfs:subPropertyOf <http://www.cidoc-crm.org/cidoc-crm/P108_has_produced> ;
    owl:inverseOf <http://iflastandards.info/ns/fr/frbr/frbroo/R18i> ;
    = <http://iflastandards.info/ns/fr/frbr/frbroo/R18_created> ;
    skos:definition "This property associates an instance of F28 Expression Creation with the first physical objects in which the resulting instance of F2 Expression was embodied."@en .

<http://iflastandards.info/ns/fr/frbr/frbroo/R18i> a rdf:Property ;
    rdfs:label "was created by Expression Creation for Manifestation Singleton"@en ;
    reg:name "wasCreatedByExpressionCreationForManifestationSingleton"@en ;
    reg:status <http://metadataregistry.org/uri/RegStatus/1001> ;
    rdfs:comment "Inverse of R18_created."@en ;
    rdfs:domain <http://iflastandards.info/ns/fr/frbr/frbroo/F4> ;
    rdfs:isDefinedBy <http://iflastandards.info/ns/fr/frbr/frbroo/> ;
    rdfs:range <http://iflastandards.info/ns/fr/frbr/frbroo/F28> ;
    rdfs:subPropertyOf <http://www.cidoc-crm.org/cidoc-crm/P108i_was_produced_by> ;
    owl:inverseOf <http://iflastandards.info/ns/fr/frbr/frbroo/R18> ;
    = <http://iflastandards.info/ns/fr/frbr/frbroo/R18i_was_created_by> .

<http://iflastandards.info/ns/fr/frbr/frbroo/R1i> a rdf:Property ;
    rdfs:label "has successor"@en ;
    reg:name "hasSuccessor"@en ;
    reg:status <http://metadataregistry.org/uri/RegStatus/1001> ;
    rdfs:comment "Inverse of R1_is_logical_successor_of."@en ;
    rdfs:domain <http://iflastandards.info/ns/fr/frbr/frbroo/F1> ;
    rdfs:isDefinedBy <http://iflastandards.info/ns/fr/frbr/frbroo/> ;
    rdfs:range <http://iflastandards.info/ns/fr/frbr/frbroo/F1> ;
    rdfs:subPropertyOf <http://www.cidoc-crm.org/cidoc-crm/P130i_features_are_also_found_on> ;
    owl:inverseOf <http://iflastandards.info/ns/fr/frbr/frbroo/R1> ;
    = <http://iflastandards.info/ns/fr/frbr/frbroo/R1i_has_successor> .

<http://iflastandards.info/ns/fr/frbr/frbroo/R2> a rdf:Property ;
    rdfs:label "is derivative of"@en ;
    reg:name "isDerivativeOf"@en ;
    reg:status <http://metadataregistry.org/uri/RegStatus/1001> ;
    rdfs:comment "This property associates an instance of F1 Work which modifies the content of another instance of F1 Work with the latter. The property R2.1 has type of this property allows for specifying the kind of derivation, such as adaptation, summarisation etc."@en ;
    rdfs:domain <http://iflastandards.info/ns/fr/frbr/frbroo/F1> ;
    rdfs:isDefinedBy <http://iflastandards.info/ns/fr/frbr/frbroo/> ;
    rdfs:range <http://iflastandards.info/ns/fr/frbr/frbroo/F1> ;
    rdfs:subPropertyOf <http://www.cidoc-crm.org/cidoc-crm/P130_shows_features_of> ;
    owl:inverseOf <http://iflastandards.info/ns/fr/frbr/frbroo/R2i> ;
    = <http://iflastandards.info/ns/fr/frbr/frbroo/R2_is_derivative_of> ;
    skos:definition "This property associates an instance of F1 Work which modifies the content of another instance of F1 Work with the latter."@en ;
    skos:scopeNote "The property R2.1 has type of this property allows for specifying the kind of derivation, such as adaptation, summarisation etc."@en .

<http://iflastandards.info/ns/fr/frbr/frbroo/R20> a rdf:Property ;
    rdfs:label "recorded"@en ;
    reg:name "recorded"@en ;
    reg:status <http://metadataregistry.org/uri/RegStatus/1001> ;
    rdfs:comment "This property associates an instance of F29 Recording Event with the instance of E5 Event which was captured."@en ;
    rdfs:domain <http://iflastandards.info/ns/fr/frbr/frbroo/F29> ;
    rdfs:isDefinedBy <http://iflastandards.info/ns/fr/frbr/frbroo/> ;
    rdfs:range <http://www.cidoc-crm.org/cidoc-crm/E2_Temporal_Entity> ;
    rdfs:subPropertyOf <http://www.cidoc-crm.org/cidoc-crm/P15_was_influenced_by> ;
    owl:inverseOf <http://iflastandards.info/ns/fr/frbr/frbroo/R20i> ;
    = <http://iflastandards.info/ns/fr/frbr/frbroo/R20_recorded> ;
    skos:definition "This property associates an instance of F29 Recording Event with the instance of E5 Event which was captured."@en .

<http://iflastandards.info/ns/fr/frbr/frbroo/R20i> a rdf:Property ;
    rdfs:label "was recorded through"@en ;
    reg:name "wasRecordedThrough"@en ;
    reg:status <http://metadataregistry.org/uri/RegStatus/1001> ;
    rdfs:comment "Inverse of R20_recorded."@en ;
    rdfs:domain <http://www.cidoc-crm.org/cidoc-crm/E2_Temporal_Entity> ;
    rdfs:isDefinedBy <http://iflastandards.info/ns/fr/frbr/frbroo/> ;
    rdfs:range <http://iflastandards.info/ns/fr/frbr/frbroo/F29> ;
    rdfs:subPropertyOf <http://www.cidoc-crm.org/cidoc-crm/P15i_influenced> ;
    owl:inverseOf <http://iflastandards.info/ns/fr/frbr/frbroo/R20> ;
    = <http://iflastandards.info/ns/fr/frbr/frbroo/R20i_was_recorded_through> .

<http://iflastandards.info/ns/fr/frbr/frbroo/R21> a rdf:Property ;
    rdfs:label "created Recording from Recording Event"@en ;
    reg:name "createdRecordingFromRecordingEvent"@en ;
    reg:status <http://metadataregistry.org/uri/RegStatus/1001> ;
    rdfs:comment "This property associates an instance of F29 Recording Event with the instance of F26 Recording that was created."@en ;
    rdfs:domain <http://iflastandards.info/ns/fr/frbr/frbroo/F29> ;
    rdfs:isDefinedBy <http://iflastandards.info/ns/fr/frbr/frbroo/> ;
    rdfs:range <http://iflastandards.info/ns/fr/frbr/frbroo/F26> ;
    rdfs:subPropertyOf <http://iflastandards.info/ns/fr/frbr/frbroo/R17> ;
    owl:inverseOf <http://iflastandards.info/ns/fr/frbr/frbroo/R21i> ;
    = <http://iflastandards.info/ns/fr/frbr/frbroo/R21_created> ;
    skos:definition "This property associates an instance of F29 Recording Event with the instance of F26 Recording that was created."@en .

<http://iflastandards.info/ns/fr/frbr/frbroo/R21i> a rdf:Property ;
    rdfs:label "was created through Recording Event for Recording"@en ;
    reg:name "wasCreatedThroughRecordingEventForRecording"@en ;
    reg:status <http://metadataregistry.org/uri/RegStatus/1001> ;
    rdfs:comment "Inverse of R21_created."@en ;
    rdfs:domain <http://iflastandards.info/ns/fr/frbr/frbroo/F26> ;
    rdfs:isDefinedBy <http://iflastandards.info/ns/fr/frbr/frbroo/> ;
    rdfs:range <http://iflastandards.info/ns/fr/frbr/frbroo/F29> ;
    rdfs:subPropertyOf <http://iflastandards.info/ns/fr/frbr/frbroo/R17i> ;
    owl:inverseOf <http://iflastandards.info/ns/fr/frbr/frbroo/R21> ;
    = <http://iflastandards.info/ns/fr/frbr/frbroo/R21i_was_created_through> .

<http://iflastandards.info/ns/fr/frbr/frbroo/R22> a rdf:Property ;
    rdfs:label "created a realization of Recording Work by Recording Event"@en ;
    reg:name "createdARealizationOfRecordingWorkByRecordingEvent"@en ;
    reg:status <http://metadataregistry.org/uri/RegStatus/1001> ;
    rdfs:comment "This property associates an instance of F29 Recording Event with the instance of F21 Recording Work it realised."@en ;
    rdfs:domain <http://iflastandards.info/ns/fr/frbr/frbroo/F29> ;
    rdfs:isDefinedBy <http://iflastandards.info/ns/fr/frbr/frbroo/> ;
    rdfs:range <http://iflastandards.info/ns/fr/frbr/frbroo/F21> ;
    rdfs:subPropertyOf <http://iflastandards.info/ns/fr/frbr/frbroo/R19> ;
    owl:inverseOf <http://iflastandards.info/ns/fr/frbr/frbroo/R22i> ;
    = <http://iflastandards.info/ns/fr/frbr/frbroo/R22_created_a_realization_of> ;
    skos:definition "This property associates an instance of F29 Recording Event with the instance of F21 Recording Work it realised."@en .

<http://iflastandards.info/ns/fr/frbr/frbroo/R22i> a rdf:Property ;
    rdfs:label "was realised through Recording Event for Recording Work"@en ;
    reg:name "wasRealisedThroughRecordingEventForRecordingWork"@en ;
    reg:status <http://metadataregistry.org/uri/RegStatus/1001> ;
    rdfs:comment "Inverse of R22_created_a_realization_of."@en ;
    rdfs:domain <http://iflastandards.info/ns/fr/frbr/frbroo/F21> ;
    rdfs:isDefinedBy <http://iflastandards.info/ns/fr/frbr/frbroo/> ;
    rdfs:range <http://iflastandards.info/ns/fr/frbr/frbroo/F29> ;
    rdfs:subPropertyOf <http://iflastandards.info/ns/fr/frbr/frbroo/R19i> ;
    owl:inverseOf <http://iflastandards.info/ns/fr/frbr/frbroo/R22> ;
    = <http://iflastandards.info/ns/fr/frbr/frbroo/R22i_was_realised_through> .

<http://iflastandards.info/ns/fr/frbr/frbroo/R23> a rdf:Property ;
    rdfs:label "created a realization of Publication Work by Publication Event"@en ;
    reg:name "createdARealizationOfPublicationWorkbyPublicationEvent"@en ;
    reg:status <http://metadataregistry.org/uri/RegStatus/1001> ;
    rdfs:comment "This property associates an instance of F30 Publication Event with the instance of F19 Publication Work it realised."@en ;
    rdfs:domain <http://iflastandards.info/ns/fr/frbr/frbroo/F30> ;
    rdfs:isDefinedBy <http://iflastandards.info/ns/fr/frbr/frbroo/> ;
    rdfs:range <http://iflastandards.info/ns/fr/frbr/frbroo/F19> ;
    rdfs:subPropertyOf <http://iflastandards.info/ns/fr/frbr/frbroo/R19> ;
    owl:inverseOf <http://iflastandards.info/ns/fr/frbr/frbroo/R23i> ;
    = <http://iflastandards.info/ns/fr/frbr/frbroo/R23_created_a_realization_of> ;
    skos:definition "This property associates an instance of F30 Publication Event with the instance of F19 Publication Work it realised."@en .

<http://iflastandards.info/ns/fr/frbr/frbroo/R23i> a rdf:Property ;
    rdfs:label "was realised through Publication Event for Publication Work"@en ;
    reg:name "wasRealisedThroughPublicationEventForPublicationWork"@en ;
    reg:status <http://metadataregistry.org/uri/RegStatus/1001> ;
    rdfs:comment "Inverse of R23_created_a_realization_of."@en ;
    rdfs:domain <http://iflastandards.info/ns/fr/frbr/frbroo/F19> ;
    rdfs:isDefinedBy <http://iflastandards.info/ns/fr/frbr/frbroo/> ;
    rdfs:range <http://iflastandards.info/ns/fr/frbr/frbroo/F30> ;
    rdfs:subPropertyOf <http://iflastandards.info/ns/fr/frbr/frbroo/R19i> ;
    owl:inverseOf <http://iflastandards.info/ns/fr/frbr/frbroo/R23> ;
    = <http://iflastandards.info/ns/fr/frbr/frbroo/R23i_was_realised_through> .

<http://iflastandards.info/ns/fr/frbr/frbroo/R24> a rdf:Property ;
    rdfs:label "created Publication Expression from Publication Event"@en ;
    reg:name "createdPublicationExpressionFromPublicationEvent"@en ;
    reg:status <http://metadataregistry.org/uri/RegStatus/1001> ;
    rdfs:comment "This property associates the instance of F24 Publication Expression that was created during a particular F30 Publication Event with that F30 Publication Event."@en ;
    rdfs:domain <http://iflastandards.info/ns/fr/frbr/frbroo/F30> ;
    rdfs:isDefinedBy <http://iflastandards.info/ns/fr/frbr/frbroo/> ;
    rdfs:range <http://iflastandards.info/ns/fr/frbr/frbroo/F24> ;
    rdfs:subPropertyOf <http://iflastandards.info/ns/fr/frbr/frbroo/R17> ;
    owl:inverseOf <http://iflastandards.info/ns/fr/frbr/frbroo/R24i> ;
    = <http://iflastandards.info/ns/fr/frbr/frbroo/R24_created> ;
    skos:definition "This property associates the instance of F24 Publication Expression that was created during a particular F30 Publication Event with that F30 Publication Event."@en .

<http://iflastandards.info/ns/fr/frbr/frbroo/R24i> a rdf:Property ;
    rdfs:label "was created through Publication Event for Publication Expression"@en ;
    reg:name "wasCreatedThroughPublicationEventForPublicationExpression"@en ;
    reg:status <http://metadataregistry.org/uri/RegStatus/1001> ;
    rdfs:comment "Inverse of R24_created."@en ;
    rdfs:domain <http://iflastandards.info/ns/fr/frbr/frbroo/F24> ;
    rdfs:isDefinedBy <http://iflastandards.info/ns/fr/frbr/frbroo/> ;
    rdfs:range <http://iflastandards.info/ns/fr/frbr/frbroo/F30> ;
    rdfs:subPropertyOf <http://iflastandards.info/ns/fr/frbr/frbroo/R17i> ;
    owl:inverseOf <http://iflastandards.info/ns/fr/frbr/frbroo/R24> ;
    = <http://iflastandards.info/ns/fr/frbr/frbroo/R24i_was_created_through> .

<http://iflastandards.info/ns/fr/frbr/frbroo/R25> a rdf:Property ;
    rdfs:label "performed Performance Plan by Performance"@en ;
    reg:name "performedPerformancePlanByPerformance"@en ;
    reg:status <http://metadataregistry.org/uri/RegStatus/1001> ;
    rdfs:comment "This property associates an instance of F31 Performance with the instance of F25 Performance Plan to which all those participating in the performance were supposed to conform."@en ;
    rdfs:domain <http://iflastandards.info/ns/fr/frbr/frbroo/F31> ;
    rdfs:isDefinedBy <http://iflastandards.info/ns/fr/frbr/frbroo/> ;
    rdfs:range <http://iflastandards.info/ns/fr/frbr/frbroo/F25> ;
    rdfs:subPropertyOf <http://www.cidoc-crm.org/cidoc-crm/P33_used_specific_technique> ;
    owl:inverseOf <http://iflastandards.info/ns/fr/frbr/frbroo/R25i> ;
    = <http://iflastandards.info/ns/fr/frbr/frbroo/R25_performed> ;
    skos:definition "This property associates an instance of F31 Performance with the instance of F25 Performance Plan to which all those participating in the performance were supposed to conform."@en .

<http://iflastandards.info/ns/fr/frbr/frbroo/R25i> a rdf:Property ;
    rdfs:label "was performed in"@en ;
    reg:name "wasPerformedIn"@en ;
    reg:status <http://metadataregistry.org/uri/RegStatus/1001> ;
    rdfs:comment "Inverse of R25_performed."@en ;
    rdfs:domain <http://iflastandards.info/ns/fr/frbr/frbroo/F25> ;
    rdfs:isDefinedBy <http://iflastandards.info/ns/fr/frbr/frbroo/> ;
    rdfs:range <http://iflastandards.info/ns/fr/frbr/frbroo/F31> ;
    rdfs:subPropertyOf <http://www.cidoc-crm.org/cidoc-crm/P33i_was_used_by> ;
    owl:inverseOf <http://iflastandards.info/ns/fr/frbr/frbroo/R25> ;
    = <http://iflastandards.info/ns/fr/frbr/frbroo/R25i_was_performed_in> .

<http://iflastandards.info/ns/fr/frbr/frbroo/R26> a rdf:Property ;
    rdfs:label "produced things of type"@en ;
    reg:name "producedThingsOfType"@en ;
    reg:status <http://metadataregistry.org/uri/RegStatus/1001> ;
    rdfs:comment "This property associates an instance of F32 Carrier Production Event with the instance of F3 Manifestation Product Type it produced items of."@en ;
    rdfs:domain <http://iflastandards.info/ns/fr/frbr/frbroo/F32> ;
    rdfs:isDefinedBy <http://iflastandards.info/ns/fr/frbr/frbroo/> ;
    rdfs:range <http://iflastandards.info/ns/fr/frbr/frbroo/F3> ;
    owl:inverseOf <http://iflastandards.info/ns/fr/frbr/frbroo/R26i> ;
    = <http://iflastandards.info/ns/fr/frbr/frbroo/R26_produced_things_of_type> ;
    skos:definition "This property associates an instance of F32 Carrier Production Event with the instance of F3 Manifestation Product Type it produced items of."@en .

<http://iflastandards.info/ns/fr/frbr/frbroo/R26i> a rdf:Property ;
    rdfs:label "was produced by Carrier Production Event for Manifestation Product Type"@en ;
    reg:name "wasProducedByCarrierProductionEventForManifestationProductType"@en ;
    reg:status <http://metadataregistry.org/uri/RegStatus/1001> ;
    rdfs:comment "Inverse of R26_produced_things_of_type."@en ;
    rdfs:domain <http://iflastandards.info/ns/fr/frbr/frbroo/F3> ;
    rdfs:isDefinedBy <http://iflastandards.info/ns/fr/frbr/frbroo/> ;
    rdfs:range <http://iflastandards.info/ns/fr/frbr/frbroo/F32> ;
    owl:inverseOf <http://iflastandards.info/ns/fr/frbr/frbroo/R26> ;
    = <http://iflastandards.info/ns/fr/frbr/frbroo/R26i_was_produced_by> .

<http://iflastandards.info/ns/fr/frbr/frbroo/R27> a rdf:Property ;
    rdfs:label "used as source material"@en ;
    reg:name "usedAsSourceMaterial"@en ;
    reg:status <http://metadataregistry.org/uri/RegStatus/1001> ;
    rdfs:comment "This property associates an instance of F32 Carrier Production Event with the set of signs provided by the publisher to be carried by all of the produced items."@en ;
    rdfs:domain <http://iflastandards.info/ns/fr/frbr/frbroo/F32> ;
    rdfs:isDefinedBy <http://iflastandards.info/ns/fr/frbr/frbroo/> ;
    rdfs:range <http://iflastandards.info/ns/fr/frbr/frbroo/F24> ;
    rdfs:subPropertyOf <http://www.cidoc-crm.org/cidoc-crm/P16_used_specific_object> ;
    owl:inverseOf <http://iflastandards.info/ns/fr/frbr/frbroo/R27i> ;
    = <http://iflastandards.info/ns/fr/frbr/frbroo/R27_used_as_source_material> ;
    skos:definition "This property associates an instance of F32 Carrier Production Event with the set of signs provided by the publisher to be carried by all of the produced items."@en .

<http://iflastandards.info/ns/fr/frbr/frbroo/R27i> a rdf:Property ;
    rdfs:label "was used by"@en ;
    reg:name "wasUsedBy"@en ;
    reg:status <http://metadataregistry.org/uri/RegStatus/1001> ;
    rdfs:comment "Inverse of R27_used_as_source_material."@en ;
    rdfs:domain <http://iflastandards.info/ns/fr/frbr/frbroo/F24> ;
    rdfs:isDefinedBy <http://iflastandards.info/ns/fr/frbr/frbroo/> ;
    rdfs:range <http://iflastandards.info/ns/fr/frbr/frbroo/F32> ;
    rdfs:subPropertyOf <http://www.cidoc-crm.org/cidoc-crm/P16i_was_used_for> ;
    owl:inverseOf <http://iflastandards.info/ns/fr/frbr/frbroo/R27> ;
    = <http://iflastandards.info/ns/fr/frbr/frbroo/R27i_was_used_by> .

<http://iflastandards.info/ns/fr/frbr/frbroo/R28> a rdf:Property ;
    rdfs:label "produced Item from Carrier Production Event"@en ;
    reg:name "producedItemFromCarrierProductionEvent"@en ;
    reg:status <http://metadataregistry.org/uri/RegStatus/1001> ;
    rdfs:comment "This property associates an instance of F32 Carrier Production Event with any one of the produced items (i.e., the instances of F5 Item)."@en ;
    rdfs:domain <http://iflastandards.info/ns/fr/frbr/frbroo/F32> ;
    rdfs:isDefinedBy <http://iflastandards.info/ns/fr/frbr/frbroo/> ;
    rdfs:range <http://iflastandards.info/ns/fr/frbr/frbroo/F5> ;
    rdfs:subPropertyOf <http://www.cidoc-crm.org/cidoc-crm/P108_has_produced> ;
    owl:inverseOf <http://iflastandards.info/ns/fr/frbr/frbroo/R28i> ;
    = <http://iflastandards.info/ns/fr/frbr/frbroo/R28_produced> ;
    skos:definition "This property associates an instance of F32 Carrier Production Event with any one of the produced items (i.e., the instances of F5 Item)."@en .

<http://iflastandards.info/ns/fr/frbr/frbroo/R28i> a rdf:Property ;
    rdfs:label "was produced by Carrier Production Event for Item"@en ;
    reg:name "wasProducedByCarrierProductionEventForItem"@en ;
    reg:status <http://metadataregistry.org/uri/RegStatus/1001> ;
    rdfs:comment "Inverse of R28_produced."@en ;
    rdfs:domain <http://iflastandards.info/ns/fr/frbr/frbroo/F5> ;
    rdfs:isDefinedBy <http://iflastandards.info/ns/fr/frbr/frbroo/> ;
    rdfs:range <http://iflastandards.info/ns/fr/frbr/frbroo/F32> ;
    rdfs:subPropertyOf <http://www.cidoc-crm.org/cidoc-crm/P108i_was_produced_by> ;
    owl:inverseOf <http://iflastandards.info/ns/fr/frbr/frbroo/R28> ;
    = <http://iflastandards.info/ns/fr/frbr/frbroo/R28i_was_produced_by> .

<http://iflastandards.info/ns/fr/frbr/frbroo/R29> a rdf:Property ;
    rdfs:label "reproduced"@en ;
    reg:name "reproduced"@en ;
    reg:status <http://metadataregistry.org/uri/RegStatus/1001> ;
    rdfs:comment "This property associates an instance of F33 Reproduction Event with an instance of E84 Information Carrier it reproduces."@en ;
    rdfs:domain <http://iflastandards.info/ns/fr/frbr/frbroo/F33> ;
    rdfs:isDefinedBy <http://iflastandards.info/ns/fr/frbr/frbroo/> ;
    rdfs:range <http://www.cidoc-crm.org/cidoc-crm/E84_Information_Carrier> ;
    rdfs:subPropertyOf <http://www.cidoc-crm.org/cidoc-crm/P16_used_specific_object> ;
    owl:inverseOf <http://iflastandards.info/ns/fr/frbr/frbroo/R29i> ;
    = <http://iflastandards.info/ns/fr/frbr/frbroo/R29_reproduced> ;
    skos:definition "This property associates an instance of F33 Reproduction Event with an instance of E84 Information Carrier it reproduces."@en .

<http://iflastandards.info/ns/fr/frbr/frbroo/R29i> a rdf:Property ;
    rdfs:label "was reproduced by"@en ;
    reg:name "wasReproducedBy"@en ;
    reg:status <http://metadataregistry.org/uri/RegStatus/1001> ;
    rdfs:comment "Inverse of R29_reproduced."@en ;
    rdfs:domain <http://www.cidoc-crm.org/cidoc-crm/E84_Information_Carrier> ;
    rdfs:isDefinedBy <http://iflastandards.info/ns/fr/frbr/frbroo/> ;
    rdfs:range <http://iflastandards.info/ns/fr/frbr/frbroo/F33> ;
    rdfs:subPropertyOf <http://www.cidoc-crm.org/cidoc-crm/P16i_was_used_for> ;
    owl:inverseOf <http://iflastandards.info/ns/fr/frbr/frbroo/R29> ;
    = <http://iflastandards.info/ns/fr/frbr/frbroo/R29i_was_reproduced_by> .

<http://iflastandards.info/ns/fr/frbr/frbroo/R2i> a rdf:Property ;
    rdfs:label "has derivative"@en ;
    reg:name "hasDerivative"@en ;
    reg:status <http://metadataregistry.org/uri/RegStatus/1001> ;
    rdfs:comment "Inverse of R2_is_derivative_of."@en ;
    rdfs:domain <http://iflastandards.info/ns/fr/frbr/frbroo/F1> ;
    rdfs:isDefinedBy <http://iflastandards.info/ns/fr/frbr/frbroo/> ;
    rdfs:range <http://iflastandards.info/ns/fr/frbr/frbroo/F1> ;
    rdfs:subPropertyOf <http://www.cidoc-crm.org/cidoc-crm/P130i_features_are_also_found_on> ;
    owl:inverseOf <http://iflastandards.info/ns/fr/frbr/frbroo/R2> ;
    = <http://iflastandards.info/ns/fr/frbr/frbroo/R2i_has_derivative> .

<http://iflastandards.info/ns/fr/frbr/frbroo/R30> a rdf:Property ;
    rdfs:label "produced Information Carrier from Reproduction Event"@en ;
    reg:name "producedInformationCarrierFromReproductionEvent"@en ;
    reg:status <http://metadataregistry.org/uri/RegStatus/1001> ;
    rdfs:comment "This property associates an instance of F33 Reproduction Event with an instance of E84 Information Carrier it produces."@en ;
    rdfs:domain <http://iflastandards.info/ns/fr/frbr/frbroo/F33> ;
    rdfs:isDefinedBy <http://iflastandards.info/ns/fr/frbr/frbroo/> ;
    rdfs:range <http://www.cidoc-crm.org/cidoc-crm/E84_Information_Carrier> ;
    rdfs:subPropertyOf <http://www.cidoc-crm.org/cidoc-crm/P108_has_produced> ;
    owl:inverseOf <http://iflastandards.info/ns/fr/frbr/frbroo/R30i> ;
    = <http://iflastandards.info/ns/fr/frbr/frbroo/R30_produced> ;
    skos:definition "This property associates an instance of F33 Reproduction Event with an instance of E84 Information Carrier it produces."@en .

<http://iflastandards.info/ns/fr/frbr/frbroo/R30i> a rdf:Property ;
    rdfs:label "was produced by"@en ;
    reg:name "wasProducedBy"@en ;
    reg:status <http://metadataregistry.org/uri/RegStatus/1001> ;
    rdfs:comment "Inverse of R30_produced."@en ;
    rdfs:domain <http://www.cidoc-crm.org/cidoc-crm/E84_Information_Carrier> ;
    rdfs:isDefinedBy <http://iflastandards.info/ns/fr/frbr/frbroo/> ;
    rdfs:range <http://iflastandards.info/ns/fr/frbr/frbroo/F33> ;
    rdfs:subPropertyOf <http://www.cidoc-crm.org/cidoc-crm/P108i_was_produced_by> ;
    owl:inverseOf <http://iflastandards.info/ns/fr/frbr/frbroo/R30> ;
    = <http://iflastandards.info/ns/fr/frbr/frbroo/R30i_was_produced_by> .

<http://iflastandards.info/ns/fr/frbr/frbroo/R31> a rdf:Property ;
    rdfs:label "is reproduction of Information Carrier for Information Carrier"@en ;
    reg:name "isReproductionOfInformationCarrierForInformationCarrier"@en ;
    reg:status <http://metadataregistry.org/uri/RegStatus/1001> ;
    rdfs:comment "This property associates an instance of E84 Information Carrier which is a reproduction of another instance of E84 Information Carrier with the latter. It is considered that a reproduction of multiple originals resulting in a single product requires a merging of those objects prior to the reproduction. Therefore an Information Carrier is regarded to be a reproduction of one and only one original. This property is a shortcut of the more fully developed path from E84 Information Carrier through R30 produced (was produced by), F33 Reproduction Event R29 reproduced (was reproduced by) to E84 Information Carrier."@en ;
    rdfs:domain <http://www.cidoc-crm.org/cidoc-crm/E84_Information_Carrier> ;
    rdfs:isDefinedBy <http://iflastandards.info/ns/fr/frbr/frbroo/> ;
    rdfs:range <http://www.cidoc-crm.org/cidoc-crm/E84_Information_Carrier> ;
    rdfs:subPropertyOf <http://www.cidoc-crm.org/cidoc-crm/P130_shows_features_of> ;
    owl:inverseOf <http://iflastandards.info/ns/fr/frbr/frbroo/R31i> ;
    = <http://iflastandards.info/ns/fr/frbr/frbroo/R31_is_reproduction_of> ;
    skos:definition "This property associates an instance of E84 Information Carrier which is a reproduction of another instance of E84 Information Carrier with the latter."@en ;
    skos:scopeNote "It is considered that a reproduction of multiple originals resulting in a single product requires a merging of those objects prior to the reproduction. Therefore an Information Carrier is regarded to be a reproduction of one and only one original. This property is a shortcut of the more fully developed path from E84 Information Carrier through R30 produced (was produced by), F33 Reproduction Event R29 reproduced (was reproduced by) to E84 Information Carrier."@en .

<http://iflastandards.info/ns/fr/frbr/frbroo/R31i> a rdf:Property ;
    rdfs:label "has reproduction"@en ;
    reg:name "hasReproduction"@en ;
    reg:status <http://metadataregistry.org/uri/RegStatus/1001> ;
    rdfs:comment "Inverse of R31_is_reproduction_of."@en ;
    rdfs:domain <http://www.cidoc-crm.org/cidoc-crm/E84_Information_Carrier> ;
    rdfs:isDefinedBy <http://iflastandards.info/ns/fr/frbr/frbroo/> ;
    rdfs:range <http://www.cidoc-crm.org/cidoc-crm/E84_Information_Carrier> ;
    rdfs:subPropertyOf <http://www.cidoc-crm.org/cidoc-crm/P130i_features_are_also_found_on> ;
    owl:inverseOf <http://iflastandards.info/ns/fr/frbr/frbroo/R31> ;
    = <http://iflastandards.info/ns/fr/frbr/frbroo/R31i_has_reproduction> .

<http://iflastandards.info/ns/fr/frbr/frbroo/R32> a rdf:Property ;
    rdfs:label "is reproduction of Name Use Activity for Nomen Use Statement"@en ;
    reg:name "isReproductionOfNameUseActivityForNomenUseStatement"@en ;
    reg:status <http://metadataregistry.org/uri/RegStatus/1001> ;
    rdfs:comment "This property associates an instance of F35 Nomen Use Statement with an instance of F52 Name Use Activity which provides evidence for the use of the particular nomen in the stated sense. The association between this name use activity and a source for it may be described by the property P70 documents (is documented in)."@en ;
    rdfs:domain <http://iflastandards.info/ns/fr/frbr/frbroo/F35> ;
    rdfs:isDefinedBy <http://iflastandards.info/ns/fr/frbr/frbroo/> ;
    rdfs:range <http://iflastandards.info/ns/fr/frbr/frbroo/F52> ;
    rdfs:subPropertyOf <http://www.cidoc-crm.org/cidoc-crm/P67_refers_to> ;
    owl:inverseOf <http://iflastandards.info/ns/fr/frbr/frbroo/R32i> ;
    = <http://iflastandards.info/ns/fr/frbr/frbroo/R32_is_warranted_by> ;
    skos:definition "This property associates an instance of F35 Nomen Use Statement with an instance of F52 Name Use Activity which provides evidence for the use of the particular nomen in the stated sense."@en ;
    skos:scopeNote "The association between this name use activity and a source for it may be described by the property P70 documents (is documented in)."@en .

<http://iflastandards.info/ns/fr/frbr/frbroo/R32i> a rdf:Property ;
    rdfs:label "warrants"@en ;
    reg:name "warrants"@en ;
    reg:status <http://metadataregistry.org/uri/RegStatus/1001> ;
    rdfs:comment "Inverse of R32_is_warranted_by."@en ;
    rdfs:domain <http://iflastandards.info/ns/fr/frbr/frbroo/F52> ;
    rdfs:isDefinedBy <http://iflastandards.info/ns/fr/frbr/frbroo/> ;
    rdfs:range <http://iflastandards.info/ns/fr/frbr/frbroo/F35> ;
    rdfs:subPropertyOf <http://www.cidoc-crm.org/cidoc-crm/P67i_is_referred_to_by> ;
    owl:inverseOf <http://iflastandards.info/ns/fr/frbr/frbroo/R32> ;
    = <http://iflastandards.info/ns/fr/frbr/frbroo/R32i_warrants> .

<http://iflastandards.info/ns/fr/frbr/frbroo/R34> a rdf:Property ;
    rdfs:label "has validity period"@en ;
    reg:name "hasValidityPeriod"@en ;
    reg:status <http://metadataregistry.org/uri/RegStatus/1001> ;
    rdfs:comment "This property associates an instance of F34 KOS with the instance of E52 Time-Span describing the period for which the particular KOS Expression was regarded as valid by its maintainers. Each change of validity status of a nomen use statement within a KOS should be associated with a release change of the KOS. The individual time-span of a validity state of a nomen would be the union of the time-spans of the KOS in which the Nomen was declared to have the particular validity status (provisional, accepted, obsolete etc. …)."@en ;
    rdfs:domain <http://iflastandards.info/ns/fr/frbr/frbroo/F34> ;
    rdfs:isDefinedBy <http://iflastandards.info/ns/fr/frbr/frbroo/> ;
    rdfs:range <http://www.cidoc-crm.org/cidoc-crm/E52_Time-Span> ;
    owl:inverseOf <http://iflastandards.info/ns/fr/frbr/frbroo/R34i> ;
    = <http://iflastandards.info/ns/fr/frbr/frbroo/R34_has_validity_period> ;
    skos:definition "This property associates an instance of F34 KOS with the instance of E52 Time-Span describing the period for which the particular KOS Expression was regarded as valid by its maintainers."@en ;
    skos:scopeNote "Each change of validity status of a nomen use statement within a KOS should be associated with a release change of the KOS. The individual time-span of a validity state of a nomen would be the union of the time-spans of the KOS in which the Nomen was declared to have the particular validity status (provisional, accepted, obsolete …)."@en .

<http://iflastandards.info/ns/fr/frbr/frbroo/R34i> a rdf:Property ;
    rdfs:label "is validity period of"@en ;
    reg:name "isValidityPeriodOf"@en ;
    reg:status <http://metadataregistry.org/uri/RegStatus/1001> ;
    rdfs:comment "Inverse of R34_has_validity_period."@en ;
    rdfs:domain <http://www.cidoc-crm.org/cidoc-crm/E52_Time-Span> ;
    rdfs:isDefinedBy <http://iflastandards.info/ns/fr/frbr/frbroo/> ;
    rdfs:range <http://iflastandards.info/ns/fr/frbr/frbroo/F34> ;
    owl:inverseOf <http://iflastandards.info/ns/fr/frbr/frbroo/R34> ;
    = <http://iflastandards.info/ns/fr/frbr/frbroo/R34i_is_validity_period_of> .

<http://iflastandards.info/ns/fr/frbr/frbroo/R35> a rdf:Property ;
    rdfs:label "specified by"@en ;
    reg:name "specifiedBy"@en ;
    reg:status <http://metadataregistry.org/uri/RegStatus/1001> ;
    rdfs:comment "This property associates an instance of F35 Nomen Use Statement with an instance of F34 KOS in which the Nomen Use Statement has a given status. The property R35.1 allows for specifying the particular status of the nomen use statement within the KOS. An instance of R35 is specified by should have only one status."@en ;
    rdfs:domain <http://iflastandards.info/ns/fr/frbr/frbroo/F35> ;
    rdfs:isDefinedBy <http://iflastandards.info/ns/fr/frbr/frbroo/> ;
    rdfs:range <http://iflastandards.info/ns/fr/frbr/frbroo/F34> ;
    rdfs:subPropertyOf <http://www.cidoc-crm.org/cidoc-crm/P148_has_component> ;
    owl:inverseOf <http://iflastandards.info/ns/fr/frbr/frbroo/R35i> ;
    = <http://iflastandards.info/ns/fr/frbr/frbroo/R35_specified_by> ;
    skos:definition "This property associates an instance of F35 Nomen Use Statement with an instance of F34 KOS in which the Nomen Use Statement has a given status."@en ;
    skos:scopeNote "The property R35.1 allows for specifying the particular status of the nomen use statement within the KOS. An instance of R35 is specified by should have only one status."@en .

<http://iflastandards.info/ns/fr/frbr/frbroo/R35i> a rdf:Property ;
    rdfs:label "specifies"@en ;
    reg:name "specifies"@en ;
    reg:status <http://metadataregistry.org/uri/RegStatus/1001> ;
    rdfs:comment "Inverse of R35_specified_by."@en ;
    rdfs:domain <http://iflastandards.info/ns/fr/frbr/frbroo/F34> ;
    rdfs:isDefinedBy <http://iflastandards.info/ns/fr/frbr/frbroo/> ;
    rdfs:range <http://iflastandards.info/ns/fr/frbr/frbroo/F35> ;
    rdfs:subPropertyOf <http://www.cidoc-crm.org/cidoc-crm/P148i_is_component_of> ;
    owl:inverseOf <http://iflastandards.info/ns/fr/frbr/frbroo/R35> ;
    = <http://iflastandards.info/ns/fr/frbr/frbroo/R35i_specifies> .

<http://iflastandards.info/ns/fr/frbr/frbroo/R36> a rdf:Property ;
    rdfs:label "uses script conversion"@en ;
    reg:name "usesScriptConversion"@en ;
    reg:status <http://metadataregistry.org/uri/RegStatus/1001> ;
    rdfs:comment "This property associates an instance of F35 Nomen Use Statement with the instance of F36 Script Conversion that was used to create the Nomen referred to in the Nomen Use Statement. The source of this conversion may or may not be explicitly mentioned. Is shortcut of: F35 Nomen Use Statement R17 was created by (created) F28 Expression Creation P33 used specific technique (was used by) E29 Design or Procedure."@en ;
    rdfs:domain <http://iflastandards.info/ns/fr/frbr/frbroo/F35> ;
    rdfs:isDefinedBy <http://iflastandards.info/ns/fr/frbr/frbroo/> ;
    rdfs:range <http://iflastandards.info/ns/fr/frbr/frbroo/F36> ;
    owl:inverseOf <http://iflastandards.info/ns/fr/frbr/frbroo/R36i> ;
    = <http://iflastandards.info/ns/fr/frbr/frbroo/R36_uses_script_conversion> ;
    skos:definition "This property associates an instance of F35 Nomen Use Statement with the instance of F36 Script Conversion that was used to create the Nomen referred to in the Nomen Use Statement."@en ;
    skos:scopeNote "The source of this conversion may or may not be explicitly mentioned. Is shortcut of: F35 Nomen Use Statement R17 was created by (created) F28 Expression Creation P33 used specific technique (was used by) E29 Design or Procedure."@en .

<http://iflastandards.info/ns/fr/frbr/frbroo/R36i> a rdf:Property ;
    rdfs:label "is script conversion used in"@en ;
    reg:name "isScriptConversionUsedIn"@en ;
    reg:status <http://metadataregistry.org/uri/RegStatus/1001> ;
    rdfs:comment "Inverse of R36_uses_script_conversion."@en ;
    rdfs:domain <http://iflastandards.info/ns/fr/frbr/frbroo/F36> ;
    rdfs:isDefinedBy <http://iflastandards.info/ns/fr/frbr/frbroo/> ;
    rdfs:range <http://iflastandards.info/ns/fr/frbr/frbroo/F35> ;
    owl:inverseOf <http://iflastandards.info/ns/fr/frbr/frbroo/R36> ;
    = <http://iflastandards.info/ns/fr/frbr/frbroo/R36i_is_script_conversion_used_in> .

<http://iflastandards.info/ns/fr/frbr/frbroo/R37> a rdf:Property ;
    rdfs:label "states as nomen"@en ;
    reg:name "statesAsNomen"@en ;
    reg:status <http://metadataregistry.org/uri/RegStatus/1001> ;
    rdfs:comment "This property associates an instance of F35 Nomen Use Statement with the instance of F12 Nomen for which it declares usage"@en ;
    rdfs:domain <http://iflastandards.info/ns/fr/frbr/frbroo/F35> ;
    rdfs:isDefinedBy <http://iflastandards.info/ns/fr/frbr/frbroo/> ;
    rdfs:range <http://iflastandards.info/ns/fr/frbr/frbroo/F12> ;
    rdfs:subPropertyOf <http://www.cidoc-crm.org/cidoc-crm/P67_refers_to> ;
    owl:inverseOf <http://iflastandards.info/ns/fr/frbr/frbroo/R37i> ;
    = <http://iflastandards.info/ns/fr/frbr/frbroo/R37_states_as_nomen> ;
    skos:definition "This property associates an instance of F35 Nomen Use Statement with the instance of F12 Nomen for which it declares usage"@en .

<http://iflastandards.info/ns/fr/frbr/frbroo/R37i> a rdf:Property ;
    rdfs:label "is stated as nomen in"@en ;
    reg:name "isStatedAsNomenIn"@en ;
    reg:status <http://metadataregistry.org/uri/RegStatus/1001> ;
    rdfs:comment "Inverse of R37_states_as_nomen."@en ;
    rdfs:domain <http://iflastandards.info/ns/fr/frbr/frbroo/F12> ;
    rdfs:isDefinedBy <http://iflastandards.info/ns/fr/frbr/frbroo/> ;
    rdfs:range <http://iflastandards.info/ns/fr/frbr/frbroo/F35> ;
    rdfs:subPropertyOf <http://www.cidoc-crm.org/cidoc-crm/P67i_is_referred_to_by> ;
    owl:inverseOf <http://iflastandards.info/ns/fr/frbr/frbroo/R37> ;
    = <http://iflastandards.info/ns/fr/frbr/frbroo/R37i_is_stated_as_nomen_in> .

<http://iflastandards.info/ns/fr/frbr/frbroo/R38> a rdf:Property ;
    rdfs:label "refers to thema"@en ;
    reg:name "refersToThema"@en ;
    reg:status <http://metadataregistry.org/uri/RegStatus/1001> ;
    rdfs:comment "This property associates an instance of F35 Nomen Use Statement with the instance of E1 CRM Entity for which it declares the usage of a nomen."@en ;
    rdfs:domain <http://iflastandards.info/ns/fr/frbr/frbroo/F35> ;
    rdfs:isDefinedBy <http://iflastandards.info/ns/fr/frbr/frbroo/> ;
    rdfs:range <http://www.cidoc-crm.org/cidoc-crm/E1_CRM_Entity> ;
    owl:inverseOf <http://iflastandards.info/ns/fr/frbr/frbroo/R38i> ;
    = <http://iflastandards.info/ns/fr/frbr/frbroo/R38_refers_to_thema> ;
    skos:definition "This property associates an instance of F35 Nomen Use Statement with the instance of E1 CRM Entity for which it declares the usage of a nomen."@en .

<http://iflastandards.info/ns/fr/frbr/frbroo/R38i> a rdf:Property ;
    rdfs:label "is thema of"@en ;
    reg:name "isThemaOf"@en ;
    reg:status <http://metadataregistry.org/uri/RegStatus/1001> ;
    rdfs:comment "Inverse of R38_refers_to_thema."@en ;
    rdfs:domain <http://www.cidoc-crm.org/cidoc-crm/E1_CRM_Entity> ;
    rdfs:isDefinedBy <http://iflastandards.info/ns/fr/frbr/frbroo/> ;
    rdfs:range <http://iflastandards.info/ns/fr/frbr/frbroo/F35> ;
    owl:inverseOf <http://iflastandards.info/ns/fr/frbr/frbroo/R38> ;
    = <http://iflastandards.info/ns/fr/frbr/frbroo/R38i_is_thema_of> .

<http://iflastandards.info/ns/fr/frbr/frbroo/R39> a rdf:Property ;
    rdfs:label "is intended for"@en ;
    reg:name "isIntendedFor"@en ;
    reg:status <http://metadataregistry.org/uri/RegStatus/1001> ;
    rdfs:comment "This property associates an instance of F35 Nomen Use Statement with an instance of E74 Group which is the target audience for which the associated nomen use is intended. To indicate that the associated nomen is declared as preferred in all contexts, the instance of E74 Group is \"mankind\"."@en ;
    rdfs:domain <http://iflastandards.info/ns/fr/frbr/frbroo/F35> ;
    rdfs:isDefinedBy <http://iflastandards.info/ns/fr/frbr/frbroo/> ;
    rdfs:range <http://www.cidoc-crm.org/cidoc-crm/E74_Group> ;
    rdfs:subPropertyOf <http://www.cidoc-crm.org/cidoc-crm/P67_refers_to> ;
    owl:inverseOf <http://iflastandards.info/ns/fr/frbr/frbroo/R39i> ;
    = <http://iflastandards.info/ns/fr/frbr/frbroo/R39_is_intended_for> ;
    skos:definition "This property associates an instance of F35 Nomen Use Statement with an instance of E74 Group which is the target audience for which the associated nomen use is intended."@en ;
    skos:scopeNote "To indicate that the associated nomen is declared as preferred in all contexts, the instance of E74 Group is \"mankind\"."@en .

<http://iflastandards.info/ns/fr/frbr/frbroo/R39i> a rdf:Property ;
    rdfs:label "is target audience in"@en ;
    reg:name "isTargetAudienceIn"@en ;
    reg:status <http://metadataregistry.org/uri/RegStatus/1001> ;
    rdfs:comment "Inverse of R39_is_intended_for."@en ;
    rdfs:domain <http://www.cidoc-crm.org/cidoc-crm/E74_Group> ;
    rdfs:isDefinedBy <http://iflastandards.info/ns/fr/frbr/frbroo/> ;
    rdfs:range <http://iflastandards.info/ns/fr/frbr/frbroo/F35> ;
    rdfs:subPropertyOf <http://www.cidoc-crm.org/cidoc-crm/P67i_is_referred_to_by> ;
    owl:inverseOf <http://iflastandards.info/ns/fr/frbr/frbroo/R39> ;
    = <http://iflastandards.info/ns/fr/frbr/frbroo/R39i_is_target_audience_in> .

<http://iflastandards.info/ns/fr/frbr/frbroo/R40> a rdf:Property ;
    rdfs:label "has representative expression"@en ;
    reg:name "hasRepresentativeExpression"@en ;
    reg:status <http://metadataregistry.org/uri/RegStatus/1001> ;
    rdfs:comment "This property identifies an instance of F22 Self-Contained Expression that has been chosen as the most characteristic expression of the instance of F1 Work of which it is an expression. There is no other semantic implication to this notion of being characteristic than to be an adequate candidate to uniquely identify the Work realized by it. Prototypically, this is the instance of F22 Self-Contained Expression that is deemed characteristic of an instance of F15 Complex Work. Typically, any expression that is not regarded as \"representative\" for the work it expresses, would require a uniform title, with qualifiers specifying the differences between that expression and a representative expression, although this may not always be done in practice. The title of a Work may not be one taken from a representative expression. A given work can have more than one representative expression, provided the differences between these expressions are not deemed \"substantial\". If the anticipated needs of users are not considered to call for bibliographic distinctions between variant expressions of a work, then even expressions that differ significantly from each other can be regarded as equally representative for the work. (See FRBR: Final Report, p. 19-20). A given expression can be deemed representative for a work with regard to some of its aspects (e.g., the text contained in an edition the title proper of which reads \"The tragicall historie of HAMLET Prince of Denmarke\", and the language of that text), and not representative for it with regard to some other aspects (e.g., the title proper \"The tragicall historie of HAMLET Prince of Denmarke\" itself, which, being different from the title that is regarded as \"representative\" for Shakespeare's work, will require the use of a uniform title). R40 has representative expression is a shortcut of the more developed path F1 Work R50B was assigned by F42 Representative Expression Assignment R51 assigned F2 Expression."@en ;
    rdfs:domain <http://iflastandards.info/ns/fr/frbr/frbroo/F1> ;
    rdfs:isDefinedBy <http://iflastandards.info/ns/fr/frbr/frbroo/> ;
    rdfs:range <http://iflastandards.info/ns/fr/frbr/frbroo/F22> ;
    rdfs:subPropertyOf <http://iflastandards.info/ns/fr/frbr/frbroo/R3> ;
    owl:inverseOf <http://iflastandards.info/ns/fr/frbr/frbroo/R40i> ;
    = <http://iflastandards.info/ns/fr/frbr/frbroo/R40_has_representative_expression> ;
    skos:definition "This property identifies an instance of F22 Self-Contained Expression that has been chosen as the most characteristic expression of the instance of F1 Work of which it is an expression."@en ;
    skos:scopeNote "There is no other semantic implication to this notion of being characteristic than to be an adequate candidate to uniquely identify the Work realized by it. Prototypically, this is the instance of F22 Self-Contained Expression that is deemed characteristic of an instance of F15 Complex Work. Typically, any expression that is not regarded as \"representative\" for the work it expresses, would require a uniform title, with qualifiers specifying the differences between that expression and a representative expression, although this may not always be done in practice. The title of a Work may not be one taken from a representative expression. A given work can have more than one representative expression, provided the differences between these expressions are not deemed \"substantial\". If the anticipated needs of users are not considered to call for bibliographic distinctions between variant expressions of a work, then even expressions that differ significantly from each other can be regarded as equally representative for the work. (See FRBR: Final Report, p. 19-20). A given expression can be deemed representative for a work with regard to some of its aspects (e.g., the text contained in an edition the title proper of which reads \"The tragicall historie of HAMLET Prince of Denmarke\", and the language of that text), and not representative for it with regard to some other aspects (e.g., the title proper \"The tragicall historie of HAMLET Prince of Denmarke\" itself, which, being different from the title that is regarded as \"representative\" for Shakespeare's work, will require the use of a uniform title). R40 has representative expression is a shortcut of the more developed path F1 Work R50B was assigned by F42 Representative Expression Assignment R51 assigned F2 Expression."@en .

<http://iflastandards.info/ns/fr/frbr/frbroo/R40i> a rdf:Property ;
    rdfs:label "is representative expression for"@en ;
    reg:name "isRepresentativeExpressionFor"@en ;
    reg:status <http://metadataregistry.org/uri/RegStatus/1001> ;
    rdfs:comment "Inverse of R40_has_representative_expression."@en ;
    rdfs:domain <http://iflastandards.info/ns/fr/frbr/frbroo/F22> ;
    rdfs:isDefinedBy <http://iflastandards.info/ns/fr/frbr/frbroo/> ;
    rdfs:range <http://iflastandards.info/ns/fr/frbr/frbroo/F1> ;
    rdfs:subPropertyOf <http://iflastandards.info/ns/fr/frbr/frbroo/R3i> ;
    owl:inverseOf <http://iflastandards.info/ns/fr/frbr/frbroo/R40> ;
    = <http://iflastandards.info/ns/fr/frbr/frbroo/R40i_is_representative_expression_for> .

<http://iflastandards.info/ns/fr/frbr/frbroo/R41> a rdf:Property ;
    rdfs:label "has representative manifestation product type"@en ;
    reg:name "hasRepresentativeManifestationProductType"@en ;
    reg:status <http://metadataregistry.org/uri/RegStatus/1001> ;
    rdfs:comment "This property identifies an instance of F3 Manifestation Product Type that has been chosen as the most characteristic Manifestation Product Type of the instance of F2 Expression of which it is a manifestation. Identifying an instance of F3 Manifestation Product Type that is representative for an instance of F2 Expression makes it possible in turn to identify an instance of F2 Expression that is representative for an instance of F1 Work, and to decide what should be regarded as the title of the work. The title of an Expression may not be one taken from a representative Manifestation Product Type or Manifestation Singleton. A given expression can have more than one Representative Manifestation Product Type. R41 has representative manifestation product type is a shortcut of the more developed path F2 Expression R48B was assigned by F41 Representative Manifestation Assignment R49 assigned F3 Manifestation Product Type."@en ;
    rdfs:domain <http://iflastandards.info/ns/fr/frbr/frbroo/F2> ;
    rdfs:isDefinedBy <http://iflastandards.info/ns/fr/frbr/frbroo/> ;
    rdfs:range <http://iflastandards.info/ns/fr/frbr/frbroo/F3> ;
    rdfs:subPropertyOf <http://iflastandards.info/ns/fr/frbr/frbroo/R4> ;
    owl:inverseOf <http://iflastandards.info/ns/fr/frbr/frbroo/R41i> ;
    = <http://iflastandards.info/ns/fr/frbr/frbroo/R41_has_representative_manifestation_product_type> ;
    skos:definition "This property identifies an instance of F3 Manifestation Product Type that has been chosen as the most characteristic Manifestation Product Type of the instance of F2 Expression of which it is a manifestation."@en ;
    skos:scopeNote "Identifying an instance of F3 Manifestation Product Type that is representative for an instance of F2 Expression makes it possible in turn to identify an instance of F2 Expression that is representative for an instance of F1 Work, and to decide what should be regarded as the title of the work. The title of an Expression may not be one taken from a representative Manifestation Product Type or Manifestation Singleton. A given expression can have more than one Representative Manifestation Product Type. R41 has representative manifestation product type is a shortcut of the more developed path F2 Expression R48B was assigned by F41 Representative Manifestation Assignment R49 assigned F3 Manifestation Product Type."@en .

<http://iflastandards.info/ns/fr/frbr/frbroo/R41i> a rdf:Property ;
    rdfs:label "is representative manifestation product type for"@en ;
    reg:name "isRepresentativeManifestationProductTypeFor"@en ;
    reg:status <http://metadataregistry.org/uri/RegStatus/1001> ;
    rdfs:comment "Inverse of R41_has_representative_manifestation_product_type."@en ;
    rdfs:domain <http://iflastandards.info/ns/fr/frbr/frbroo/F3> ;
    rdfs:isDefinedBy <http://iflastandards.info/ns/fr/frbr/frbroo/> ;
    rdfs:range <http://iflastandards.info/ns/fr/frbr/frbroo/F2> ;
    rdfs:subPropertyOf <http://iflastandards.info/ns/fr/frbr/frbroo/R4i> ;
    owl:inverseOf <http://iflastandards.info/ns/fr/frbr/frbroo/R41> ;
    = <http://iflastandards.info/ns/fr/frbr/frbroo/R41i_is_representative_manifestation_product_type_for> .

<http://iflastandards.info/ns/fr/frbr/frbroo/R42> a rdf:Property ;
    rdfs:label "is representative manifestation singleton for"@en ;
    reg:name "isRepresentativeManifestationSingletonFor"@en ;
    reg:status <http://metadataregistry.org/uri/RegStatus/1001> ;
    rdfs:comment "This property identifies an instance of Manifestation Singleton that has been declared as the unique representative for an instance of F2 Expression by some bibliographic agency. This property identifies an instance of F4 Manifestation Singleton that has been chosen as the most characteristic Manifestation Singleton of the instance of F2 Expression of which it is a manifestation. Identifying an instance of F4 Manifestation Singleton that is representative for an instance of F2 Expression makes it possible in turn to identify an instance of F2 Expression that is representative for an instance of F1 Work, and to decide what should be regarded as the title of the work. The title of an Expression may not be one taken from a representative Manifestation Product Type or Manifestation Singleton. A given expression can have more than one representative Manifestation Singleton. It is a shortcut for the more developed path: F2 Expression R48B was assigned by F41 Representative Manifestation Assignment R53 assigned F4 Manifestation Singleton."@en ;
    rdfs:domain <http://iflastandards.info/ns/fr/frbr/frbroo/F4> ;
    rdfs:isDefinedBy <http://iflastandards.info/ns/fr/frbr/frbroo/> ;
    rdfs:range <http://iflastandards.info/ns/fr/frbr/frbroo/F2> ;
    rdfs:subPropertyOf <http://www.cidoc-crm.org/cidoc-crm/P128_carries> ;
    owl:inverseOf <http://iflastandards.info/ns/fr/frbr/frbroo/R42i> ;
    = <http://iflastandards.info/ns/fr/frbr/frbroo/R42_is_representative_manifestation_singleton_for> ;
    skos:definition "This property identifies an instance of Manifestation Singleton that has been declared as the unique representative for an instance of F2 Expression by some bibliographic agency. This property identifies an instance of F4 Manifestation Singleton that has been chosen as the most characteristic Manifestation Singleton of the instance of F2 Expression of which it is a manifestation."@en ;
    skos:scopeNote "Identifying an instance of F4 Manifestation Singleton that is representative for an instance of F2 Expression makes it possible in turn to identify an instance of F2 Expression that is representative for an instance of F1 Work, and to decide what should be regarded as the title of the work. The title of an Expression may not be one taken from a representative Manifestation Product Type or Manifestation Singleton. A given expression can have more than one representative Manifestation Singleton. It is a shortcut for the more developed path: F2 Expression R48B was assigned by F41 Representative Manifestation Assignment R53 assigned F4 Manifestation Singleton."@en .

<http://iflastandards.info/ns/fr/frbr/frbroo/R42i> a rdf:Property ;
    rdfs:label "has representative manifestation singleton"@en ;
    reg:name "hasRepresentativeManifestationSingleton"@en ;
    reg:status <http://metadataregistry.org/uri/RegStatus/1001> ;
    rdfs:comment "Inverse of R42_is_representative_manifestation_singleton_for."@en ;
    rdfs:domain <http://iflastandards.info/ns/fr/frbr/frbroo/F2> ;
    rdfs:isDefinedBy <http://iflastandards.info/ns/fr/frbr/frbroo/> ;
    rdfs:range <http://iflastandards.info/ns/fr/frbr/frbroo/F4> ;
    rdfs:subPropertyOf <http://www.cidoc-crm.org/cidoc-crm/P128i_is_carried_by> ;
    owl:inverseOf <http://iflastandards.info/ns/fr/frbr/frbroo/R42> ;
    = <http://iflastandards.info/ns/fr/frbr/frbroo/R42i_has_representative_manifestation_singleton> .

<http://iflastandards.info/ns/fr/frbr/frbroo/R43> a rdf:Property ;
    rdfs:label "carried out by Bibliographic Agency in Representative Manifestation Assignment"@en ;
    reg:name "carriedOutByBibliographicAgencyInRepresentativeManifestationAssignment"@en ;
    reg:status <http://metadataregistry.org/uri/RegStatus/1001> ;
    rdfs:comment "This property associates a bibliographic agency (represented by one or more of its cataloguers) and the assigning of which Manifestation (i.e., which instance of F3 Manifestation Product Type or F4 Manifestation Singleton) is representative for a given expression. In cataloguing practice, such a relationship is usually just implicit. However, it can become explicit, for example when a bibliographic agency creates an authority record for a given work and fills the \"Source\" field with information about the publication that contains the expression that was used by the bibliographic agency to establish the uniform title for the work realised in that expression."@en ;
    rdfs:domain <http://iflastandards.info/ns/fr/frbr/frbroo/F41> ;
    rdfs:isDefinedBy <http://iflastandards.info/ns/fr/frbr/frbroo/> ;
    rdfs:range <http://iflastandards.info/ns/fr/frbr/frbroo/F44> ;
    rdfs:subPropertyOf <http://www.cidoc-crm.org/cidoc-crm/P14_carried_out_by> ;
    owl:inverseOf <http://iflastandards.info/ns/fr/frbr/frbroo/R43i> ;
    = <http://iflastandards.info/ns/fr/frbr/frbroo/R43_carried_out_by> ;
    skos:definition "This property associates a bibliographic agency (represented by one or more of its cataloguers) and the assigning of which Manifestation (i.e., which instance of F3 Manifestation Product Type or F4 Manifestation Singleton) is representative for a given expression."@en ;
    skos:scopeNote "In cataloguing practice, such a relationship is usually just implicit. However, it can become explicit, for example when a bibliographic agency creates an authority record for a given work and fills the \"Source\" field with information about the publication that contains the expression that was used by the bibliographic agency to establish the uniform title for the work realised in that expression."@en .

<http://iflastandards.info/ns/fr/frbr/frbroo/R43i> a rdf:Property ;
    rdfs:label "performed Representative Manifestation Assignment by Bibliographic Agency"@en ;
    reg:name "performed RepresentativeManifestation Assignment by Bibliographic Agency"@en ;
    reg:status <http://metadataregistry.org/uri/RegStatus/1001> ;
    rdfs:comment "Inverse of R43_carried_out_by."@en ;
    rdfs:domain <http://iflastandards.info/ns/fr/frbr/frbroo/F44> ;
    rdfs:isDefinedBy <http://iflastandards.info/ns/fr/frbr/frbroo/> ;
    rdfs:range <http://iflastandards.info/ns/fr/frbr/frbroo/F41> ;
    rdfs:subPropertyOf <http://www.cidoc-crm.org/cidoc-crm/P14i_performed> ;
    owl:inverseOf <http://iflastandards.info/ns/fr/frbr/frbroo/R43> ;
    = <http://iflastandards.info/ns/fr/frbr/frbroo/R43i_performed> .

<http://iflastandards.info/ns/fr/frbr/frbroo/R44> a rdf:Property ;
    rdfs:label "carried out by Bibliographic Agency in Representative Expression Assignment"@en ;
    reg:name "carriedOutByBibliographicAgencyInRepresentativeExpressionAssignment"@en ;
    reg:status <http://metadataregistry.org/uri/RegStatus/1001> ;
    rdfs:comment "This property associates a bibliographic agency (represented by one or more of its cataloguers) and the assigning of which expression is representative for a given Work. In cataloguing practice, such a relationship is usually just implicit. However, it can become explicit, for example when a bibliographic agency creates an authority record for a given work and fills the \"Source\" field with information about the publication that contains the expression that was used by the bibliographic agency to establish the uniform title for the work realised in that expression."@en ;
    rdfs:domain <http://iflastandards.info/ns/fr/frbr/frbroo/F42> ;
    rdfs:isDefinedBy <http://iflastandards.info/ns/fr/frbr/frbroo/> ;
    rdfs:range <http://iflastandards.info/ns/fr/frbr/frbroo/F44> ;
    rdfs:subPropertyOf <http://www.cidoc-crm.org/cidoc-crm/P14_carried_out_by> ;
    owl:inverseOf <http://iflastandards.info/ns/fr/frbr/frbroo/R44i> ;
    = <http://iflastandards.info/ns/fr/frbr/frbroo/R44_carried_out_by> ;
    skos:definition "This property associates a bibliographic agency (represented by one or more of its cataloguers) and the assigning of which expression is representative for a given Work."@en ;
    skos:scopeNote "In cataloguing practice, such a relationship is usually just implicit. However, it can become explicit, for example when a bibliographic agency creates an authority record for a given work and fills the \"Source\" field with information about the publication that contains the expression that was used by the bibliographic agency to establish the uniform title for the work realised in that expression."@en .

<http://iflastandards.info/ns/fr/frbr/frbroo/R44i> a rdf:Property ;
    rdfs:label "performed Representative Expression Assignment by Bibliographic Agency"@en ;
    reg:name "performedRepresentativeExpressionAssignmentByBibliographicAgency"@en ;
    reg:status <http://metadataregistry.org/uri/RegStatus/1001> ;
    rdfs:comment "Inverse of R44_carried_out_by."@en ;
    rdfs:domain <http://iflastandards.info/ns/fr/frbr/frbroo/F44> ;
    rdfs:isDefinedBy <http://iflastandards.info/ns/fr/frbr/frbroo/> ;
    rdfs:range <http://iflastandards.info/ns/fr/frbr/frbroo/F42> ;
    rdfs:subPropertyOf <http://www.cidoc-crm.org/cidoc-crm/P14i_performed> ;
    owl:inverseOf <http://iflastandards.info/ns/fr/frbr/frbroo/R44> ;
    = <http://iflastandards.info/ns/fr/frbr/frbroo/R44i_performed> .

<http://iflastandards.info/ns/fr/frbr/frbroo/R45> a rdf:Property ;
    rdfs:label "assigned to Entity by Identifier Assignment"@en ;
    reg:name "assignedToEntityByIdentifierAssignment"@en ;
    reg:status <http://metadataregistry.org/uri/RegStatus/1001> ;
    rdfs:comment "This property identifies the entity to which an actor, such as a bibliographic agency, assigned an instance of F13 Identifier."@en ;
    rdfs:domain <http://iflastandards.info/ns/fr/frbr/frbroo/F40> ;
    rdfs:isDefinedBy <http://iflastandards.info/ns/fr/frbr/frbroo/> ;
    rdfs:range <http://www.cidoc-crm.org/cidoc-crm/E1_CRM_Entity> ;
    rdfs:subPropertyOf <http://www.cidoc-crm.org/cidoc-crm/P140_assigned_attribute_to> ;
    owl:inverseOf <http://iflastandards.info/ns/fr/frbr/frbroo/R45i> ;
    = <http://iflastandards.info/ns/fr/frbr/frbroo/R45_assigned_to> ;
    skos:definition "This property identifies the entity to which an actor, such as a bibliographic agency, assigned an instance of F13 Identifier."@en .

<http://iflastandards.info/ns/fr/frbr/frbroo/R45i> a rdf:Property ;
    rdfs:label "was assigned by"@en ;
    reg:name "wasAssignedBy"@en ;
    reg:status <http://metadataregistry.org/uri/RegStatus/1001> ;
    rdfs:comment "Inverse of R45_assigned_to."@en ;
    rdfs:domain <http://www.cidoc-crm.org/cidoc-crm/E1_CRM_Entity> ;
    rdfs:isDefinedBy <http://iflastandards.info/ns/fr/frbr/frbroo/> ;
    rdfs:range <http://iflastandards.info/ns/fr/frbr/frbroo/F40> ;
    rdfs:subPropertyOf <http://www.cidoc-crm.org/cidoc-crm/P140i_was_attributed_by> ;
    owl:inverseOf <http://iflastandards.info/ns/fr/frbr/frbroo/R45> ;
    = <http://iflastandards.info/ns/fr/frbr/frbroo/R45i_was_assigned_by> .

<http://iflastandards.info/ns/fr/frbr/frbroo/R46> a rdf:Property ;
    rdfs:label "assigned to Identifier by Identifier Assignment"@en ;
    reg:name "assignedToIdentifieByIdentifierAssignment"@en ;
    reg:status <http://metadataregistry.org/uri/RegStatus/1001> ;
    rdfs:comment "This property associates the instance of F13 Identifier assigned to an instance of E1 CRM Entity and the event of assigning it."@en ;
    rdfs:domain <http://iflastandards.info/ns/fr/frbr/frbroo/F40> ;
    rdfs:isDefinedBy <http://iflastandards.info/ns/fr/frbr/frbroo/> ;
    rdfs:range <http://iflastandards.info/ns/fr/frbr/frbroo/F13> ;
    rdfs:subPropertyOf <http://www.cidoc-crm.org/cidoc-crm/P37_assigned> ;
    owl:inverseOf <http://iflastandards.info/ns/fr/frbr/frbroo/R46i> ;
    = <http://iflastandards.info/ns/fr/frbr/frbroo/R46_assigned_to> ;
    skos:definition "This property associates the instance of F13 Identifier assigned to an instance of E1 CRM Entity and the event of assigning it."@en .

<http://iflastandards.info/ns/fr/frbr/frbroo/R46i> a rdf:Property ;
    rdfs:label "was assigned by Identifier Assignment for Identifier"@en ;
    reg:name "wasAssignedByIdentifierAssignmentForIdentifier"@en ;
    reg:status <http://metadataregistry.org/uri/RegStatus/1001> ;
    rdfs:comment "Inverse of R46_assigned_to."@en ;
    rdfs:domain <http://iflastandards.info/ns/fr/frbr/frbroo/F13> ;
    rdfs:isDefinedBy <http://iflastandards.info/ns/fr/frbr/frbroo/> ;
    rdfs:range <http://iflastandards.info/ns/fr/frbr/frbroo/F40> ;
    rdfs:subPropertyOf <http://www.cidoc-crm.org/cidoc-crm/P37i_was_assigned_by> ;
    owl:inverseOf <http://iflastandards.info/ns/fr/frbr/frbroo/R46> ;
    = <http://iflastandards.info/ns/fr/frbr/frbroo/R46i_was_assigned_by> .

<http://iflastandards.info/ns/fr/frbr/frbroo/R47> a rdf:Property ;
    rdfs:label "used constituent"@en ;
    reg:name "usedConstituent"@en ;
    reg:status <http://metadataregistry.org/uri/RegStatus/1001> ;
    rdfs:comment "This property associates the event of assigning an instance of F13 Identifier to an entity with the elements that an actor used to compose that identifier."@en ;
    rdfs:domain <http://iflastandards.info/ns/fr/frbr/frbroo/F40> ;
    rdfs:isDefinedBy <http://iflastandards.info/ns/fr/frbr/frbroo/> ;
    rdfs:range <http://www.cidoc-crm.org/cidoc-crm/E90_Symbolic_Object> ;
    rdfs:subPropertyOf <http://www.cidoc-crm.org/cidoc-crm/P16_used_specific_object> ;
    owl:inverseOf <http://iflastandards.info/ns/fr/frbr/frbroo/R47i> ;
    = <http://iflastandards.info/ns/fr/frbr/frbroo/R47_used_constituent> ;
    skos:definition "This property associates the event of assigning an instance of F13 Identifier to an entity with the elements that an actor used to compose that identifier."@en .

<http://iflastandards.info/ns/fr/frbr/frbroo/R47i> a rdf:Property ;
    rdfs:label "was used in"@en ;
    reg:name "wasUsedIn"@en ;
    reg:status <http://metadataregistry.org/uri/RegStatus/1001> ;
    rdfs:comment "Inverse of R47_used_constituent."@en ;
    rdfs:domain <http://www.cidoc-crm.org/cidoc-crm/E90_Symbolic_Object> ;
    rdfs:isDefinedBy <http://iflastandards.info/ns/fr/frbr/frbroo/> ;
    rdfs:range <http://iflastandards.info/ns/fr/frbr/frbroo/F40> ;
    rdfs:subPropertyOf <http://www.cidoc-crm.org/cidoc-crm/P16i_was_used_for> ;
    owl:inverseOf <http://iflastandards.info/ns/fr/frbr/frbroo/R47> ;
    = <http://iflastandards.info/ns/fr/frbr/frbroo/R47i_was_used_in> .

<http://iflastandards.info/ns/fr/frbr/frbroo/R48> a rdf:Property ;
    rdfs:label "assigned to Expression by Representative Manifestation Assignment"@en ;
    reg:name "assignedToExpressionByRepresentativeManifestationAssignment"@en ;
    reg:status <http://metadataregistry.org/uri/RegStatus/1001> ;
    rdfs:comment "This property associates the event of assigning a representative instance of F3 Manifestation Product Type or F4 Manifestation Singleton with the expression to which it was assigned."@en ;
    rdfs:domain <http://iflastandards.info/ns/fr/frbr/frbroo/F41> ;
    rdfs:isDefinedBy <http://iflastandards.info/ns/fr/frbr/frbroo/> ;
    rdfs:range <http://iflastandards.info/ns/fr/frbr/frbroo/F2> ;
    rdfs:subPropertyOf <http://www.cidoc-crm.org/cidoc-crm/P140_assigned_attribute_to> ;
    owl:inverseOf <http://iflastandards.info/ns/fr/frbr/frbroo/R48i> ;
    = <http://iflastandards.info/ns/fr/frbr/frbroo/R48_assigned_to> ;
    skos:definition "This property associates the event of assigning a representative instance of F3 Manifestation Product Type or F4 Manifestation Singleton with the expression to which it was assigned."@en .

<http://iflastandards.info/ns/fr/frbr/frbroo/R48i> a rdf:Property ;
    rdfs:label "assigned"@en ;
    reg:name "assigned"@en ;
    reg:status <http://metadataregistry.org/uri/RegStatus/1001> ;
    rdfs:comment "Inverse of R48_assigned_to."@en ;
    rdfs:domain <http://iflastandards.info/ns/fr/frbr/frbroo/F2> ;
    rdfs:isDefinedBy <http://iflastandards.info/ns/fr/frbr/frbroo/> ;
    rdfs:range <http://iflastandards.info/ns/fr/frbr/frbroo/F41> ;
    rdfs:subPropertyOf <http://www.cidoc-crm.org/cidoc-crm/P140i_was_attributed_by> ;
    owl:inverseOf <http://iflastandards.info/ns/fr/frbr/frbroo/R48> ;
    = <http://iflastandards.info/ns/fr/frbr/frbroo/R48i_assigned> .

<http://iflastandards.info/ns/fr/frbr/frbroo/R49> a rdf:Property ;
    rdfs:label "assigned Manifestation Product Type from Representative Manifestation Assignment"@en ;
    reg:name "assignedManifestationProduceTypeFromRepresentativeManifestationAssignment"@en ;
    reg:status <http://metadataregistry.org/uri/RegStatus/1001> ;
    rdfs:comment "This property associates the event of assigning a representative instance of F3 Manifestation Product Type with the F3 Manifestation Product Type which has been assigned."@en ;
    rdfs:domain <http://iflastandards.info/ns/fr/frbr/frbroo/F41> ;
    rdfs:isDefinedBy <http://iflastandards.info/ns/fr/frbr/frbroo/> ;
    rdfs:range <http://iflastandards.info/ns/fr/frbr/frbroo/F3> ;
    rdfs:subPropertyOf <http://www.cidoc-crm.org/cidoc-crm/P141_assigned> ;
    owl:inverseOf <http://iflastandards.info/ns/fr/frbr/frbroo/R49i> ;
    = <http://iflastandards.info/ns/fr/frbr/frbroo/R49_assigned> ;
    skos:definition "This property associates the event of assigning a representative instance of F3 Manifestation Product Type with the F3 Manifestation Product Type which has been assigned."@en .

<http://iflastandards.info/ns/fr/frbr/frbroo/R49i> a rdf:Property ;
    rdfs:label "was assigned by Representative Manifestation Assignment for Manifestation Product Type"@en ;
    reg:name "wasAssignedByRepresentativeManifestationAssignmentForManifestationProductType"@en ;
    reg:status <http://metadataregistry.org/uri/RegStatus/1001> ;
    rdfs:comment "Inverse of R49_assigned."@en ;
    rdfs:domain <http://iflastandards.info/ns/fr/frbr/frbroo/F3> ;
    rdfs:isDefinedBy <http://iflastandards.info/ns/fr/frbr/frbroo/> ;
    rdfs:range <http://iflastandards.info/ns/fr/frbr/frbroo/F41> ;
    rdfs:subPropertyOf <http://www.cidoc-crm.org/cidoc-crm/P141i_was_assigned_by> ;
    owl:inverseOf <http://iflastandards.info/ns/fr/frbr/frbroo/R49> ;
    = <http://iflastandards.info/ns/fr/frbr/frbroo/R49i_was_assigned_by> .

<http://iflastandards.info/ns/fr/frbr/frbroo/R5> a rdf:Property ;
    rdfs:label "has component"@en ;
    reg:name "hasComponent"@en ;
    reg:status <http://metadataregistry.org/uri/RegStatus/1001> ;
    rdfs:comment "This property associates an F2 Expression X with a structural component Y that conveys in itself the complete concept of a work that is member of (R10) the overall work realized by X. It does not cover the relationship that exists between pre-existing expressions that are re-used in a new, larger expression and that new, larger expression. Such a relationship is modelled by R14 incorporates."@en ;
    rdfs:domain <http://iflastandards.info/ns/fr/frbr/frbroo/F2> ;
    rdfs:isDefinedBy <http://iflastandards.info/ns/fr/frbr/frbroo/> ;
    rdfs:range <http://iflastandards.info/ns/fr/frbr/frbroo/F22> ;
    rdfs:subPropertyOf <http://www.cidoc-crm.org/cidoc-crm/P148_has_component> ;
    owl:inverseOf <http://iflastandards.info/ns/fr/frbr/frbroo/R5i> ;
    = <http://iflastandards.info/ns/fr/frbr/frbroo/R5_has_component> ;
    skos:definition "This property associates an F2 Expression X with a structural component Y that conveys in itself the complete concept of a work that is member of (R10) the overall work realized by X."@en ;
    skos:scopeNote "It does not cover the relationship that exists between pre-existing expressions that are re-used in a new, larger expression and that new, larger expression. Such a relationship is modelled by R14 incorporates."@en .

<http://iflastandards.info/ns/fr/frbr/frbroo/R50> a rdf:Property ;
    rdfs:label "assigned to Complex Work by Representative Expression Assignment"@en ;
    reg:name "assignedToComplexWorkByRepresentativeExpressionAssignment"@en ;
    reg:status <http://metadataregistry.org/uri/RegStatus/1001> ;
    rdfs:comment "This property associates the event of assigning a representative instance of F2 Expression with the instance of F15 Complex Work to which it was assigned."@en ;
    rdfs:domain <http://iflastandards.info/ns/fr/frbr/frbroo/F42> ;
    rdfs:isDefinedBy <http://iflastandards.info/ns/fr/frbr/frbroo/> ;
    rdfs:range <http://iflastandards.info/ns/fr/frbr/frbroo/F15> ;
    rdfs:subPropertyOf <http://www.cidoc-crm.org/cidoc-crm/P140_assigned_attribute_to> ;
    owl:inverseOf <http://iflastandards.info/ns/fr/frbr/frbroo/R50i> ;
    = <http://iflastandards.info/ns/fr/frbr/frbroo/R50_assigned_to> ;
    skos:definition "This property associates the event of assigning a representative instance of F2 Expression with the instance of F15 Complex Work to which it was assigned."@en .

<http://iflastandards.info/ns/fr/frbr/frbroo/R50i> a rdf:Property ;
    rdfs:label "was assigned by Representative Expression Assignment for Complex Work"@en ;
    reg:name "wasAssignedBy RepresentativeExpressionAssignmentForComplexWork"@en ;
    reg:status <http://metadataregistry.org/uri/RegStatus/1001> ;
    rdfs:comment "Inverse of R50_assigned_to."@en ;
    rdfs:domain <http://iflastandards.info/ns/fr/frbr/frbroo/F15> ;
    rdfs:isDefinedBy <http://iflastandards.info/ns/fr/frbr/frbroo/> ;
    rdfs:range <http://iflastandards.info/ns/fr/frbr/frbroo/F42> ;
    rdfs:subPropertyOf <http://www.cidoc-crm.org/cidoc-crm/P140i_was_attributed_by> ;
    owl:inverseOf <http://iflastandards.info/ns/fr/frbr/frbroo/R50> ;
    = <http://iflastandards.info/ns/fr/frbr/frbroo/R50i_was_assigned_by> .

<http://iflastandards.info/ns/fr/frbr/frbroo/R51> a rdf:Property ;
    rdfs:label "assigned Expression from Representative Expression Assignment"@en ;
    reg:name "assignedExpressionFromRepresentativeExpressionAssignment"@en ;
    reg:status <http://metadataregistry.org/uri/RegStatus/1001> ;
    rdfs:comment "This property associates the event of assigning a representative instance of F2 Expression with the F2 Expression which has been assigned."@en ;
    rdfs:domain <http://iflastandards.info/ns/fr/frbr/frbroo/F42> ;
    rdfs:isDefinedBy <http://iflastandards.info/ns/fr/frbr/frbroo/> ;
    rdfs:range <http://iflastandards.info/ns/fr/frbr/frbroo/F2> ;
    rdfs:subPropertyOf <http://www.cidoc-crm.org/cidoc-crm/P141_assigned> ;
    owl:inverseOf <http://iflastandards.info/ns/fr/frbr/frbroo/R51i> ;
    = <http://iflastandards.info/ns/fr/frbr/frbroo/R51_assigned> ;
    skos:definition "This property associates the event of assigning a representative instance of F2 Expression with the F2 Expression which has been assigned."@en .

<http://iflastandards.info/ns/fr/frbr/frbroo/R51i> a rdf:Property ;
    rdfs:label "was assigned by Representative Expression Assignment for Expression"@en ;
    reg:name "wasAssignedByRepresentativeExpressionAssignmentForExpression"@en ;
    reg:status <http://metadataregistry.org/uri/RegStatus/1001> ;
    rdfs:comment "Inverse of R51_assigned."@en ;
    rdfs:domain <http://iflastandards.info/ns/fr/frbr/frbroo/F2> ;
    rdfs:isDefinedBy <http://iflastandards.info/ns/fr/frbr/frbroo/> ;
    rdfs:range <http://iflastandards.info/ns/fr/frbr/frbroo/F42> ;
    rdfs:subPropertyOf <http://www.cidoc-crm.org/cidoc-crm/P141i_was_assigned_by> ;
    owl:inverseOf <http://iflastandards.info/ns/fr/frbr/frbroo/R51> ;
    = <http://iflastandards.info/ns/fr/frbr/frbroo/R51i_was_assigned_by> .

<http://iflastandards.info/ns/fr/frbr/frbroo/R52> a rdf:Property ;
    rdfs:label "used rule"@en ;
    reg:name "usedRule"@en ;
    reg:status <http://metadataregistry.org/uri/RegStatus/1001> ;
    rdfs:comment "This property associates the event of assigning an instance of F13 Identifier with the instructions followed by an actor, such as a Bibliographic Agency, in creating that identifier."@en ;
    rdfs:domain <http://iflastandards.info/ns/fr/frbr/frbroo/F40> ;
    rdfs:isDefinedBy <http://iflastandards.info/ns/fr/frbr/frbroo/> ;
    rdfs:range <http://iflastandards.info/ns/fr/frbr/frbroo/F43> ;
    rdfs:subPropertyOf <http://www.cidoc-crm.org/cidoc-crm/P33_used_specific_technique> ;
    owl:inverseOf <http://iflastandards.info/ns/fr/frbr/frbroo/R52i> ;
    = <http://iflastandards.info/ns/fr/frbr/frbroo/R52_used_rule> ;
    skos:definition "This property associates the event of assigning an instance of F13 Identifier with the instructions followed by an actor, such as a Bibliographic Agency, in creating that identifier."@en .

<http://iflastandards.info/ns/fr/frbr/frbroo/R52i> a rdf:Property ;
    rdfs:label "was the rule used in"@en ;
    reg:name "wasTheRuleUsedIn"@en ;
    reg:status <http://metadataregistry.org/uri/RegStatus/1001> ;
    rdfs:comment "Inverse of R52_used_rule."@en ;
    rdfs:domain <http://iflastandards.info/ns/fr/frbr/frbroo/F43> ;
    rdfs:isDefinedBy <http://iflastandards.info/ns/fr/frbr/frbroo/> ;
    rdfs:range <http://iflastandards.info/ns/fr/frbr/frbroo/F40> ;
    rdfs:subPropertyOf <http://www.cidoc-crm.org/cidoc-crm/P33i_was_used_in> ;
    owl:inverseOf <http://iflastandards.info/ns/fr/frbr/frbroo/R52> ;
    = <http://iflastandards.info/ns/fr/frbr/frbroo/R52i_was_the_rule_used_by> .

<http://iflastandards.info/ns/fr/frbr/frbroo/R53> a rdf:Property ;
    rdfs:label "assigned Manifestation Singleton from Representative Manifestation Assignment"@en ;
    reg:name "assignedManifestationSingletonFromRepresentativeManifestationAssignment"@en ;
    reg:status <http://metadataregistry.org/uri/RegStatus/1001> ;
    rdfs:comment "This property associates the event of assigning a representative instance of F4 Manifestation Singleton with the F4 Manifestation Singleton which has been assigned."@en ;
    rdfs:domain <http://iflastandards.info/ns/fr/frbr/frbroo/F41> ;
    rdfs:isDefinedBy <http://iflastandards.info/ns/fr/frbr/frbroo/> ;
    rdfs:range <http://iflastandards.info/ns/fr/frbr/frbroo/F4> ;
    rdfs:subPropertyOf <http://www.cidoc-crm.org/cidoc-crm/P141_assigned> ;
    owl:inverseOf <http://iflastandards.info/ns/fr/frbr/frbroo/R53i> ;
    = <http://iflastandards.info/ns/fr/frbr/frbroo/R53_assigned> ;
    skos:definition "This property associates the event of assigning a representative instance of F4 Manifestation Singleton with the F4 Manifestation Singleton which has been assigned."@en .

<http://iflastandards.info/ns/fr/frbr/frbroo/R53i> a rdf:Property ;
    rdfs:label "was assigned by Representative Manifestation Assignment for Manifestation Singleton"@en ;
    reg:name "wasAssignedByRepresentativeManifestationAssignmentForManifestationSingleton"@en ;
    reg:status <http://metadataregistry.org/uri/RegStatus/1001> ;
    rdfs:comment "Inverse of R53_assigned."@en ;
    rdfs:domain <http://iflastandards.info/ns/fr/frbr/frbroo/F4> ;
    rdfs:isDefinedBy <http://iflastandards.info/ns/fr/frbr/frbroo/> ;
    rdfs:range <http://iflastandards.info/ns/fr/frbr/frbroo/F41> ;
    rdfs:subPropertyOf <http://www.cidoc-crm.org/cidoc-crm/P141i_was_assigned_by> ;
    owl:inverseOf <http://iflastandards.info/ns/fr/frbr/frbroo/R53> ;
    = <http://iflastandards.info/ns/fr/frbr/frbroo/R53i_was_assigned_by> .

<http://iflastandards.info/ns/fr/frbr/frbroo/R54> a rdf:Property ;
    rdfs:label "has nomen language"@en ;
    reg:name "hasNomenLanguage"@en ;
    reg:status <http://metadataregistry.org/uri/RegStatus/1001> ;
    rdfs:comment "This property associates an instance of F35 Nomen Use Statement with an instance of E56 Language which is a target language for the associated nomen use."@en ;
    rdfs:domain <http://iflastandards.info/ns/fr/frbr/frbroo/F35> ;
    rdfs:isDefinedBy <http://iflastandards.info/ns/fr/frbr/frbroo/> ;
    rdfs:range <http://www.cidoc-crm.org/cidoc-crm/E56_Language> ;
    rdfs:subPropertyOf <http://www.cidoc-crm.org/cidoc-crm/P67_refers_to> ;
    owl:inverseOf <http://iflastandards.info/ns/fr/frbr/frbroo/R54i> ;
    = <http://iflastandards.info/ns/fr/frbr/frbroo/R54_has_nomen_language> ;
    skos:definition "This property associates an instance of F35 Nomen Use Statement with an instance of E56 Language which is a target language for the associated nomen use."@en .

<http://iflastandards.info/ns/fr/frbr/frbroo/R54i> a rdf:Property ;
    rdfs:label "is language of nomen in"@en ;
    reg:name "isLanguageOfNomenIn"@en ;
    reg:status <http://metadataregistry.org/uri/RegStatus/1001> ;
    rdfs:comment "Inverse of R54_has_nomen_language."@en ;
    rdfs:domain <http://www.cidoc-crm.org/cidoc-crm/E56_Language> ;
    rdfs:isDefinedBy <http://iflastandards.info/ns/fr/frbr/frbroo/> ;
    rdfs:range <http://iflastandards.info/ns/fr/frbr/frbroo/F35> ;
    rdfs:subPropertyOf <http://www.cidoc-crm.org/cidoc-crm/P67i_is_referred_to_by> ;
    owl:inverseOf <http://iflastandards.info/ns/fr/frbr/frbroo/R54> ;
    = <http://iflastandards.info/ns/fr/frbr/frbroo/R54i_is_language_of_nomen_in> .

<http://iflastandards.info/ns/fr/frbr/frbroo/R55> a rdf:Property ;
    rdfs:label "has nomen form"@en ;
    reg:name "hasNomenForm"@en ;
    reg:status <http://metadataregistry.org/uri/RegStatus/1001> ;
    rdfs:comment "This property associates an instance of F35 Nomen Use Statement with the instance of E55 Type that characterizes the Nomen referred to in the Nomen Use Statement, such as abbreviation, full name etc. In the case of abbreviations, the source of this form may or may not be explicitly mentioned."@en ;
    rdfs:domain <http://iflastandards.info/ns/fr/frbr/frbroo/F35> ;
    rdfs:isDefinedBy <http://iflastandards.info/ns/fr/frbr/frbroo/> ;
    rdfs:range <http://www.cidoc-crm.org/cidoc-crm/E55_Type> ;
    rdfs:subPropertyOf <http://www.cidoc-crm.org/cidoc-crm/P67_refers_to> ;
    owl:inverseOf <http://iflastandards.info/ns/fr/frbr/frbroo/R55i> ;
    = <http://iflastandards.info/ns/fr/frbr/frbroo/R55_has_nomen_form> ;
    skos:definition "This property associates an instance of F35 Nomen Use Statement with the instance of E55 Type that characterizes the Nomen referred to in the Nomen Use Statement, such as abbreviation, full name etc. In the case of abbreviations, the source of this form may or may not be explicitly mentioned."@en .

<http://iflastandards.info/ns/fr/frbr/frbroo/R55i> a rdf:Property ;
    rdfs:label "is nomen form in"@en ;
    reg:name "isNomenFormIn"@en ;
    reg:status <http://metadataregistry.org/uri/RegStatus/1001> ;
    rdfs:comment "Inverse of R55_has_nomen_form."@en ;
    rdfs:domain <http://www.cidoc-crm.org/cidoc-crm/E55_Type> ;
    rdfs:isDefinedBy <http://iflastandards.info/ns/fr/frbr/frbroo/> ;
    rdfs:range <http://iflastandards.info/ns/fr/frbr/frbroo/F35> ;
    rdfs:subPropertyOf <http://www.cidoc-crm.org/cidoc-crm/P67i_is_referred_to_by> ;
    owl:inverseOf <http://iflastandards.info/ns/fr/frbr/frbroo/R55> ;
    = <http://iflastandards.info/ns/fr/frbr/frbroo/R55i_is_nomen_form_in> .

<http://iflastandards.info/ns/fr/frbr/frbroo/R56> a rdf:Property ;
    rdfs:label "has related use"@en ;
    reg:name "hasRelatedUse"@en ;
    reg:status <http://metadataregistry.org/uri/RegStatus/1001> ;
    rdfs:comment "This property associates an instance of F35 Nomen Use Statement with another instance of F35 Nomen Use Statement which has a related use in some context, such as alternative, lexical variant, replacing former use etc. The property R56.1 allows for specifying the particular kind of the nomen use statement relationship."@en ;
    rdfs:domain <http://iflastandards.info/ns/fr/frbr/frbroo/F35> ;
    rdfs:isDefinedBy <http://iflastandards.info/ns/fr/frbr/frbroo/> ;
    rdfs:range <http://iflastandards.info/ns/fr/frbr/frbroo/F35> ;
    rdfs:subPropertyOf <http://www.cidoc-crm.org/cidoc-crm/P69_has_association_with> ;
    owl:inverseOf <http://iflastandards.info/ns/fr/frbr/frbroo/R56i> ;
    = <http://iflastandards.info/ns/fr/frbr/frbroo/R56_has_related_use> ;
    skos:definition "This property associates an instance of F35 Nomen Use Statement with another instance of F35 Nomen Use Statement which has a related use in some context, such as alternative, lexical variant, replacing former use etc."@en ;
    skos:scopeNote "The property R56.1 allows for specifying the particular kind of the nomen use statement relationship."@en .

<http://iflastandards.info/ns/fr/frbr/frbroo/R56i> a rdf:Property ;
    rdfs:label "is related use for"@en ;
    reg:name "isRelatedUseFor"@en ;
    reg:status <http://metadataregistry.org/uri/RegStatus/1001> ;
    rdfs:comment "Inverse of R56_has_related_use."@en ;
    rdfs:domain <http://iflastandards.info/ns/fr/frbr/frbroo/F35> ;
    rdfs:isDefinedBy <http://iflastandards.info/ns/fr/frbr/frbroo/> ;
    rdfs:range <http://iflastandards.info/ns/fr/frbr/frbroo/F35> ;
    rdfs:subPropertyOf <http://www.cidoc-crm.org/cidoc-crm/P69i_is_associated_with> ;
    owl:inverseOf <http://iflastandards.info/ns/fr/frbr/frbroo/R56> ;
    = <http://iflastandards.info/ns/fr/frbr/frbroo/R56i_is_related_use_for> .

<http://iflastandards.info/ns/fr/frbr/frbroo/R57> a rdf:Property ;
    rdfs:label "is based on"@en ;
    reg:name "isBasedOn"@en ;
    reg:status <http://metadataregistry.org/uri/RegStatus/1001> ;
    rdfs:comment "This property associates an instance of F38 Character with an instance of E39 Actor that the character is motivated by or is intended to represent. An instance of F38 Character may be based on a combination of features taken from several actors."@en ;
    rdfs:domain <http://iflastandards.info/ns/fr/frbr/frbroo/F38> ;
    rdfs:isDefinedBy <http://iflastandards.info/ns/fr/frbr/frbroo/> ;
    rdfs:range <http://www.cidoc-crm.org/cidoc-crm/E39_Actor> ;
    owl:inverseOf <http://iflastandards.info/ns/fr/frbr/frbroo/R57i> ;
    = <http://iflastandards.info/ns/fr/frbr/frbroo/R57_is_based_on> ;
    skos:definition "This property associates an instance of F38 Character with an instance of E39 Actor that the character is motivated by or is intended to represent."@en ;
    skos:scopeNote "An instance of F38 Character may be based on a combination of features taken from several actors."@en .

<http://iflastandards.info/ns/fr/frbr/frbroo/R57i> a rdf:Property ;
    rdfs:label "is basis for"@en ;
    reg:name "isBasisFor"@en ;
    reg:status <http://metadataregistry.org/uri/RegStatus/1001> ;
    rdfs:comment "Inverse of R57_is_based_on."@en ;
    rdfs:domain <http://www.cidoc-crm.org/cidoc-crm/E39_Actor> ;
    rdfs:isDefinedBy <http://iflastandards.info/ns/fr/frbr/frbroo/> ;
    rdfs:range <http://iflastandards.info/ns/fr/frbr/frbroo/F38> ;
    owl:inverseOf <http://iflastandards.info/ns/fr/frbr/frbroo/R57> ;
    = <http://iflastandards.info/ns/fr/frbr/frbroo/R57i_is_basis_for> .

<http://iflastandards.info/ns/fr/frbr/frbroo/R58> a rdf:Property ;
    rdfs:label "has fictional member"@en ;
    reg:name "hasFictionalMember"@en ;
    reg:status <http://metadataregistry.org/uri/RegStatus/1001> ;
    rdfs:comment "This property associates an instance of F38 Character representing a group with another instance of F38 Character that is presented in relevant fiction as a member of the fictional group."@en ;
    rdfs:domain <http://iflastandards.info/ns/fr/frbr/frbroo/F38> ;
    rdfs:isDefinedBy <http://iflastandards.info/ns/fr/frbr/frbroo/> ;
    rdfs:range <http://iflastandards.info/ns/fr/frbr/frbroo/F38> ;
    owl:inverseOf <http://iflastandards.info/ns/fr/frbr/frbroo/R58i> ;
    = <http://iflastandards.info/ns/fr/frbr/frbroo/R58_has_fictional_member> ;
    skos:definition "This property associates an instance of F38 Character representing a group with another instance of F38 Character that is presented in relevant fiction as a member of the fictional group."@en .

<http://iflastandards.info/ns/fr/frbr/frbroo/R58i> a rdf:Property ;
    rdfs:label "is fictional member of"@en ;
    reg:name "isFictionalMemberOf"@en ;
    reg:status <http://metadataregistry.org/uri/RegStatus/1001> ;
    rdfs:comment "Inverse of R58_has_fictional_member."@en ;
    rdfs:domain <http://iflastandards.info/ns/fr/frbr/frbroo/F38> ;
    rdfs:isDefinedBy <http://iflastandards.info/ns/fr/frbr/frbroo/> ;
    rdfs:range <http://iflastandards.info/ns/fr/frbr/frbroo/F38> ;
    owl:inverseOf <http://iflastandards.info/ns/fr/frbr/frbroo/R58> ;
    = <http://iflastandards.info/ns/fr/frbr/frbroo/R58i_is_fictional_member_of> .

<http://iflastandards.info/ns/fr/frbr/frbroo/R59> a rdf:Property ;
    rdfs:label "had typical subject"@en ;
    reg:name "hadTypicalSubject"@en ;
    reg:status <http://metadataregistry.org/uri/RegStatus/1001> ;
    rdfs:comment "This property associates an instance of F51 Pursuit with the instance of E1 CRM Entity that is the typical subject of the associated activity, such as an area of expertise in which the actor is engaged or was engaged."@en ;
    rdfs:domain <http://iflastandards.info/ns/fr/frbr/frbroo/F51> ;
    rdfs:isDefinedBy <http://iflastandards.info/ns/fr/frbr/frbroo/> ;
    rdfs:range <http://www.cidoc-crm.org/cidoc-crm/E1_CRM_Entity> ;
    owl:inverseOf <http://iflastandards.info/ns/fr/frbr/frbroo/R59i> ;
    = <http://iflastandards.info/ns/fr/frbr/frbroo/R59_had_typical_subject> ;
    skos:definition "This property associates an instance of F51 Pursuit with the instance of E1 CRM Entity that is the typical subject of the associated activity, such as an area of expertise in which the actor is engaged or was engaged."@en .

<http://iflastandards.info/ns/fr/frbr/frbroo/R59i> a rdf:Property ;
    rdfs:label "was typical subject of"@en ;
    reg:name "wasTypicalSubjectOf"@en ;
    reg:status <http://metadataregistry.org/uri/RegStatus/1001> ;
    rdfs:comment "Inverse of R59_had_typical_subject."@en ;
    rdfs:domain <http://www.cidoc-crm.org/cidoc-crm/E1_CRM_Entity> ;
    rdfs:isDefinedBy <http://iflastandards.info/ns/fr/frbr/frbroo/> ;
    rdfs:range <http://iflastandards.info/ns/fr/frbr/frbroo/F51> ;
    owl:inverseOf <http://iflastandards.info/ns/fr/frbr/frbroo/R59> ;
    = <http://iflastandards.info/ns/fr/frbr/frbroo/R59i_was_typical_subject_of> .

<http://iflastandards.info/ns/fr/frbr/frbroo/R5i> a rdf:Property ;
    rdfs:label "is component of"@en ;
    reg:name "isComponentOf"@en ;
    reg:status <http://metadataregistry.org/uri/RegStatus/1001> ;
    rdfs:comment "Inverse of R5_has_component."@en ;
    rdfs:domain <http://iflastandards.info/ns/fr/frbr/frbroo/F22> ;
    rdfs:isDefinedBy <http://iflastandards.info/ns/fr/frbr/frbroo/> ;
    rdfs:range <http://iflastandards.info/ns/fr/frbr/frbroo/F2> ;
    rdfs:subPropertyOf <http://www.cidoc-crm.org/cidoc-crm/P148i_is_component_of> ;
    owl:inverseOf <http://iflastandards.info/ns/fr/frbr/frbroo/R5> ;
    = <http://iflastandards.info/ns/fr/frbr/frbroo/R5i_is_component_of> .

<http://iflastandards.info/ns/fr/frbr/frbroo/R6> a rdf:Property ;
    rdfs:label "carries"@en ;
    reg:name "carries"@en ;
    reg:status <http://metadataregistry.org/uri/RegStatus/1001> ;
    rdfs:comment "This property associates an instance of F5 Item with the unique instance of F24 Publication Expression it carries."@en ;
    rdfs:domain <http://iflastandards.info/ns/fr/frbr/frbroo/F5> ;
    rdfs:isDefinedBy <http://iflastandards.info/ns/fr/frbr/frbroo/> ;
    rdfs:range <http://iflastandards.info/ns/fr/frbr/frbroo/F24> ;
    rdfs:subPropertyOf <http://www.cidoc-crm.org/cidoc-crm/P128_carries> ;
    owl:inverseOf <http://iflastandards.info/ns/fr/frbr/frbroo/R6i> ;
    = <http://iflastandards.info/ns/fr/frbr/frbroo/R6_carries> ;
    skos:definition "This property associates an instance of F5 Item with the unique instance of F24 Publication Expression it carries."@en .

<http://iflastandards.info/ns/fr/frbr/frbroo/R60> a rdf:Property ;
    rdfs:label "used to use language"@en ;
    reg:name "usedToUseLanguage"@en ;
    reg:status <http://metadataregistry.org/uri/RegStatus/1001> ;
    rdfs:comment "This property associates an instance of F51 Pursuit with the instance of E56 Language that was characteristically used for the products of the associated activity. The property R60.1 has type of use allows for specifying a particular form of use."@en ;
    rdfs:domain <http://iflastandards.info/ns/fr/frbr/frbroo/F51> ;
    rdfs:isDefinedBy <http://iflastandards.info/ns/fr/frbr/frbroo/> ;
    rdfs:range <http://www.cidoc-crm.org/cidoc-crm/E56_Language> ;
    owl:inverseOf <http://iflastandards.info/ns/fr/frbr/frbroo/R60i> ;
    = <http://iflastandards.info/ns/fr/frbr/frbroo/R60_used_to_use_language> ;
    skos:definition "This property associates an instance of F51 Pursuit with the instance of E56 Language that was characteristically used for the products of the associated activity."@en ;
    skos:scopeNote "The property R60.1 has type of use allows for specifying a particular form of use."@en .

<http://iflastandards.info/ns/fr/frbr/frbroo/R60i> a rdf:Property ;
    rdfs:label "was language used by"@en ;
    reg:name "wasLanguageUsedBy"@en ;
    reg:status <http://metadataregistry.org/uri/RegStatus/1001> ;
    rdfs:comment "Inverse of R60_used_to_use_language."@en ;
    rdfs:domain <http://www.cidoc-crm.org/cidoc-crm/E56_Language> ;
    rdfs:isDefinedBy <http://iflastandards.info/ns/fr/frbr/frbroo/> ;
    rdfs:range <http://iflastandards.info/ns/fr/frbr/frbroo/F51> ;
    owl:inverseOf <http://iflastandards.info/ns/fr/frbr/frbroo/R60> ;
    = <http://iflastandards.info/ns/fr/frbr/frbroo/R60i_was_language_used_by> .

<http://iflastandards.info/ns/fr/frbr/frbroo/R61> a rdf:Property ;
    rdfs:label "occured in kind of context"@en ;
    reg:name "occuredInKindOfContext"@en ;
    reg:status <http://metadataregistry.org/uri/RegStatus/1001> ;
    rdfs:comment "This property associates an instance of F52 Name Use Activity with the instance of E55 Type that characterizes the kind of role or context within which the associated name was used."@en ;
    rdfs:domain <http://iflastandards.info/ns/fr/frbr/frbroo/F52> ;
    rdfs:isDefinedBy <http://iflastandards.info/ns/fr/frbr/frbroo/> ;
    rdfs:range <http://www.cidoc-crm.org/cidoc-crm/E55_Type> ;
    owl:inverseOf <http://iflastandards.info/ns/fr/frbr/frbroo/R61i> ;
    = <http://iflastandards.info/ns/fr/frbr/frbroo/R61_occured_in_kind_of_context> ;
    skos:definition "This property associates an instance of F52 Name Use Activity with the instance of E55 Type that characterizes the kind of role or context within which the associated name was used."@en .

<http://iflastandards.info/ns/fr/frbr/frbroo/R61i> a rdf:Property ;
    rdfs:label "was kind of context for"@en ;
    reg:name "wasKindOfContextFor"@en ;
    reg:status <http://metadataregistry.org/uri/RegStatus/1001> ;
    rdfs:comment "Inverse of R61_occured_in_kind_of_context."@en ;
    rdfs:domain <http://www.cidoc-crm.org/cidoc-crm/E55_Type> ;
    rdfs:isDefinedBy <http://iflastandards.info/ns/fr/frbr/frbroo/> ;
    rdfs:range <http://iflastandards.info/ns/fr/frbr/frbroo/F52> ;
    owl:inverseOf <http://iflastandards.info/ns/fr/frbr/frbroo/R61> ;
    = <http://iflastandards.info/ns/fr/frbr/frbroo/R61i_was_kind_of_context_for> .

<http://iflastandards.info/ns/fr/frbr/frbroo/R62> a rdf:Property ;
    rdfs:label "was used for membership in"@en ;
    reg:name "wasUsedForMembershipIn"@en ;
    reg:status <http://metadataregistry.org/uri/RegStatus/1001> ;
    rdfs:comment "This property associates an instance of F52 Name Use Activity with the instance of E74 Group that characterizes the context within which the associated name was used as the membership in that group."@en ;
    rdfs:domain <http://iflastandards.info/ns/fr/frbr/frbroo/F52> ;
    rdfs:isDefinedBy <http://iflastandards.info/ns/fr/frbr/frbroo/> ;
    rdfs:range <http://www.cidoc-crm.org/cidoc-crm/E74_Group> ;
    owl:inverseOf <http://iflastandards.info/ns/fr/frbr/frbroo/R62i> ;
    = <http://iflastandards.info/ns/fr/frbr/frbroo/R62_was_used_for_membership_in> ;
    skos:definition "This property associates an instance of F52 Name Use Activity with the instance of E74 Group that characterizes the context within which the associated name was used as the membership in that group."@en .

<http://iflastandards.info/ns/fr/frbr/frbroo/R62i> a rdf:Property ;
    rdfs:label "was context for"@en ;
    reg:name "wasContextFor"@en ;
    reg:status <http://metadataregistry.org/uri/RegStatus/1001> ;
    rdfs:comment "Inverse of R62_was_used_for_membership_in."@en ;
    rdfs:domain <http://www.cidoc-crm.org/cidoc-crm/E74_Group> ;
    rdfs:isDefinedBy <http://iflastandards.info/ns/fr/frbr/frbroo/> ;
    rdfs:range <http://iflastandards.info/ns/fr/frbr/frbroo/F52> ;
    owl:inverseOf <http://iflastandards.info/ns/fr/frbr/frbroo/R62> ;
    = <http://iflastandards.info/ns/fr/frbr/frbroo/R62i_was_context_for> .

<http://iflastandards.info/ns/fr/frbr/frbroo/R63> a rdf:Property ;
    rdfs:label "named"@en ;
    reg:name "named"@en ;
    reg:status <http://metadataregistry.org/uri/RegStatus/1001> ;
    rdfs:comment "This property associates an instance of F52 Name Use Activity with the instance of E1 CRM Entity that the associated name was used for."@en ;
    rdfs:domain <http://iflastandards.info/ns/fr/frbr/frbroo/F52> ;
    rdfs:isDefinedBy <http://iflastandards.info/ns/fr/frbr/frbroo/> ;
    rdfs:range <http://www.cidoc-crm.org/cidoc-crm/E1_CRM_Entity> ;
    rdfs:subPropertyOf <http://www.cidoc-crm.org/cidoc-crm/P140_assigned_attribute_to> ;
    owl:inverseOf <http://iflastandards.info/ns/fr/frbr/frbroo/R63i> ;
    = <http://iflastandards.info/ns/fr/frbr/frbroo/R63_named> ;
    skos:definition "This property associates an instance of F52 Name Use Activity with the instance of E1 CRM Entity that the associated name was used for."@en .

<http://iflastandards.info/ns/fr/frbr/frbroo/R63i> a rdf:Property ;
    rdfs:label "was named by"@en ;
    reg:name "wasNamedBy"@en ;
    reg:status <http://metadataregistry.org/uri/RegStatus/1001> ;
    rdfs:comment "Inverse of R63_named."@en ;
    rdfs:domain <http://www.cidoc-crm.org/cidoc-crm/E1_CRM_Entity> ;
    rdfs:isDefinedBy <http://iflastandards.info/ns/fr/frbr/frbroo/> ;
    rdfs:range <http://iflastandards.info/ns/fr/frbr/frbroo/F52> ;
    rdfs:subPropertyOf <http://www.cidoc-crm.org/cidoc-crm/P140i_was_attributed_by> ;
    owl:inverseOf <http://iflastandards.info/ns/fr/frbr/frbroo/R63> ;
    = <http://iflastandards.info/ns/fr/frbr/frbroo/R63i_was_named_by> .

<http://iflastandards.info/ns/fr/frbr/frbroo/R64> a rdf:Property ;
    rdfs:label "used name"@en ;
    reg:name "usedName"@en ;
    reg:status <http://metadataregistry.org/uri/RegStatus/1001> ;
    rdfs:comment "This property associates an instance of F52 Name Use Activity with the instance of E41 Appellation that was used for the associated entity."@en ;
    rdfs:domain <http://iflastandards.info/ns/fr/frbr/frbroo/F52> ;
    rdfs:isDefinedBy <http://iflastandards.info/ns/fr/frbr/frbroo/> ;
    rdfs:range <http://www.cidoc-crm.org/cidoc-crm/E41_Appellation> ;
    rdfs:subPropertyOf <http://www.cidoc-crm.org/cidoc-crm/P141_assigned> ;
    owl:inverseOf <http://iflastandards.info/ns/fr/frbr/frbroo/R64i> ;
    = <http://iflastandards.info/ns/fr/frbr/frbroo/R64_used_name> ;
    skos:definition "This property associates an instance of F52 Name Use Activity with the instance of E41 Appellation that was used for the associated entity."@en .

<http://iflastandards.info/ns/fr/frbr/frbroo/R64i> a rdf:Property ;
    rdfs:label "was name used by"@en ;
    reg:name "wasNameUsedBy"@en ;
    reg:status <http://metadataregistry.org/uri/RegStatus/1001> ;
    rdfs:comment "Inverse of R64_used_name."@en ;
    rdfs:domain <http://www.cidoc-crm.org/cidoc-crm/E41_Appellation> ;
    rdfs:isDefinedBy <http://iflastandards.info/ns/fr/frbr/frbroo/> ;
    rdfs:range <http://iflastandards.info/ns/fr/frbr/frbroo/F52> ;
    rdfs:subPropertyOf <http://www.cidoc-crm.org/cidoc-crm/P141i_was_assigned_by> ;
    owl:inverseOf <http://iflastandards.info/ns/fr/frbr/frbroo/R64> ;
    = <http://iflastandards.info/ns/fr/frbr/frbroo/R64i_was_name_used_by> .

<http://iflastandards.info/ns/fr/frbr/frbroo/R6i> a rdf:Property ;
    rdfs:label "is carried by"@en ;
    reg:name "isCarriedBy"@en ;
    reg:status <http://metadataregistry.org/uri/RegStatus/1001> ;
    rdfs:comment "Inverse of R6_carries."@en ;
    rdfs:domain <http://iflastandards.info/ns/fr/frbr/frbroo/F24> ;
    rdfs:isDefinedBy <http://iflastandards.info/ns/fr/frbr/frbroo/> ;
    rdfs:range <http://iflastandards.info/ns/fr/frbr/frbroo/F5> ;
    rdfs:subPropertyOf <http://www.cidoc-crm.org/cidoc-crm/P128i_is_carried_by> ;
    owl:inverseOf <http://iflastandards.info/ns/fr/frbr/frbroo/R6> ;
    = <http://iflastandards.info/ns/fr/frbr/frbroo/R6i_is_carried_by> .

<http://iflastandards.info/ns/fr/frbr/frbroo/R7> a rdf:Property ;
    rdfs:label "is example of"@en ;
    reg:name "isExampleOf"@en ;
    reg:status <http://metadataregistry.org/uri/RegStatus/1001> ;
    rdfs:comment "This property associates a publication with one of its exemplars. It is a shortcut of the more developed path: F5 Item R28B was produced by F32 Carrier Production R26 produced things of type (was produced by): F3 Manifestation Product Type."@en ;
    rdfs:domain <http://iflastandards.info/ns/fr/frbr/frbroo/F5> ;
    rdfs:isDefinedBy <http://iflastandards.info/ns/fr/frbr/frbroo/> ;
    rdfs:range <http://iflastandards.info/ns/fr/frbr/frbroo/F3> ;
    rdfs:subPropertyOf <http://www.cidoc-crm.org/cidoc-crm/P2_has_type> ;
    owl:inverseOf <http://iflastandards.info/ns/fr/frbr/frbroo/R7i> ;
    = <http://iflastandards.info/ns/fr/frbr/frbroo/R7_is_example_of> ;
    skos:definition "This property associates a publication with one of its exemplars."@en ;
    skos:scopeNote "It is a shortcut of the more developed path: F5 Item R28B was produced by F32 Carrier Production R26 produced things of type (was produced by): F3 Manifestation Product Type."@en .

<http://iflastandards.info/ns/fr/frbr/frbroo/R7i> a rdf:Property ;
    rdfs:label "has example"@en ;
    reg:name "hasExample"@en ;
    reg:status <http://metadataregistry.org/uri/RegStatus/1001> ;
    rdfs:comment "Inverse of R7_is_example_of."@en ;
    rdfs:domain <http://iflastandards.info/ns/fr/frbr/frbroo/F3> ;
    rdfs:isDefinedBy <http://iflastandards.info/ns/fr/frbr/frbroo/> ;
    rdfs:range <http://iflastandards.info/ns/fr/frbr/frbroo/F5> ;
    rdfs:subPropertyOf <http://www.cidoc-crm.org/cidoc-crm/P2i_is_type_of> ;
    owl:inverseOf <http://iflastandards.info/ns/fr/frbr/frbroo/R7> ;
    = <http://iflastandards.info/ns/fr/frbr/frbroo/R7i_has_example> .

<http://iflastandards.info/ns/fr/frbr/frbroo/R8> a rdf:Property ;
    rdfs:label "consists of"@en ;
    reg:name "consistsOf"@en ;
    reg:status <http://metadataregistry.org/uri/RegStatus/1001> ;
    rdfs:comment "This property associates an instance of F13 Identifier with one of the non-syntactic instances of E90 Symbolic Object which form part of it."@en ;
    rdfs:domain <http://iflastandards.info/ns/fr/frbr/frbroo/F13> ;
    rdfs:isDefinedBy <http://iflastandards.info/ns/fr/frbr/frbroo/> ;
    rdfs:range <http://www.cidoc-crm.org/cidoc-crm/E90_Symbolic_Object> ;
    rdfs:subPropertyOf <http://www.cidoc-crm.org/cidoc-crm/P106_is_composed_of> ;
    owl:inverseOf <http://iflastandards.info/ns/fr/frbr/frbroo/R8i> ;
    = <http://iflastandards.info/ns/fr/frbr/frbroo/R8_consists_of> ;
    skos:definition "This property associates an instance of F13 Identifier with one of the non-syntactic instances of E90 Symbolic Object which form part of it."@en .

<http://iflastandards.info/ns/fr/frbr/frbroo/R8i> a rdf:Property ;
    rdfs:label "forms part of"@en ;
    reg:name "formsPartOf"@en ;
    reg:status <http://metadataregistry.org/uri/RegStatus/1001> ;
    rdfs:comment "Inverse of R8_consists_of."@en ;
    rdfs:domain <http://www.cidoc-crm.org/cidoc-crm/E90_Symbolic_Object> ;
    rdfs:isDefinedBy <http://iflastandards.info/ns/fr/frbr/frbroo/> ;
    rdfs:range <http://iflastandards.info/ns/fr/frbr/frbroo/F13> ;
    rdfs:subPropertyOf <http://www.cidoc-crm.org/cidoc-crm/P106i_forms_part_of> ;
    owl:inverseOf <http://iflastandards.info/ns/fr/frbr/frbroo/R8> ;
    = <http://iflastandards.info/ns/fr/frbr/frbroo/R8i_forms_part_of> .

<http://iflastandards.info/ns/fr/frbr/frbroo/R9> a rdf:Property ;
    rdfs:label "is realised in Self-Contained Expression of Individual Work"@en ;
    reg:name "isRealisedInSelfContainedExpressionOfIndividualWork"@en ;
    reg:status <http://metadataregistry.org/uri/RegStatus/1001> ;
    rdfs:comment "This property associates an F14 Individual Work with the unique F22 Self-Contained Expression that completely conveys it. It is a short cut for the more developed path: F14 Individual Work R19B was realised through F28 Expression Creation R17 created F22 Self-Contained Expression."@en ;
    rdfs:domain <http://iflastandards.info/ns/fr/frbr/frbroo/F14> ;
    rdfs:isDefinedBy <http://iflastandards.info/ns/fr/frbr/frbroo/> ;
    rdfs:range <http://iflastandards.info/ns/fr/frbr/frbroo/F22> ;
    rdfs:subPropertyOf <http://iflastandards.info/ns/fr/frbr/frbroo/R3> ;
    owl:inverseOf <http://iflastandards.info/ns/fr/frbr/frbroo/R9i> ;
    = <http://iflastandards.info/ns/fr/frbr/frbroo/R9_is_realised_in> ;
    skos:definition "This property associates an F14 Individual Work with the unique F22 Self-Contained Expression that completely conveys it."@en ;
    skos:scopeNote "It is a short cut for the more developed path: F14 Individual Work R19B was realised through F28 Expression Creation R17 created F22 Self-Contained Expression."@en .

<http://iflastandards.info/ns/fr/frbr/frbroo/R9i> a rdf:Property ;
    rdfs:label "realises Individual Work by Self-Contained Expression"@en ;
    reg:name "realisesIndividualWorkBySelfContainedExpression"@en ;
    reg:status <http://metadataregistry.org/uri/RegStatus/1001> ;
    rdfs:comment "Inverse of R9_is_realised_in."@en ;
    rdfs:domain <http://iflastandards.info/ns/fr/frbr/frbroo/F22> ;
    rdfs:isDefinedBy <http://iflastandards.info/ns/fr/frbr/frbroo/> ;
    rdfs:range <http://iflastandards.info/ns/fr/frbr/frbroo/F14> ;
    rdfs:subPropertyOf <http://iflastandards.info/ns/fr/frbr/frbroo/R3i> ;
    owl:inverseOf <http://iflastandards.info/ns/fr/frbr/frbroo/R9> ;
    = <http://iflastandards.info/ns/fr/frbr/frbroo/R9i_realises> .

<http://iflastandards.info/ns/fr/frbr/frbroo/F16> a owl:Class ;
    rdfs:label "Container Work"@en ;
    reg:name "ContainerWork"@en ;
    reg:status <http://metadataregistry.org/uri/RegStatus/1001> ;
    rdfs:comment "This class comprises works whose essence is to enhance or add value to expressions from one or more other works without altering them, by the selection, arrangement and/or addition of features of different form, such as layout to words, recitation and movement to texts, instrumentation to musical scores etc. This does not make the contents of the incorporated expressions part of the Container Work, but only part of the resulting expression. Container Work may include the addition of new, original parts to the incorporated expressions, such as introductions, graphics, etc. A new version of a container work does not make the resulting complex work a Container Work as well. The inclusion of expressions from a complex work in a Container Work does not make the Container Work itself complex."@en ;
    rdfs:isDefinedBy <http://iflastandards.info/ns/fr/frbr/frbroo/> ;
    rdfs:subClassOf <http://iflastandards.info/ns/fr/frbr/frbroo/F1> ;
    = <http://iflastandards.info/ns/fr/frbr/frbroo/F16_Container_Work> ;
    skos:definition "This class comprises works whose essence is to enhance or add value to expressions from one or more other works without altering them, by the selection, arrangement and/or addition of features of different form, such as layout to words, recitation and movement to texts, instrumentation to musical scores etc. This does not make the contents of the incorporated expressions part of the Container Work, but only part of the resulting expression."@en ;
    skos:scopeNote "Container Work may include the addition of new, original parts to the incorporated expressions, such as introductions, graphics, etc. A new version of a container work does not make the resulting complex work a Container Work as well. The inclusion of expressions from a complex work in a Container Work does not make the Container Work itself complex."@en .

<http://iflastandards.info/ns/fr/frbr/frbroo/F18> a owl:Class ;
    rdfs:label "Serial Work"@en ;
    reg:name "SerialWork"@en,
        "http://iflastandards.info/ns/fr/frbr/frbroo/F19"@en ;
    reg:status <http://metadataregistry.org/uri/RegStatus/1001> ;
    rdfs:comment "This class comprises works that are, or have been, planned to result in sequences of manifestations with common features. Whereas a work can acquire new members over the time it evolves Expressions and Manifestations are identified with a certain state achieved at a particular point in time. Therefore there is in general no single expression or manifestation representing a complete serial work, unless the serial work is ended. Serial Works may or may not have a plan for an overall expression. The retrospective reprinting of all issues of a Serial Work at once, in the form of a monograph, is regarded to be another member of a Complex Work, which contains the Serial Work and the Individual Work realised in the monograph. This does not make the monograph part of the Serial Work."@en ;
    rdfs:isDefinedBy <http://iflastandards.info/ns/fr/frbr/frbroo/> ;
    rdfs:subClassOf <http://iflastandards.info/ns/fr/frbr/frbroo/F15> ;
    = <http://iflastandards.info/ns/fr/frbr/frbroo/F18_Serial_Work> ;
    skos:definition "This class comprises works that are, or have been, planned to result in sequences of manifestations with common features."@en ;
    skos:scopeNote "Whereas a work can acquire new members over the time it evolves Expressions and Manifestations are identified with a certain state achieved at a particular point in time. Therefore there is in general no single expression or manifestation representing a complete serial work, unless the serial work is ended. Serial Works may or may not have a plan for an overall expression. The retrospective reprinting of all issues of a Serial Work at once, in the form of a monograph, is regarded to be another member of a Complex Work, which contains the Serial Work and the Individual Work realised in the monograph. This does not make the monograph part of the Serial Work."@en .

<http://iflastandards.info/ns/fr/frbr/frbroo/F19> a owl:Class ;
    rdfs:label "Publication Work"@en ;
    reg:name "PublicationWork"@en ;
    reg:status <http://metadataregistry.org/uri/RegStatus/1001> ;
    rdfs:comment "This class comprises works that have been planned to result in a manifestation product type and that pertain to the rendering of expressions from other works."@en ;
    rdfs:isDefinedBy <http://iflastandards.info/ns/fr/frbr/frbroo/> ;
    rdfs:subClassOf <http://iflastandards.info/ns/fr/frbr/frbroo/F16> ;
    = <http://iflastandards.info/ns/fr/frbr/frbroo/F19_Publication_Work> ;
    skos:definition "This class comprises works that have been planned to result in a manifestation product type and that pertain to the rendering of expressions from other works."@en .

<http://iflastandards.info/ns/fr/frbr/frbroo/F20> a owl:Class ;
    rdfs:label "Performance Work"@en ;
    reg:name "PerformanceWork"@en ;
    reg:status <http://metadataregistry.org/uri/RegStatus/1001> ;
    rdfs:comment "This class comprises the sets of concepts for rendering a particular or a series of like performances. F20 Performance Work is declared as a subclass of F16 Container Work. This implies that the incorporated expressions (such as the text of the staged play, the text of the argument for the ballet, the recorded music to be used for the ballet, or the content of the musical score to be used for a concert, etc.) are not by themselves a part of the expression of this F1 Work. Rather, an expression (F25 Performance Plan) of the instructions the stage production, choreography or musical performance consists of incorporates (R14) that textual or musical content. In other words, the text of \"Hamlet\" is not a component of the concepts that underlie a given mise-en-scène of \"Hamlet\", but any staging directions (F25 Performance Plan) that convey a given director's vision of \"Hamlet\" must necessarily incorporate the text of \"Hamlet\"."@en ;
    rdfs:isDefinedBy <http://iflastandards.info/ns/fr/frbr/frbroo/> ;
    rdfs:subClassOf <http://iflastandards.info/ns/fr/frbr/frbroo/F16> ;
    = <http://iflastandards.info/ns/fr/frbr/frbroo/F20_Performance_Work> ;
    skos:definition "This class comprises the sets of concepts for rendering a particular or a series of like performances."@en ;
    skos:scopeNote "F20 Performance Work is declared as a subclass of F16 Container Work. This implies that the incorporated expressions (such as the text of the staged play, the text of the argument for the ballet, the recorded music to be used for the ballet, or the content of the musical score to be used for a concert, etc.) are not by themselves a part of the expression of this F1 Work. Rather, an expression (F25 Performance Plan) of the instructions the stage production, choreography or musical performance consists of incorporates (R14) that textual or musical content. In other words, the text of \"Hamlet\" is not a component of the concepts that underlie a given mise-en-scène of \"Hamlet\", but any staging directions (F25 Performance Plan) that convey a given director's vision of \"Hamlet\" must necessarily incorporate the text of \"Hamlet\"."@en .

<http://iflastandards.info/ns/fr/frbr/frbroo/F23> a owl:Class ;
    rdfs:label "Expression Fragment"@en ;
    reg:name "ExpressionFragment"@en ;
    reg:status <http://metadataregistry.org/uri/RegStatus/1001> ;
    rdfs:comment "This class comprises parts of Expressions and these parts are not Self-contained Expressions themselves. The existence of an instance of F23 Expression Fragment can be due to accident, such as loss of material over time, e.g. the only remaining manuscript of an antique text being partially eaten by worms, or due to deliberate isolation, such as excerpts taken from a text by the compiler of a collection of excerpts. An F23 Expression Fragment is only identified with respect to its occurrence in a known or assumed whole. The size of an instance of F23 Expression Fragment ranges from more than 99% of an instance of F22 Self-Contained Expression to tiny bits (a few words from a text, one bar from a musical composition, one detail from a still image, a two-second clip from a movie, etc.)."@en ;
    rdfs:isDefinedBy <http://iflastandards.info/ns/fr/frbr/frbroo/> ;
    rdfs:subClassOf <http://iflastandards.info/ns/fr/frbr/frbroo/F2> ;
    = <http://iflastandards.info/ns/fr/frbr/frbroo/F23_Expression_Fragment> ;
    skos:definition "This class comprises parts of Expressions and these parts are not Self-contained Expressions themselves."@en ;
    skos:scopeNote "The existence of an instance of F23 Expression Fragment can be due to accident, such as loss of material over time, e.g. the only remaining manuscript of an antique text being partially eaten by worms, or due to deliberate isolation, such as excerpts taken from a text by the compiler of a collection of excerpts. An F23 Expression Fragment is only identified with respect to its occurrence in a known or assumed whole. The size of an instance of F23 Expression Fragment ranges from more than 99% of an instance of F22 Self-Contained Expression to tiny bits (a few words from a text, one bar from a musical composition, one detail from a still image, a two-second clip from a movie, etc.)."@en .

<http://iflastandards.info/ns/fr/frbr/frbroo/F27> a owl:Class ;
    rdfs:label "Work Conception"@en ;
    reg:name "WorkConception"@en ;
    reg:status <http://metadataregistry.org/uri/RegStatus/1001> ;
    rdfs:comment "This class comprises the births of original ideas. It marks the initiation of the creation of a work. This class should be used where there is historical evidence of the initiation before the appearance of physical evidence for the F1 Work. This does not always correlate with the date assigned in common library practice to the work; which is usually a later event."@en ;
    rdfs:isDefinedBy <http://iflastandards.info/ns/fr/frbr/frbroo/> ;
    rdfs:subClassOf <http://www.cidoc-crm.org/cidoc-crm/E65_Creation> ;
    = <http://iflastandards.info/ns/fr/frbr/frbroo/F27_Work_Conception> ;
    skos:definition "This class comprises the births of original ideas. It marks the initiation of the creation of a work."@en ;
    skos:scopeNote "This class should be used where there is historical evidence of the initiation before the appearance of physical evidence for the F1 Work. This does not always correlate with the date assigned in common library practice to the work; which is usually a later event."@en .

<http://iflastandards.info/ns/fr/frbr/frbroo/F31> a owl:Class ;
    rdfs:label "Performance"@en ;
    reg:name "Performance"@en ;
    reg:status <http://metadataregistry.org/uri/RegStatus/1001> ;
    rdfs:comment "This class comprises activities that follow the directions of a performance plan, such as a theatrical play, an expression of a choreographic work or a musical work; i.e., they are intended to communicate directly or indirectly to an audience. Such activities can be identified at various levels of granularity, and can be contiguous or not. Any individual performance (with or without intermissions) is a single instance of F31 Performance. In addition, a complete run of performances can also be seen as an instance of F31 Performance, with individual performances as parts. A complete run of performances may comprise an original run plus any of its extensions and tours. Note that a performance plan may be more or less elaborate, and may even foresee just improvisation."@en ;
    rdfs:isDefinedBy <http://iflastandards.info/ns/fr/frbr/frbroo/> ;
    rdfs:subClassOf <http://www.cidoc-crm.org/cidoc-crm/E7_Activity> ;
    = <http://iflastandards.info/ns/fr/frbr/frbroo/F31_Performance> ;
    skos:definition "This class comprises activities that follow the directions of a performance plan, such as a theatrical play, an expression of a choreographic work or a musical work; i.e., they are intended to communicate directly or indirectly to an audience."@en ;
    skos:scopeNote "Such activities can be identified at various levels of granularity, and can be contiguous or not. Any individual performance (with or without intermissions) is a single instance of F31 Performance. In addition, a complete run of performances can also be seen as an instance of F31 Performance, with individual performances as parts. A complete run of performances may comprise an original run plus any of its extensions and tours. Note that a performance plan may be more or less elaborate, and may even foresee just improvisation."@en .

<http://iflastandards.info/ns/fr/frbr/frbroo/F36> a owl:Class ;
    rdfs:label "Script Conversion"@en ;
    reg:name "ScriptConversion"@en ;
    reg:status <http://metadataregistry.org/uri/RegStatus/1001> ;
    rdfs:comment "This class comprises rule sets for converting signs or arrangements of signs from one script or type set to another."@en ;
    rdfs:isDefinedBy <http://iflastandards.info/ns/fr/frbr/frbroo/> ;
    rdfs:subClassOf <http://www.cidoc-crm.org/cidoc-crm/E29_Design_or_Procedure> ;
    = <http://iflastandards.info/ns/fr/frbr/frbroo/F36_Script_Conversion> ;
    skos:definition "This class comprises rule sets for converting signs or arrangements of signs from one script or type set to another."@en .

<http://iflastandards.info/ns/fr/frbr/frbroo/F43> a owl:Class ;
    rdfs:label "Identifier Rule"@en ;
    reg:name "IdentifierRule"@en,
        "http://www.cidoc-crm.org/cidoc-crm/E29_Design_or_Procedure"@en ;
    reg:status <http://metadataregistry.org/uri/RegStatus/1001> ;
    rdfs:comment "This class comprises sets of instructions relating to the formulation of a unique identifier"@en ;
    rdfs:isDefinedBy <http://iflastandards.info/ns/fr/frbr/frbroo/> ;
    rdfs:subClassOf <http://iflastandards.info/ns/fr/frbr/frbroo/F2> ;
    = <http://iflastandards.info/ns/fr/frbr/frbroo/F43_Identifier_Rule> ;
    skos:definition "This class comprises sets of instructions relating to the formulation of a unique identifier"@en .

<http://iflastandards.info/ns/fr/frbr/frbroo/R4> a rdf:Property ;
    rdfs:label "carriers provided by"@en ;
    reg:name "carriersProvidedBy"@en ;
    reg:status <http://metadataregistry.org/uri/RegStatus/1001> ;
    rdfs:comment "This property associates a publication, i.e. an instance of F3 Manifestation Product Type, with an instance of F2 Expression, which all exemplars of that publication should carry, as long as they are recognised as complete exemplars of that publication. Typically, this property is observed on one exemplar of a publication, and extrapolated to all other exemplars of the same publication. This property is a shortcut of: F2 Expression R14B is incorporated in F24 Publication Expression CLR6B should be carried by F3 Manifestation Product Type."@en ;
    rdfs:domain <http://iflastandards.info/ns/fr/frbr/frbroo/F2> ;
    rdfs:isDefinedBy <http://iflastandards.info/ns/fr/frbr/frbroo/> ;
    rdfs:range <http://iflastandards.info/ns/fr/frbr/frbroo/F3> ;
    rdfs:subPropertyOf <http://www.cidoc-crm.org/cidoc-crm/P128i_is_carried_by> ;
    owl:inverseOf <http://iflastandards.info/ns/fr/frbr/frbroo/R4i> ;
    = <http://iflastandards.info/ns/fr/frbr/frbroo/R4_carriers_provided_by> ;
    skos:definition "This property associates a publication, i.e. an instance of F3 Manifestation Product Type, with an instance of F2 Expression, which all exemplars of that publication should carry, as long as they are recognised as complete exemplars of that publication."@en ;
    skos:scopeNote "Typically, this property is observed on one exemplar of a publication, and extrapolated to all other exemplars of the same publication. This property is a shortcut of: F2 Expression R14B is incorporated in F24 Publication Expression CLR6B should be carried by F3 Manifestation Product Type."@en .

<http://iflastandards.info/ns/fr/frbr/frbroo/R4i> a rdf:Property ;
    rdfs:label "comprises carriers of"@en ;
    reg:name "comprisesCarriersOf"@en ;
    reg:status <http://metadataregistry.org/uri/RegStatus/1001> ;
    rdfs:comment "Inverse of R4_carriers_provided_by."@en ;
    rdfs:domain <http://iflastandards.info/ns/fr/frbr/frbroo/F3> ;
    rdfs:isDefinedBy <http://iflastandards.info/ns/fr/frbr/frbroo/> ;
    rdfs:range <http://iflastandards.info/ns/fr/frbr/frbroo/F2> ;
    rdfs:subPropertyOf <http://www.cidoc-crm.org/cidoc-crm/P128_carries> ;
    owl:inverseOf <http://iflastandards.info/ns/fr/frbr/frbroo/R4> ;
    = <http://iflastandards.info/ns/fr/frbr/frbroo/R4i_comprises_carriers_of> .

<http://iflastandards.info/ns/fr/frbr/frbroo/F14> a owl:Class ;
    rdfs:label "Individual Work"@en ;
    reg:name "IndividualWork"@en ;
    reg:status <http://metadataregistry.org/uri/RegStatus/1001> ;
    rdfs:comment "This class comprises works that are realised by one and only one self-contained expression, i.e., works representing the concept as expressed by precisely this expression, and that do not have other works as parts. Inherent to the notion of work is the completion of recognisable outcomes of the work. These outcomes, i.e. the Self-Contained Expressions, are regarded as the symbolic equivalents of Individual Works, which form the atoms of a complex work. Normally creators would characterise an outcome of a work as finished. In other cases, one could recognise an outcome of a work as complete from the elaboration or logical coherence of its content, or if there is any historical knowledge about the creator deliberately or accidentally never finishing (completing) that particular expression. In all those cases, one would regard the corresponding expression as equivalent to one Individual Work."@en ;
    rdfs:isDefinedBy <http://iflastandards.info/ns/fr/frbr/frbroo/> ;
    rdfs:subClassOf <http://iflastandards.info/ns/fr/frbr/frbroo/F1> ;
    = <http://iflastandards.info/ns/fr/frbr/frbroo/F14_Individual_Work> ;
    skos:definition "This class comprises works that are realised by one and only one self-contained expression, i.e., works representing the concept as expressed by precisely this expression, and that do not have other works as parts."@en ;
    skos:scopeNote "Inherent to the notion of work is the completion of recognisable outcomes of the work. These outcomes, i.e. the Self-Contained Expressions, are regarded as the symbolic equivalents of Individual Works, which form the atoms of a complex work. Normally creators would characterise an outcome of a work as finished. In other cases, one could recognise an outcome of a work as complete from the elaboration or logical coherence of its content, or if there is any historical knowledge about the creator deliberately or accidentally never finishing (completing) that particular expression. In all those cases, one would regard the corresponding expression as equivalent to one Individual Work."@en .

<http://iflastandards.info/ns/fr/frbr/frbroo/R17> a rdf:Property ;
    rdfs:label "created Expression from Expression Creation"@en ;
    reg:name "createdExpressionFromExpressionCreation"@en ;
    reg:status <http://metadataregistry.org/uri/RegStatus/1001> ;
    rdfs:comment "This property associates the expression that was first externalised during a particular creation event with that particular creation event."@en ;
    rdfs:domain <http://iflastandards.info/ns/fr/frbr/frbroo/F28> ;
    rdfs:isDefinedBy <http://iflastandards.info/ns/fr/frbr/frbroo/> ;
    rdfs:range <http://iflastandards.info/ns/fr/frbr/frbroo/F2> ;
    rdfs:subPropertyOf <http://www.cidoc-crm.org/cidoc-crm/P94_has_created> ;
    owl:inverseOf <http://iflastandards.info/ns/fr/frbr/frbroo/R17i> ;
    = <http://iflastandards.info/ns/fr/frbr/frbroo/R17_created> ;
    skos:definition "This property associates the expression that was first externalised during a particular creation event with that particular creation event."@en .

<http://iflastandards.info/ns/fr/frbr/frbroo/R17i> a rdf:Property ;
    rdfs:label "was created by Expression Creation for Expression"@en ;
    reg:name "wasCreatedByExpressionCreationForExpression"@en ;
    reg:status <http://metadataregistry.org/uri/RegStatus/1001> ;
    rdfs:comment "Inverse of R17_created."@en ;
    rdfs:domain <http://iflastandards.info/ns/fr/frbr/frbroo/F2> ;
    rdfs:isDefinedBy <http://iflastandards.info/ns/fr/frbr/frbroo/> ;
    rdfs:range <http://iflastandards.info/ns/fr/frbr/frbroo/F28> ;
    rdfs:subPropertyOf <http://www.cidoc-crm.org/cidoc-crm/P94i_was_created_by> ;
    owl:inverseOf <http://iflastandards.info/ns/fr/frbr/frbroo/R17> ;
    = <http://iflastandards.info/ns/fr/frbr/frbroo/R17i_was_created_by> .

<http://iflastandards.info/ns/fr/frbr/frbroo/R19> a rdf:Property ;
    rdfs:label "created a realization of Work by Expression Creation"@en ;
    reg:name "createdARealizationOfWorkByExpressionCreation"@en ;
    reg:status <http://metadataregistry.org/uri/RegStatus/1001> ;
    rdfs:comment "This property associates an instance of F28 Expression Creation with the corresponding instance of F14 Individual Work or an instance of F15 Complex Work of which the corresponding instance of F14 Individual Work is a member."@en ;
    rdfs:domain <http://iflastandards.info/ns/fr/frbr/frbroo/F28> ;
    rdfs:isDefinedBy <http://iflastandards.info/ns/fr/frbr/frbroo/> ;
    rdfs:range <http://iflastandards.info/ns/fr/frbr/frbroo/F1> ;
    rdfs:subPropertyOf <http://www.cidoc-crm.org/cidoc-crm/P16_used_specific_object> ;
    owl:inverseOf <http://iflastandards.info/ns/fr/frbr/frbroo/R19i> ;
    = <http://iflastandards.info/ns/fr/frbr/frbroo/R19_created_a_realization_of> ;
    skos:definition "This property associates an instance of F28 Expression Creation with the corresponding instance of F14 Individual Work or an instance of F15 Complex Work of which the corresponding instance of F14 Individual Work is a member."@en .

<http://iflastandards.info/ns/fr/frbr/frbroo/R19i> a rdf:Property ;
    rdfs:label "was realised through Expression Creation for Work"@en ;
    reg:name "wasRealisedThroughExpressionCreationForWork"@en ;
    reg:status <http://metadataregistry.org/uri/RegStatus/1001> ;
    rdfs:comment "Inverse of R19_created_a_realization_of."@en ;
    rdfs:domain <http://iflastandards.info/ns/fr/frbr/frbroo/F1> ;
    rdfs:isDefinedBy <http://iflastandards.info/ns/fr/frbr/frbroo/> ;
    rdfs:range <http://iflastandards.info/ns/fr/frbr/frbroo/F28> ;
    rdfs:subPropertyOf <http://www.cidoc-crm.org/cidoc-crm/P16i_was_used_for> ;
    owl:inverseOf <http://iflastandards.info/ns/fr/frbr/frbroo/R19> ;
    = <http://iflastandards.info/ns/fr/frbr/frbroo/R19i_was_realised_through> .

<http://iflastandards.info/ns/fr/frbr/frbroo/F12> a owl:Class ;
    rdfs:label "Nomen"@en ;
    reg:name "Nomen"@en ;
    reg:status <http://metadataregistry.org/uri/RegStatus/1001> ;
    rdfs:comment "This class comprises any sign or arrangements of signs following a specific syntax (sequences of alphanumeric characters, chemical structure symbols, sound symbols, ideograms etc.) that are used or can be used to refer to and identify a specific instance of some class or category within a certain context. The scripts or type sets for the types of symbols used to compose an instance of F12 Nomen have to be explicitly specified. The identity of an instance of F12 Nomen is given by the order of its symbols and their individual role with respect to their scripts, regardless of the semantics of the larger structural components it may be built from. Structural tags occurring in the nomen string are regarded as symbols constituting the nomen. Spelling variants are regarded as different nomina, whereas the use of different fonts (visual representation variants) or different digital encodings do not change the identity."@en ;
    rdfs:isDefinedBy <http://iflastandards.info/ns/fr/frbr/frbroo/> ;
    rdfs:subClassOf <http://www.cidoc-crm.org/cidoc-crm/E41_Appellation> ;
    = <http://iflastandards.info/ns/fr/frbr/frbroo/F12_Nomen> ;
    skos:definition "This class comprises any sign or arrangements of signs following a specific syntax (sequences of alphanumeric characters, chemical structure symbols, sound symbols, ideograms etc.) that are used or can be used to refer to and identify a specific instance of some class or category within a certain context."@en ;
    skos:scopeNote "The scripts or type sets for the types of symbols used to compose an instance of F12 Nomen have to be explicitly specified. The identity of an instance of F12 Nomen is given by the order of its symbols and their individual role with respect to their scripts, regardless of the semantics of the larger structural components it may be built from. Structural tags occurring in the nomen string are regarded as symbols constituting the nomen. Spelling variants are regarded as different nomina, whereas the use of different fonts (visual representation variants) or different digital encodings do not change the identity."@en .

<http://iflastandards.info/ns/fr/frbr/frbroo/F21> a owl:Class ;
    rdfs:label "Recording Work"@en ;
    reg:name "RecordingWork"@en ;
    reg:status <http://metadataregistry.org/uri/RegStatus/1001> ;
    rdfs:comment "This class comprises works that conceptualise the capturing of features of perdurants. The characteristics of the manifestation of a recording work are those of the product of the capture process. The characteristics of any other works recorded are distinct from those of the recording work itself. In the case where the recorded perdurant expresses some Work, the respective instance of F21 is also an F16 Container Work"@en ;
    rdfs:isDefinedBy <http://iflastandards.info/ns/fr/frbr/frbroo/> ;
    rdfs:subClassOf <http://iflastandards.info/ns/fr/frbr/frbroo/F1> ;
    = <http://iflastandards.info/ns/fr/frbr/frbroo/F21_Recording_Work> ;
    skos:definition "This class comprises works that conceptualise the capturing of features of perdurants."@en ;
    skos:scopeNote "The characteristics of the manifestation of a recording work are those of the product of the capture process. The characteristics of any other works recorded are distinct from those of the recording work itself. In the case where the recorded perdurant expresses some Work, the respective instance of F21 is also an F16 Container Work"@en .

<http://iflastandards.info/ns/fr/frbr/frbroo/F25> a owl:Class ;
    rdfs:label "Performance Plan"@en ;
    reg:name "PerformancePlan"@en,
        "http://www.cidoc-crm.org/cidoc-crm/E29_Design_or_Procedure"@en ;
    reg:status <http://metadataregistry.org/uri/RegStatus/1001> ;
    rdfs:comment "This class comprises sets of directions to which individual performances of theatrical, choreographic, or musical works and their combinations should conform. In the case of theatrical performances, such directions incorporate, but are not limited nor reducible to, the text of a given version of the play performed (e.g., a translated text, some passages of which are deliberately omitted, with some rephrased lines, etc.). In the case of choreographic performances, such directions may incorporate, but are neither limited nor reducible to, the notation of choreographic movements in systems such as labanotation. In the case of musical performances, such directions may incorporate, but are neither limited nor reducible to, the musical score. In case of electronic music, they may incorporate software instructions. These directions may or may not completely determine the form of the intended performance. Depending on the nature of the directions, the form of the intended performance, such as the sets of movements or the sound characteristics, may or may not be predictable from the directions. Note that a performance plan may be more or less elaborate, and may even foresee just improvisation."@en ;
    rdfs:isDefinedBy <http://iflastandards.info/ns/fr/frbr/frbroo/> ;
    rdfs:subClassOf <http://iflastandards.info/ns/fr/frbr/frbroo/F22> ;
    = <http://iflastandards.info/ns/fr/frbr/frbroo/F25_Performance_Plan> ;
    skos:definition "This class comprises sets of directions to which individual performances of theatrical, choreographic, or musical works and their combinations should conform."@en ;
    skos:scopeNote "In the case of theatrical performances, such directions incorporate, but are not limited nor reducible to, the text of a given version of the play performed (e.g., a translated text, some passages of which are deliberately omitted, with some rephrased lines, etc.). In the case of choreographic performances, such directions may incorporate, but are neither limited nor reducible to, the notation of choreographic movements in systems such as labanotation. In the case of musical performances, such directions may incorporate, but are neither limited nor reducible to, the musical score. In case of electronic music, they may incorporate software instructions."@en .

<http://iflastandards.info/ns/fr/frbr/frbroo/F26> a owl:Class ;
    rdfs:label "Recording"@en ;
    reg:name "Recording"@en ;
    reg:status <http://metadataregistry.org/uri/RegStatus/1001> ;
    rdfs:comment "This class comprises expressions which are created in instances of F29 Recording Event. A recording is intended to convey (and preserve) the features of one or more perdurants."@en ;
    rdfs:isDefinedBy <http://iflastandards.info/ns/fr/frbr/frbroo/> ;
    rdfs:subClassOf <http://iflastandards.info/ns/fr/frbr/frbroo/F22> ;
    = <http://iflastandards.info/ns/fr/frbr/frbroo/F26_Recording> ;
    skos:definition "This class comprises expressions which are created in instances of F29 Recording Event. A recording is intended to convey (and preserve) the features of one or more perdurants."@en .

<http://iflastandards.info/ns/fr/frbr/frbroo/F30> a owl:Class ;
    rdfs:label "Publication Event"@en ;
    reg:name "PublicationEvent"@en ;
    reg:status <http://metadataregistry.org/uri/RegStatus/1001> ;
    rdfs:comment "This class comprises the activities of publishing. Such an event includes the creation of an F24 Publication Expression and setting up the means of production. The end of this event is regarded as the date of publication, regardless of whether the carrier production is started. Publishing can be either physical or electronic. Electronic publishing is regarded as making an instance of F24 Publication Expression available in electronic form on a public network. Electronic Publishing does not mean producing a physical F5 Item by partially electronic means. Making an electronic file available on a physical carrier can be regarded as equivalent to setting up the means of production; downloading the file is regarded as the electronic equivalent of F32 Carrier Production Event."@en ;
    rdfs:isDefinedBy <http://iflastandards.info/ns/fr/frbr/frbroo/> ;
    rdfs:subClassOf <http://iflastandards.info/ns/fr/frbr/frbroo/F28> ;
    = <http://iflastandards.info/ns/fr/frbr/frbroo/F30_Publication_Event> ;
    skos:definition "This class comprises the activities of publishing."@en ;
    skos:scopeNote "Such an event includes the creation of an F24 Publication Expression and setting up the means of production. The end of this event is regarded as the date of publication, regardless of whether the carrier production is started. Publishing can be either physical or electronic. Electronic publishing is regarded as making an instance of F24 Publication Expression available in electronic form on a public network. Electronic Publishing does not mean producing a physical F5 Item by partially electronic means. Making an electronic file available on a physical carrier can be regarded as equivalent to setting up the means of production; downloading the file is regarded as the electronic equivalent of F32 Carrier Production Event."@en .

<http://iflastandards.info/ns/fr/frbr/frbroo/F33> a owl:Class ;
    rdfs:label "Reproduction Event"@en ;
    reg:name "ReproductionEvent"@en ;
    reg:status <http://metadataregistry.org/uri/RegStatus/1001> ;
    rdfs:comment "This class comprises activities that consist in making copies, more or less mechanically, of an instance of E84 Information Carrier (such as an F5 Item or an F4 Manifestation Singleton which is also instance of E84 Information Carrier), preserving the expression carried by it. A Reproduction Event results in new instances of E84 Information Carrier coming into existence. In general, the copy will have different attributes from the original and they are therefore not regarded as siblings. This class makes it possible to account for the legal distinction between private copying for the purpose of \"fair use\", and mass production for the purpose of dissemination. It can prove difficult to determine where to draw the line between F33 Reproduction Event and F32 Carrier Production Event in cases where multiple copies are produced. In this case, the copies, but not the original, may be regarded as instances of F5 Item. It is the existence of an explicit production plan that makes the difference. As a consequence, F33 Reproduction Event and F32 Carrier Production Event are not declared as disjoint, which makes it possible to account for such situations that could be regarded as instances of both Production Event and Reproduction Event."@en ;
    rdfs:isDefinedBy <http://iflastandards.info/ns/fr/frbr/frbroo/> ;
    rdfs:subClassOf <http://www.cidoc-crm.org/cidoc-crm/E12_Production> ;
    = <http://iflastandards.info/ns/fr/frbr/frbroo/F33_Reproduction_Event> ;
    skos:definition "This class comprises activities that consist in making copies, more or less mechanically, of an instance of E84 Information Carrier (such as an F5 Item or an F4 Manifestation Singleton which is also instance of E84 Information Carrier), preserving the expression carried by it."@en ;
    skos:scopeNote "A Reproduction Event results in new instances of E84 Information Carrier coming into existence. In general, the copy will have different attributes from the original and they are therefore not regarded as siblings. This class makes it possible to account for the legal distinction between private copying for the purpose of \"fair use\", and mass production for the purpose of dissemination. It can prove difficult to determine where to draw the line between F33 Reproduction Event and F32 Carrier Production Event in cases where multiple copies are produced. In this case, the copies, but not the original, may be regarded as instances of F5 Item. It is the existence of an explicit production plan that makes the difference. As a consequence, F33 Reproduction Event and F32 Carrier Production Event are not declared as disjoint, which makes it possible to account for such situations that could be regarded as instances of both Production Event and Reproduction Event."@en .

<http://iflastandards.info/ns/fr/frbr/frbroo/F34> a owl:Class ;
    rdfs:label "KOS"@en ;
    reg:name "KOS"@en,
        "http://www.cidoc-crm.org/cidoc-crm/E29_Design_or_Procedure"@en,
        "http://www.cidoc-crm.org/cidoc-crm/E32_Authority_Document"@en ;
    reg:status <http://metadataregistry.org/uri/RegStatus/1001> ;
    rdfs:comment "This class comprises documents that establish controlled terminology (nomina) for consistent use. They may also describe relationships between entities and controlled terminology and relationships between entities. Note that any meaningful change in a Knowledge Organisation System (KOS) that affects the validity status of its elements defines a new release (Expression) of the KOS. Note that identifiers created following a rule in a KOS are to be regarded as being taken from this KOS, even though not explicitly spelled out. This definition of KOS reflects current library practice and not the use of the term in general."@en ;
    rdfs:isDefinedBy <http://iflastandards.info/ns/fr/frbr/frbroo/> ;
    rdfs:subClassOf <http://iflastandards.info/ns/fr/frbr/frbroo/F2> ;
    = <http://iflastandards.info/ns/fr/frbr/frbroo/F34_KOS> ;
    skos:definition "This class comprises documents that establish controlled terminology (nomina) for consistent use. They may also describe relationships between entities and controlled terminology and relationships between entities."@en ;
    skos:scopeNote "Note that any meaningful change in a Knowledge Organisation System (KOS) that affects the validity status of its elements defines a new release (Expression) of the KOS. Note that identifiers created following a rule in a KOS are to be regarded as being taken from this KOS, even though not explicitly spelled out. This definition of KOS reflects current library practice and not the use of the term in general."@en .

<http://iflastandards.info/ns/fr/frbr/frbroo/F44> a owl:Class ;
    rdfs:label "Bibliographic Agency"@en ;
    reg:name "BibliographicAgency"@en ;
    reg:status <http://metadataregistry.org/uri/RegStatus/1001> ;
    rdfs:comment "This class comprises agents who create the bibliographic description of publications and perform the authority control associated with such descriptions, for the description of copies of such publications actually held by libraries, and for the description of unique documents (manuscripts, objects …) held by libraries. The activity of creating such descriptions implies that one has to make decisions (as to the uniform title for a work, as to whether an arrangement still belongs to the same work or is definitely a new work, etc.). Since such decisions always are debatable and different agencies can make different decisions about the same real-world entities, it is important to document which agency made which decision."@en ;
    rdfs:isDefinedBy <http://iflastandards.info/ns/fr/frbr/frbroo/> ;
    rdfs:subClassOf <http://www.cidoc-crm.org/cidoc-crm/E40_Legal_Body> ;
    = <http://iflastandards.info/ns/fr/frbr/frbroo/F44_Bibliographic_Agency> ;
    skos:definition "This class comprises agents who create the bibliographic description of publications and perform the authority control associated with such descriptions, for the description of copies of such publications actually held by libraries, and for the description of unique documents (manuscripts, objects …) held by libraries."@en ;
    skos:scopeNote "The activity of creating such descriptions implies that one has to make decisions (as to the uniform title for a work, as to whether an arrangement still belongs to the same work or is definitely a new work, etc.). Since such decisions always are debatable and different agencies can make different decisions about the same real-world entities, it is important to document which agency made which decision."@en .

<http://iflastandards.info/ns/fr/frbr/frbroo/F51> a owl:Class ;
    rdfs:label "Pursuit"@en ;
    reg:name "Pursuit"@en ;
    reg:status <http://metadataregistry.org/uri/RegStatus/1001> ;
    rdfs:comment "This class comprises periods of continuous activity of an Actor in a specific professional or creative domain or field."@en ;
    rdfs:isDefinedBy <http://iflastandards.info/ns/fr/frbr/frbroo/> ;
    rdfs:subClassOf <http://www.cidoc-crm.org/cidoc-crm/E7_Activity> ;
    = <http://iflastandards.info/ns/fr/frbr/frbroo/F51_Pursuit> ;
    skos:definition "This class comprises periods of continuous activity of an Actor in a specific professional or creative domain or field."@en .

<http://iflastandards.info/ns/fr/frbr/frbroo/F13> a owl:Class ;
    rdfs:label "Identifier"@en ;
    reg:name "Identifier"@en,
        "http://www.cidoc-crm.org/cidoc-crm/E42_Identifier"@en ;
    reg:status <http://metadataregistry.org/uri/RegStatus/1001> ;
    rdfs:comment "This class comprises strings or codes assigned to instances of E1 CRM Entity in order to identify them uniquely and permanently within the context of one or more organisations. Such codes are often known as inventory numbers, registration codes, etc. and are typically composed of alphanumeric sequences. The class E42 Identifier is not normally used for machine-generated identifiers used for automated processing unless these are also used by human agents. [Adapted from the Scope Note of CIDOC CRM E42 Identifier ver. 5.0.1]"@en ;
    rdfs:isDefinedBy <http://iflastandards.info/ns/fr/frbr/frbroo/> ;
    rdfs:subClassOf <http://iflastandards.info/ns/fr/frbr/frbroo/F12> ;
    = <http://iflastandards.info/ns/fr/frbr/frbroo/F13_Identifier> ;
    skos:definition "This class comprises strings or codes assigned to instances of E1 CRM Entity in order to identify them uniquely and permanently within the context of one or more organisations. Such codes are often known as inventory numbers, registration codes, etc. and are typically composed of alphanumeric sequences."@en ;
    skos:scopeNote "The class E42 Identifier is not normally used for machine-generated identifiers used for automated processing unless these are also used by human agents."@en .

<http://iflastandards.info/ns/fr/frbr/frbroo/F15> a owl:Class ;
    rdfs:label "Complex Work"@en ;
    reg:name "ComplexWork"@en ;
    reg:status <http://metadataregistry.org/uri/RegStatus/1001> ;
    rdfs:comment "This class comprises works that have more than one work as members. The members of a Complex Work may constitute components of the overall concept or be alternatives to other members of the work. In practice, no clear line can be drawn between parallel and subsequent processes in the evolution of a work. One part may not be finished when another is already revised. An initially monolithic work may be taken up and evolve in pieces. The member relationship of Work is based on the conceptual relationship, and should not be confused with the internal structural parts of an individual expression. The fact that an expression may contain parts from other work(s) does not make the expressed work complex. For instance, an anthology for which only one version exists is not a complex work. The boundaries of a Complex Work have nothing to do with the value of the intellectual achievement but only with the dominance of a concept. Thus, derivations such as translations are regarded as belonging to the same Complex Work, even though in addition they constitute an Individual Work themselves. In contrast, a Work that significantly takes up and merges concepts of other works so that it is no longer dominated by the initial concept is regarded as a new work. In cataloguing practice, detailed rules are established prescribing which kinds of derivation should be regarded as crossing the boundaries of a complex work. Adaptation and derivation graphs allow the recognition of distinct sub-units, i.e. a complex work contained in a larger complex work. As a Complex Work can be taken up by any creator who acquires the spirit of its concept, it is never finished in an absolute sense."@en ;
    rdfs:isDefinedBy <http://iflastandards.info/ns/fr/frbr/frbroo/> ;
    rdfs:subClassOf <http://iflastandards.info/ns/fr/frbr/frbroo/F1> ;
    = <http://iflastandards.info/ns/fr/frbr/frbroo/F15_Complex_Work> ;
    skos:definition "This class comprises works that have more than one work as members."@en ;
    skos:scopeNote "The members of a Complex Work may constitute components of the overall concept or be alternatives to other members of the work. In practice, no clear line can be drawn between parallel and subsequent processes in the evolution of a work. One part may not be finished when another is already revised. An initially monolithic work may be taken up and evolve in pieces. The member relationship of Work is based on the conceptual relationship, and should not be confused with the internal structural parts of an individual expression. The fact that an expression may contain parts from other work(s) does not make the expressed work complex. For instance, an anthology for which only one version exists is not a complex work. The boundaries of a Complex Work have nothing to do with the value of the intellectual achievement but only with the dominance of a concept. Thus, derivations such as translations are regarded as belonging to the same Complex Work, even though in addition they constitute an Individual Work themselves. In contrast, a Work that significantly takes up and merges concepts of other works so that it is no longer dominated by the initial concept is regarded as a new work. In cataloguing practice, detailed rules are established prescribing which kinds of derivation should be regarded as crossing the boundaries of a complex work. Adaptation and derivation graphs allow the recognition of distinct sub-units, i.e. a complex work contained in a larger complex work. As a Complex Work can be taken up by any creator who acquires the spirit of its concept, it is never finished in an absolute sense."@en .

<http://iflastandards.info/ns/fr/frbr/frbroo/R3> a rdf:Property ;
    rdfs:label "is realised in Self-Contained Expression of Work"@en ;
    reg:name "isRealisedInSelfContainedExpressionOfWork"@en ;
    reg:status <http://metadataregistry.org/uri/RegStatus/1001> ;
    rdfs:comment "This property associates an instance of F22 Self-Contained Expression with an instance of F1 Work. This property expresses the association that exists between an expression (F22) and the work that this expression conveys. The semantics of the association will be different depending on what specific subtype of F1 Work the work is an instance of. If the work is an instance of F14 Individual Work, the F22 Self-Contained Expression completely conveys the individual work. If the work is an instance of F15 Complex work, the F22 Self-Contained Expression conveys an alternative member of the complex work. Our factual knowledge of how a given work is realised into an expression is often limited and this property makes it possible to express the association between instances of F22 Self-Contained Expression and the work it conveys without using the more developed paths."@en ;
    rdfs:domain <http://iflastandards.info/ns/fr/frbr/frbroo/F1> ;
    rdfs:isDefinedBy <http://iflastandards.info/ns/fr/frbr/frbroo/> ;
    rdfs:range <http://iflastandards.info/ns/fr/frbr/frbroo/F22> ;
    rdfs:subPropertyOf <http://www.cidoc-crm.org/cidoc-crm/P130_shows_features_of> ;
    owl:inverseOf <http://iflastandards.info/ns/fr/frbr/frbroo/R3i> ;
    = <http://iflastandards.info/ns/fr/frbr/frbroo/R3_is_realised_in> ;
    skos:definition "This property associates an instance of F22 Self-Contained Expression with an instance of F1 Work."@en ;
    skos:scopeNote "This property expresses the association that exists between an expression (F22) and the work that this expression conveys. The semantics of the association will be different depending on what specific subtype of F1 Work the work is an instance of. If the work is an instance of F14 Individual Work, the F22 Self-Contained Expression completely conveys the individual work. If the work is an instance of F15 Complex work, the F22 Self-Contained Expression conveys an alternative member of the complex work. Our factual knowledge of how a given work is realised into an expression is often limited and this property makes it possible to express the association between instances of F22 Self-Contained Expression and the work it conveys without using the more developed paths."@en .

<http://iflastandards.info/ns/fr/frbr/frbroo/R3i> a rdf:Property ;
    rdfs:label "realises Work by Self-Contained Expression"@en ;
    reg:name "realisesWorkBySelfContainedExpression"@en ;
    reg:status <http://metadataregistry.org/uri/RegStatus/1001> ;
    rdfs:comment "Inverse of R3_is_realised_in."@en ;
    rdfs:domain <http://iflastandards.info/ns/fr/frbr/frbroo/F22> ;
    rdfs:isDefinedBy <http://iflastandards.info/ns/fr/frbr/frbroo/> ;
    rdfs:range <http://iflastandards.info/ns/fr/frbr/frbroo/F1> ;
    rdfs:subPropertyOf <http://www.cidoc-crm.org/cidoc-crm/P130i_features_are_also_found_on> ;
    owl:inverseOf <http://iflastandards.info/ns/fr/frbr/frbroo/R3> ;
    = <http://iflastandards.info/ns/fr/frbr/frbroo/R3i_realises> .

<http://iflastandards.info/ns/fr/frbr/frbroo/F29> a owl:Class ;
    rdfs:label "Recording Event"@en ;
    reg:name "RecordingEvent"@en ;
    reg:status <http://metadataregistry.org/uri/RegStatus/1001> ;
    rdfs:comment "This class comprises activities that intend to convey (and preserve) the content of events in a recording, such as a live recording of a performance, a documentary, or other capture of a perdurant. Such activities may follow the directions of a recording plan. They may include postproduction."@en ;
    rdfs:isDefinedBy <http://iflastandards.info/ns/fr/frbr/frbroo/> ;
    rdfs:subClassOf <http://iflastandards.info/ns/fr/frbr/frbroo/F28> ;
    = <http://iflastandards.info/ns/fr/frbr/frbroo/F29_Recording_Event> ;
    skos:definition "This class comprises activities that intend to convey (and preserve) the content of events in a recording, such as a live recording of a performance, a documentary, or other capture of a perdurant."@en ;
    skos:scopeNote "Such activities may follow the directions of a recording plan. They may include postproduction."@en .

<http://iflastandards.info/ns/fr/frbr/frbroo/F32> a owl:Class ;
    rdfs:label "Carrier Production Event"@en ;
    reg:name "CarrierProductionEvent"@en ;
    reg:status <http://metadataregistry.org/uri/RegStatus/1001> ;
    rdfs:comment "This class comprises activities that result in instances of F5 Item coming into existence. The creation of a new copy of a file on an electronic carrier is also regarded as a Carrier Production Event. Typically, the production of copies of a publication (no matter whether it is a book, a sound recording, a DVD, a cartographic resource, etc.) strives to produce items all as similar as possible to a prototype that displays all the features that all the copies of the publication should also display, which is reflected in property R27 used as source material F24 Publication Expression."@en ;
    rdfs:isDefinedBy <http://iflastandards.info/ns/fr/frbr/frbroo/> ;
    rdfs:subClassOf <http://www.cidoc-crm.org/cidoc-crm/E12_Production> ;
    = <http://iflastandards.info/ns/fr/frbr/frbroo/F32_Carrier_Production_Event> ;
    skos:definition "This class comprises activities that result in instances of F5 Item coming into existence."@en ;
    skos:scopeNote "The creation of a new copy of a file on an electronic carrier is also regarded as a Carrier Production Event. Typically, the production of copies of a publication (no matter whether it is a book, a sound recording, a DVD, a cartographic resource, etc.) strives to produce items all as similar as possible to a prototype that displays all the features that all the copies of the publication should also display, which is reflected in property R27 used as source material F24 Publication Expression."@en .

<http://iflastandards.info/ns/fr/frbr/frbroo/F38> a owl:Class ;
    rdfs:label "Character"@en ;
    reg:name "Character"@en ;
    reg:status <http://metadataregistry.org/uri/RegStatus/1001> ;
    rdfs:comment "This class comprises fictional or iconographic individuals or groups of individual appearing in works in a way relevant as subjects. Characters may be purely fictitious or based on real persons or groups, but as characters they may exhibit properties that would be inconsistent with a real person or group. Rather than merging characters with real persons, they should be described as disjoint, but related entities."@en ;
    rdfs:isDefinedBy <http://iflastandards.info/ns/fr/frbr/frbroo/> ;
    rdfs:subClassOf <http://www.cidoc-crm.org/cidoc-crm/E28_Conceptual_Object> ;
    = <http://iflastandards.info/ns/fr/frbr/frbroo/F38_Character> ;
    skos:definition "This class comprises fictional or iconographic individuals or groups of individual appearing in works in a way relevant as subjects."@en ;
    skos:scopeNote "Characters may be purely fictitious or based on real persons or groups, but as characters they may exhibit properties that would be inconsistent with a real person or group. Rather than merging characters with real persons, they should be described as disjoint, but related entities."@en .

<http://iflastandards.info/ns/fr/frbr/frbroo/F4> a owl:Class ;
    rdfs:label "Manifestation Singleton"@en ;
    reg:name "ManifestationSingleton"@en ;
    reg:status <http://metadataregistry.org/uri/RegStatus/1001> ;
    rdfs:comment "This class comprises physical objects that each carry an instance of F2 Expression, and that were produced as unique objects, with no siblings intended in the course of their production. It should be noted that if all but one copy of a given publication are destroyed, then that copy does not become an instance of F4 Manifestation Singleton, because it was produced together with sibling copies, even though it now happens to be unique. Examples of instances of F4 Manifestation Singleton include manuscripts, preparatory sketches and the final clean draft sent by an author or a composer to a publisher."@en ;
    rdfs:isDefinedBy <http://iflastandards.info/ns/fr/frbr/frbroo/> ;
    rdfs:subClassOf <http://www.cidoc-crm.org/cidoc-crm/E24_Physical_Man-Made_Thing> ;
    = <http://iflastandards.info/ns/fr/frbr/frbroo/F4_Manifestation_Singleton> ;
    skos:definition "This class comprises physical objects that each carry an instance of F2 Expression, and that were produced as unique objects, with no siblings intended in the course of their production."@en ;
    skos:scopeNote "It should be noted that if all but one copy of a given publication are destroyed, then that copy does not become an instance of F4 Manifestation Singleton, because it was produced together with sibling copies, even though it now happens to be unique. Examples of instances of F4 Manifestation Singleton include manuscripts, preparatory sketches and the final clean draft sent by an author or a composer to a publisher."@en .

<http://iflastandards.info/ns/fr/frbr/frbroo/F42> a owl:Class ;
    rdfs:label "Representative Expression Assignment"@en ;
    reg:name "RepresentativeExpressionAssignment"@en ;
    reg:status <http://metadataregistry.org/uri/RegStatus/1001> ;
    rdfs:comment "This class comprises activities through which an Agency declares (implicitly or explicitly) that a given instance of F2 Expression is representative for a given F15 Complex Work, i.e., that some attributes of that instance of F2 Expression (most prominently, information about the title) can be inferred to also apply to that instance of F15 Complex Work, no matter in which particular expression it is realised. The reasoning behind this is that the Work title is known through the title of an Expression that is deemed representative of the Work, and the title of the representative Expression is known through the title of a Manifestation that is deemed representative of the Expression that is representative of the Work. For instance, by using the qualified uniform title \"Poe, Edgar Allan, 1809-1849. Murders in the rue Morgue (French)\" for the French rendition of Poe's \"Murders in the rue Morgue\" by Baudelaire, an Agency implicitly states that the French text does not constitute a representative F2 Expression for Poe's F1 Work, however the original English text does constitute a representative F2 Expression for Poe's F1 Work."@en ;
    rdfs:isDefinedBy <http://iflastandards.info/ns/fr/frbr/frbroo/> ;
    rdfs:subClassOf <http://www.cidoc-crm.org/cidoc-crm/E13_Attribute_Assignment> ;
    = <http://iflastandards.info/ns/fr/frbr/frbroo/F42_Representative_Expression_Assignment> ;
    skos:definition "This class comprises activities through which an Agency declares (implicitly or explicitly) that a given instance of F2 Expression is representative for a given F15 Complex Work, i.e., that some attributes of that instance of F2 Expression (most prominently, information about the title) can be inferred to also apply to that instance of F15 Complex Work, no matter in which particular expression it is realised."@en ;
    skos:scopeNote "The reasoning behind this is that the Work title is known through the title of an Expression that is deemed representative of the Work, and the title of the representative Expression is known through the title of a Manifestation that is deemed representative of the Expression that is representative of the Work. For instance, by using the qualified uniform title \"Poe, Edgar Allan, 1809-1849. Murders in the rue Morgue (French)\" for the French rendition of Poe's \"Murders in the rue Morgue\" by Baudelaire, an Agency implicitly states that the French text does not constitute a representative F2 Expression for Poe's F1 Work, however the original English text does constitute a representative F2 Expression for Poe's F1 Work."@en .

<http://iflastandards.info/ns/fr/frbr/frbroo/F5> a owl:Class ;
    rdfs:label "Item"@en ;
    reg:name "Item"@en ;
    reg:status <http://metadataregistry.org/uri/RegStatus/1001> ;
    rdfs:comment "This class comprises physical objects (printed books, scores, CDs, DVDs, CD-ROMS, etc.) that carry a F24 Publication Expression and were produced by an industrial process involving a F3 Manifestation Product Type."@en ;
    rdfs:isDefinedBy <http://iflastandards.info/ns/fr/frbr/frbroo/> ;
    rdfs:subClassOf <http://www.cidoc-crm.org/cidoc-crm/E84_Information_Carrier> ;
    = <http://iflastandards.info/ns/fr/frbr/frbroo/F5_Item> ;
    skos:definition "This class comprises physical objects (printed books, scores, CDs, DVDs, CD-ROMS, etc.) that carry a F24 Publication Expression and were produced by an industrial process involving a F3 Manifestation Product Type."@en .

<http://iflastandards.info/ns/fr/frbr/frbroo/F24> a owl:Class ;
    rdfs:label "Publication Expression"@en ;
    reg:name "PublicationExpression"@en ;
    reg:status <http://metadataregistry.org/uri/RegStatus/1001> ;
    rdfs:comment "This class comprises complete sets of signs present in publications, reflecting publishers' final decisions as to both selection of content and layout of the publications. Frequently the creation of a Publication Expression includes both adding graphical form and fonts to Expressions consisting of words alone and selecting illustrations and other content. As such, an instance of Publication Expression incorporates all Expressions combined for the resulting final form of rendering, whether visual, audio or tactile. An instance of Publication Expression is one entity regardless of the number of independent Expressions published within it, as long as it represents one unit of release. The published third party content can be associated via the property R14 incorporates (is incorporated in)."@en ;
    rdfs:isDefinedBy <http://iflastandards.info/ns/fr/frbr/frbroo/> ;
    rdfs:subClassOf <http://iflastandards.info/ns/fr/frbr/frbroo/F22> ;
    = <http://iflastandards.info/ns/fr/frbr/frbroo/F24_Publication_Expression> ;
    skos:definition "This class comprises complete sets of signs present in publications, reflecting publishers' final decisions as to both selection of content and layout of the publications."@en ;
    skos:scopeNote "Frequently the creation of a Publication Expression includes both adding graphical form and fonts to Expressions consisting of words alone and selecting illustrations and other content. As such, an instance of Publication Expression incorporates all Expressions combined for the resulting final form of rendering, whether visual, audio or tactile. An instance of Publication Expression is one entity regardless of the number of independent Expressions published within it, as long as it represents one unit of release. The published third party content can be associated via the property R14 incorporates (is incorporated in)."@en .

<http://iflastandards.info/ns/fr/frbr/frbroo/F28> a owl:Class ;
    rdfs:label "Expression Creation"@en ;
    reg:name "ExpressionCreation"@en,
        "http://www.cidoc-crm.org/cidoc-crm/E65_Creation"@en ;
    reg:status <http://metadataregistry.org/uri/RegStatus/1001> ;
    rdfs:comment "This class comprises activities that result in instances of F2 Expression coming into existence. This class characterises the externalisation of an Individual Work. Although F2 Expression is an abstract entity, a conceptual object, the creation of an expression inevitably also affects the physical world: when you scribble the first draft of a poem on a sheet of paper, you produce an F4 Manifestation Singleton; F28 Expression Creation is a subclass of E12 Production because the recording of the expression causes a physical modification of the carrying E18 Physical Thing. The work becomes manifest by being expressed on a physical carrier different from the creator's brain. The spatio-temporal circumstances under which the expression is created are necessarily the same spatio-temporal circumstances under which the first F4 Manifestation Singleton is produced. The mechanisms through which oral tradition (of myths, tales, music, etc.) operates are not further investigated in this model. As far as bibliographic practice is concerned, only those instances of F2 Expression that are externalised on physical carriers other than both the creator's brain and the auditor's brain are taken into account (for a discussion of the modelling of oral traditions, see: Nicolas, Yann. \"Folklore Requirements for Bibliographic Records: oral traditions and FRBR.\" In: Cataloging & Classification Quarterly (2005). Vol. 39, No. 3-4. P. 179-195)."@en ;
    rdfs:isDefinedBy <http://iflastandards.info/ns/fr/frbr/frbroo/> ;
    rdfs:subClassOf <http://www.cidoc-crm.org/cidoc-crm/E12_Production> ;
    = <http://iflastandards.info/ns/fr/frbr/frbroo/F28_Expression_Creation> ;
    skos:definition "This class comprises activities that result in instances of F2 Expression coming into existence."@en ;
    skos:scopeNote "This class characterises the externalisation of an Individual Work. Although F2 Expression is an abstract entity, a conceptual object, the creation of an expression inevitably also affects the physical world: when you scribble the first draft of a poem on a sheet of paper, you produce an F4 Manifestation Singleton; F28 Expression Creation is a subclass of E12 Production because the recording of the expression causes a physical modification of the carrying E18 Physical Thing. The work becomes manifest by being expressed on a physical carrier different from the creator's brain. The spatio-temporal circumstances under which the expression is created are necessarily the same spatio-temporal circumstances under which the first F4 Manifestation Singleton is produced. The mechanisms through which oral tradition (of myths, tales, music, etc.) operates are not further investigated in this model. As far as bibliographic practice is concerned, only those instances of F2 Expression that are externalised on physical carriers other than both the creator's brain and the auditor's brain are taken into account."@en .

<http://iflastandards.info/ns/fr/frbr/frbroo/F40> a owl:Class ;
    rdfs:label "Identifier Assignment"@en ;
    reg:name "IdentifierAssignment"@en ;
    reg:status <http://metadataregistry.org/uri/RegStatus/1001> ;
    rdfs:comment "This class comprises activities that result in the allocation of an identifier to any E1 CRM Entity. An F40 Identifier Assignment may include the creation of the identifier from multiple constituents. The syntax of the identifier and the kinds of constituents to be used in constructing it may be declared in a rule. The construction of controlled access points for the names of persons, families and corporate bodies following specific cataloguing rules is a typical library application. F40 Identifier Assignment also includes the assignment of uniform titles as controlled access points for works or expressions"@en ;
    rdfs:isDefinedBy <http://iflastandards.info/ns/fr/frbr/frbroo/> ;
    rdfs:subClassOf <http://www.cidoc-crm.org/cidoc-crm/E15_Identifier_Assignment> ;
    = <http://iflastandards.info/ns/fr/frbr/frbroo/F40_Identifier_Assignment> ;
    skos:definition "This class comprises activities that result in the allocation of an identifier to any E1 CRM Entity."@en ;
    skos:scopeNote "An F40 Identifier Assignment may include the creation of the identifier from multiple constituents. The syntax of the identifier and the kinds of constituents to be used in constructing it may be declared in a rule. The construction of controlled access points for the names of persons, families and corporate bodies following specific cataloguing rules is a typical library application. F40 Identifier Assignment also includes the assignment of uniform titles as controlled access points for works or expressions"@en .

<http://iflastandards.info/ns/fr/frbr/frbroo/F41> a owl:Class ;
    rdfs:label "Representative Manifestation Assignment"@en ;
    reg:name "RepresentativeManifestationAssignment"@en ;
    reg:status <http://metadataregistry.org/uri/RegStatus/1001> ;
    rdfs:comment "This class comprises activities through which an Agency declares (implicitly or explicitly) that a given instance of F3 Manifestation Product Type or F4 Manifestation Singleton is representative for a given F2 Expression, i.e., that some features found on that instance of F3 Manifestation Product Type or F4 Manifestation Singleton (most prominently, information about the title) can be inferred to also apply to that instance of F2 Expression, no matter within which manifestation it is embodied. The reasoning behind is that the Work title is known through the title of an Expression that is deemed representative of the Work, and the title of the representative Expression is known through the title proper of a Manifestation that is deemed representative of the Expression representative of the Work."@en ;
    rdfs:isDefinedBy <http://iflastandards.info/ns/fr/frbr/frbroo/> ;
    rdfs:subClassOf <http://www.cidoc-crm.org/cidoc-crm/E13_Attribute_Assignment> ;
    = <http://iflastandards.info/ns/fr/frbr/frbroo/F41_Representative_Manifestation_Assignment> ;
    skos:definition "This class comprises activities through which an Agency declares (implicitly or explicitly) that a given instance of F3 Manifestation Product Type or F4 Manifestation Singleton is representative for a given F2 Expression, i.e., that some features found on that instance of F3 Manifestation Product Type or F4 Manifestation Singleton (most prominently, information about the title) can be inferred to also apply to that instance of F2 Expression, no matter within which manifestation it is embodied."@en ;
    skos:scopeNote "The reasoning behind is that the Work title is known through the title of an Expression that is deemed representative of the Work, and the title of the representative Expression is known through the title proper of a Manifestation that is deemed representative of the Expression representative of the Work."@en .

<http://iflastandards.info/ns/fr/frbr/frbroo/F52> a owl:Class ;
    rdfs:label "Name Use Activity"@en ;
    reg:name "NameUseActivity"@en ;
    reg:status <http://metadataregistry.org/uri/RegStatus/1001> ;
    rdfs:comment "This class comprises periods of continuous use of a specific instance of E41 Appellation for a particular instance of E1 CRM Entity by an E39 Actor. It includes in particular the use of the name by its carrier. Characteristically, actors performing an activity may choose a particular appellation for themselves in the context of this activity. Such cases should be modelled by additionally classifying these activities as instances of F52 Name Use Activity."@en ;
    rdfs:isDefinedBy <http://iflastandards.info/ns/fr/frbr/frbroo/> ;
    rdfs:subClassOf <http://www.cidoc-crm.org/cidoc-crm/E13_Attribute_Assignment> ;
    = <http://iflastandards.info/ns/fr/frbr/frbroo/F52_Name_Use_Activity> ;
    skos:definition "This class comprises periods of continuous use of a specific instance of E41 Appellation for a particular instance of E1 CRM Entity by an E39 Actor."@en ;
    skos:scopeNote "It includes in particular the use of the name by its carrier. Characteristically, actors performing an activity may choose a particular appellation for themselves in the context of this activity. Such cases should be modelled by additionally classifying these activities as instances of F52 Name Use Activity."@en .

<http://iflastandards.info/ns/fr/frbr/frbroo/F22> a owl:Class ;
    rdfs:label "Self Contained Expression"@en ;
    reg:name "SelfContainedExpression"@en ;
    reg:status <http://metadataregistry.org/uri/RegStatus/1001> ;
    rdfs:comment "This class comprises the immaterial realisations of individual works at a particular time that are regarded as a complete whole. The quality of wholeness reflects the intention of its creator that this expression should convey the concept of the work. Such a whole can in turn be part of a larger whole. Inherent to the notion of work is the completion of recognisable outcomes of the work. These outcomes, i.e. the Self-Contained Expressions, are regarded as the symbolic equivalents of Individual Works, which form the atoms of a complex work. A Self-Contained Expression may contain expressions or parts of expressions from other work, such as citations or items collected in anthologies. Even though they are incorporated in the Self-Contained Expression, they are not regarded as becoming members of the expressed container work by their inclusion in the expression, but are rather regarded as foreign or referred elements. F22 Self-Contained Expression can be distinguished from F23 Expression Fragment in that an F23 Expression Fragment was not intended by its creator to make sense by itself. Normally creators would characterise an outcome of a work as finished. In other cases, one could recognise an outcome of a work as complete from the elaboration or logical coherence of its content, or if there is any historical knowledge about the creator deliberately or accidentally never finishing (completing) that particular expression. In all those cases, one would regard an expression as self-contained."@en ;
    rdfs:isDefinedBy <http://iflastandards.info/ns/fr/frbr/frbroo/> ;
    rdfs:subClassOf <http://iflastandards.info/ns/fr/frbr/frbroo/F2> ;
    = <http://iflastandards.info/ns/fr/frbr/frbroo/F22_Self_Contained_Expression> ;
    skos:definition "This class comprises the immaterial realisations of individual works at a particular time that are regarded as a complete whole."@en ;
    skos:scopeNote "The quality of wholeness reflects the intention of its creator that this expression should convey the concept of the work. Such a whole can in turn be part of a larger whole. Inherent to the notion of work is the completion of recognisable outcomes of the work. These outcomes, i.e. the Self-Contained Expressions, are regarded as the symbolic equivalents of Individual Works, which form the atoms of a complex work. A Self-Contained Expression may contain expressions or parts of expressions from other work, such as citations or items collected in anthologies. Even though they are incorporated in the Self-Contained Expression, they are not regarded as becoming members of the expressed container work by their inclusion in the expression, but are rather regarded as foreign or referred elements. F22 Self-Contained Expression can be distinguished from F23 Expression Fragment in that an F23 Expression Fragment was not intended by its creator to make sense by itself. Normally creators would characterise an outcome of a work as finished. In other cases, one could recognise an outcome of a work as complete from the elaboration or logical coherence of its content, or if there is any historical knowledge about the creator deliberately or accidentally never finishing (completing) that particular expression. In all those cases, one would regard an expression as self-contained."@en .

<http://iflastandards.info/ns/fr/frbr/frbroo/F35> a owl:Class ;
    rdfs:label "Nomen Use Statement"@en ;
    reg:name "NomenUseStatement"@en,
        "http://www.cidoc-crm.org/cidoc-crm/E29_Design_or_Procedure"@en ;
    reg:status <http://metadataregistry.org/uri/RegStatus/1001> ;
    rdfs:comment "This class comprises statements relating a Thema with a particular Nomen and its usage in the context of a common Complex Work realized by one or more KOS."@en ;
    rdfs:isDefinedBy <http://iflastandards.info/ns/fr/frbr/frbroo/> ;
    rdfs:subClassOf <http://iflastandards.info/ns/fr/frbr/frbroo/F2> ;
    = <http://iflastandards.info/ns/fr/frbr/frbroo/F35_Nomen_Use_Statement> ;
    skos:definition "This class comprises statements relating a Thema with a particular Nomen and its usage in the context of a common Complex Work realized by one or more KOS."@en .

<http://iflastandards.info/ns/fr/frbr/frbroo/F1> a owl:Class ;
    rdfs:label "Work"@en ;
    reg:name "Work"@en ;
    reg:status <http://metadataregistry.org/uri/RegStatus/1001> ;
    rdfs:comment "This class comprises the sums of concepts which appear in the course of the coherent evolution of an original idea into one or more expressions that are dominated by the original idea. The substance of Work is concepts. A Work may be elaborated by one or more Actors simultaneously or over time. A Work may have members that constitute components of the overall concept or that are alternatives to other members of the work. Members of a work may or may not represent the concept of the Work as a whole; for instance a translation reinterprets the whole, a volume of a trilogy represents a part of the concept. A Work can be either individual or complex. If it is individual its concept is completely realised in a single F22 Self-Contained Expression. If it is complex its concept is embedded in an F15 Complex Work. An F15 Complex Work consists of members that are either F15 Complex Works themselves or F14 Individual Works. The member relationship of Work is based on the members respecting the same concept, and should not be confused with the structural parts of an expression, that might be taken from other work(s). A Work is the product of an intellectual process of one or more persons, yet only indirect evidence about it is at our hands. This can be contextual information such as the existence of an order for a work, reflections of the creators themselves that are documented somewhere, and finally the expressions of the work created. As ideas normally take shape during discussion, elaboration and implementation, it is not reasonable to assume that a work starts with a complete concept. Moreover, it can be very difficult or impossible to define the whole of the concept of a work at some given time. The only objective evidence for such a notion can be based on a stage of expressions at a given time. In this sense, self-contained expressions serve as a kind of \"snap-shots\" of a work. A Work may aggregate expressions of other works into a new expression. For instance, an anthology of poems is regarded as a work in its own right that makes use of expressions of the individual poems that have been selected and ordered as part of an intellectual process. This does not make the contents of the aggregated expressions part of this work, but only parts of the resulting expression."@en ;
    rdfs:isDefinedBy <http://iflastandards.info/ns/fr/frbr/frbroo/> ;
    rdfs:subClassOf <http://www.cidoc-crm.org/cidoc-crm/E89_Propositional_Object> ;
    = <http://iflastandards.info/ns/fr/frbr/frbroo/F1_Work> ;
    skos:definition "This class comprises the sums of concepts which appear in the course of the coherent evolution of an original idea into one or more expressions that are dominated by the original idea."@en ;
    skos:scopeNote "The substance of Work is concepts. A Work may be elaborated by one or more Actors simultaneously or over time. A Work may have members that constitute components of the overall concept or that are alternatives to other members of the work. Members of a work may or may not represent the concept of the Work as a whole; for instance a translation reinterprets the whole, a volume of a trilogy represents a part of the concept. A Work can be either individual or complex. If it is individual its concept is completely realised in a single F22 Self-Contained Expression. If it is complex its concept is embedded in an F15 Complex Work. An F15 Complex Work consists of members that are either F15 Complex Works themselves or F14 Individual Works. The member relationship of Work is based on the members respecting the same concept, and should not be confused with the structural parts of an expression, that might be taken from other work(s). A Work is the product of an intellectual process of one or more persons, yet only indirect evidence about it is at our hands. This can be contextual information such as the existence of an order for a work, reflections of the creators themselves that are documented somewhere, and finally the expressions of the work created. As ideas normally take shape during discussion, elaboration and implementation, it is not reasonable to assume that a work starts with a complete concept. Moreover, it can be very difficult or impossible to define the whole of the concept of a work at some given time. The only objective evidence for such a notion can be based on a stage of expressions at a given time. In this sense, self-contained expressions serve as a kind of \"snap-shots\" of a work. A Work may aggregate expressions of other works into a new expression. For instance, an anthology of poems is regarded as a work in its own right that makes use of expressions of the individual poems that have been selected and ordered as part of an intellectual process. This does not make the contents of the aggregated expressions part of this work, but only parts of the resulting expression."@en .

<http://iflastandards.info/ns/fr/frbr/frbroo/F2> a owl:Class ;
    rdfs:label "Expression"@en ;
    reg:name "Expression"@en ;
    reg:status <http://metadataregistry.org/uri/RegStatus/1001> ;
    rdfs:comment "This class comprises the intellectual or artistic realisations of works in the form of identifiable immaterial objects, such as texts, poems, jokes, musical or choreographic notations, movement pattern, sound pattern, images, multimedia objects, or any combination of such forms that have objectively recognisable structures. The substance of F2 Expression is signs. Expressions cannot exist without a physical carrier, but do not depend on a specific physical carrier and can exist on one or more carriers simultaneously. Carriers may include human memory. Inasmuch as the form of F2 Expression is an inherent characteristic of the F2 Expression, any change in form (e.g., from alpha-numeric notation to spoken word, a poem created in capitals and rendered in lower case) is a new F2 Expression. Similarly, changes in the intellectual conventions or instruments that are employed to express a work (e.g., translation from one language to another) result in the creation of a new F2 Expression. Thus, if a text is revised or modified, the resulting F2 Expression is considered to be a new F2 Expression. Minor changes, such as corrections of spelling and punctuation, etc., are normally considered variations within the same F2 Expression. On a practical level, the degree to which distinctions are made between variant expressions of a work will depend to some extent on the nature of the F1 Work itself, and on the anticipated needs of users. The genre of the work may provide an indication of which features are essential to the expression. In some cases, aspects of physical form, such as typeface and page layout, are not integral to the intellectual or artistic realisation of the work as such, and therefore are not distinctive criteria for the respective expressions. For another work features such as layout may be essential. For instance, the author or a graphic designer may wrap a poem around an image. An expression of a work may include expressions of other works within it. For instance, an anthology of poems is regarded as a work in its own right that makes use of expressions of the individual poems that have been selected and ordered as part of an intellectual process. This does not make the contents of the aggregated expressions part of this work, but only parts of the resulting expression. If an instance of F2 Expression is of a specific form, such as text, image, etc., it may be simultaneously instantiated in the specific classes representing these forms in CIDOC CRM. Thereby one can make use of the more specific properties of these classes, such as language (which is applicable to linguistic objects only)."@en ;
    rdfs:isDefinedBy <http://iflastandards.info/ns/fr/frbr/frbroo/> ;
    rdfs:subClassOf <http://www.cidoc-crm.org/cidoc-crm/E73_Information_Object> ;
    = <http://iflastandards.info/ns/fr/frbr/frbroo/F2_Expression> ;
    skos:definition "This class comprises the intellectual or artistic realisations of works in the form of identifiable immaterial objects, such as texts, poems, jokes, musical or choreographic notations, movement pattern, sound pattern, images, multimedia objects, or any combination of such forms that have objectively recognisable structures."@en ;
    skos:scopeNote "The substance of F2 Expression is signs. Expressions cannot exist without a physical carrier, but do not depend on a specific physical carrier and can exist on one or more carriers simultaneously. Carriers may include human memory. Inasmuch as the form of F2 Expression is an inherent characteristic of the F2 Expression, any change in form (e.g., from alpha-numeric notation to spoken word, a poem created in capitals and rendered in lower case) is a new F2 Expression. Similarly, changes in the intellectual conventions or instruments that are employed to express a work (e.g., translation from one language to another) result in the creation of a new F2 Expression. Thus, if a text is revised or modified, the resulting F2 Expression is considered to be a new F2 Expression. Minor changes, such as corrections of spelling and punctuation, etc., are normally considered variations within the same F2 Expression. On a practical level, the degree to which distinctions are made between variant expressions of a work will depend to some extent on the nature of the F1 Work itself, and on the anticipated needs of users. The genre of the work may provide an indication of which features are essential to the expression. In some cases, aspects of physical form, such as typeface and page layout, are not integral to the intellectual or artistic realisation of the work as such, and therefore are not distinctive criteria for the respective expressions. For another work features such as layout may be essential. For instance, the author or a graphic designer may wrap a poem around an image. An expression of a work may include expressions of other works within it. For instance, an anthology of poems is regarded as a work in its own right that makes use of expressions of the individual poems that have been selected and ordered as part of an intellectual process. This does not make the contents of the aggregated expressions part of this work, but only parts of the resulting expression. If an instance of F2 Expression is of a specific form, such as text, image, etc., it may be simultaneously instantiated in the specific classes representing these forms in CIDOC CRM. Thereby one can make use of the more specific properties of these classes, such as language (which is applicable to linguistic objects only)."@en .

<http://iflastandards.info/ns/fr/frbr/frbroo/F3> a owl:Class ;
    rdfs:label "Manifestation Product Type"@en ;
    reg:name "ManifestationProductType"@en,
        "http://www.cidoc-crm.org/cidoc-crm/E72_Legal_Object"@en ;
    reg:status <http://metadataregistry.org/uri/RegStatus/1001> ;
    rdfs:comment "This class comprises the definitions of publication products. An instance of F3 Manifestation Product Type is the \"species\", and all copies of a given object are \"specimens\" of it. An instance of F3 Manifestation Product Type defines all of the features or traits that instances of F5 Item normally display in order that they may be recognised as copies of a particular publication. However, due to production problems or subsequent events, one or more instances of F5 Item may not exhibit all these features or traits; yet such instances still retain their relationship to the same instance of F3 Manifestation Product Type. The features that characterise a given instance of F3 Manifestation Product Type include: one instance of F24 Publication Expression, containing one or more than one instance of F2 Expression, reflecting the authors’ content of the manifestation and all additional input by the publisher; and the appropriate types of physical features for that form of the object. For example, hardcover and paperback are two distinct publications (i.e. two distinct instances of F3 Manifestation Product Type) even though authorial and editorial content are otherwise identical in both publications. The activity of cataloguing aims at the most accurate listing of features or traits of an instance of F3 Manifestation Product Type that are sufficient to distinguish it from another instance of F3 Manifestation Product Type. In this sense, it may be said that a typical bibliographic record for a publication (not a manuscript) reflects the notion of F3 Manifestation Product Type."@en ;
    rdfs:isDefinedBy <http://iflastandards.info/ns/fr/frbr/frbroo/> ;
    rdfs:subClassOf <http://www.cidoc-crm.org/cidoc-crm/E55_Type> ;
    = <http://iflastandards.info/ns/fr/frbr/frbroo/F3_Manifestation_Product_Type> ;
    skos:definition "This class comprises the definitions of publication products."@en ;
    skos:scopeNote "An instance of F3 Manifestation Product Type is the \"species\", and all copies of a given object are \"specimens\" of it. An instance of F3 Manifestation Product Type defines all of the features or traits that instances of F5 Item normally display in order that they may be recognised as copies of a particular publication. However, due to production problems or subsequent events, one or more instances of F5 Item may not exhibit all these features or traits; yet such instances still retain their relationship to the same instance of F3 Manifestation Product Type. The features that characterise a given instance of F3 Manifestation Product Type include: one instance of F24 Publication Expression, containing one or more than one instance of F2 Expression, reflecting the authors’ content of the manifestation and all additional input by the publisher; and the appropriate types of physical features for that form of the object. For example, hardcover and paperback are two distinct publications (i.e. two distinct instances of F3 Manifestation Product Type) even though authorial and editorial content are otherwise identical in both publications. The activity of cataloguing aims at the most accurate listing of features or traits of an instance of F3 Manifestation Product Type that are sufficient to distinguish it from another instance of F3 Manifestation Product Type. In this sense, it may be said that a typical bibliographic record for a publication (not a manuscript) reflects the notion of F3 Manifestation Product Type."@en .

<http://iflastandards.info/ns/fr/frbr/frbroo/> dc:title "FRBRoo model"@en ;
    skos:note "Element set of the Functional Requirements for Bibliographic Records object-oriented extension to the the CIDOC Conceptual Reference Model (CRM)"@en .

<http://metadataregistry.org/uri/RegStatus/1001> a skos:Concept ;
    skos:prefLabel "Published"@en .

