@prefix dc: <http://purl.org/dc/elements/1.1/> .
@prefix rdf: <http://www.w3.org/1999/02/22-rdf-syntax-ns#> .
@prefix rdfs: <http://www.w3.org/2000/01/rdf-schema#> .
@prefix reg: <http://metadataregistry.org/uri/profile/regap/> .
@prefix skos: <http://www.w3.org/2004/02/skos/core#> .
@prefix xml: <http://www.w3.org/XML/1998/namespace> .
@prefix xsd: <http://www.w3.org/2001/XMLSchema#> .

<http://iflastandards.info/ns/isbd/terms/contentformbase/T1001> a skos:Concept ;
    reg:identifier <http://metadataregistry.org/concepts/8678> ;
    reg:status <http://metadataregistry.org/uri/RegStatus/1001> ;
    skos:broadMatch <http://iflastandards.info/ns/isbd/terms/contentform/T1004> ;
    skos:definition "Content expressed through ordered tones or sounds in succession, in combination, and in temporal relationships to produce a composition, expressed in an audible form, at a given time, and recorded in a resource."@en ;
    skos:inScheme <http://iflastandards.info/ns/isbd/terms/contentformbase> ;
    skos:prefLabel "music (performed)"@en .

<http://iflastandards.info/ns/isbd/terms/contentformbase/T1002> a skos:Concept ;
    reg:identifier <http://metadataregistry.org/concepts/8679> ;
    reg:status <http://metadataregistry.org/uri/RegStatus/1001> ;
    skos:broadMatch <http://iflastandards.info/ns/isbd/terms/contentform/T1002> ;
    skos:definition "Content expressed through line, shape, shading, etc. that is perceived to be in motion, usually by means of a quick succession of images, and in two dimensions."@en ;
    skos:inScheme <http://iflastandards.info/ns/isbd/terms/contentformbase> ;
    skos:prefLabel "image (moving ; 2-dimensional)"@en .

<http://iflastandards.info/ns/isbd/terms/contentformbase/T1003> a skos:Concept ;
    reg:identifier <http://metadataregistry.org/concepts/8680> ;
    reg:status <http://metadataregistry.org/uri/RegStatus/1001> ;
    skos:broadMatch <http://iflastandards.info/ns/isbd/terms/contentform/T1002> ;
    skos:definition "Content expressed through line, shape, shading, etc. that is perceived to be in motion, usually by means of a quick succession of images, and in three dimensions."@en ;
    skos:inScheme <http://iflastandards.info/ns/isbd/terms/contentformbase> ;
    skos:prefLabel "image (moving ; 3-dimensional)"@en .

<http://iflastandards.info/ns/isbd/terms/contentformbase/T1004> a skos:Concept ;
    reg:identifier <http://metadataregistry.org/concepts/8681> ;
    reg:status <http://metadataregistry.org/uri/RegStatus/1001> ;
    skos:broadMatch <http://iflastandards.info/ns/isbd/terms/contentform/T1002> ;
    skos:definition "Content expressed through line, shape, shading, etc. that is perceived to be static and in two dimensions, and intended to be perceived through sight."@en ;
    skos:inScheme <http://iflastandards.info/ns/isbd/terms/contentformbase> ;
    skos:prefLabel "image (still ; 2-dimensional ; visual)"@en .

<http://iflastandards.info/ns/isbd/terms/contentformbase/T1005> a skos:Concept ;
    reg:identifier <http://metadataregistry.org/concepts/8682> ;
    reg:status <http://metadataregistry.org/uri/RegStatus/1001> ;
    skos:broadMatch <http://iflastandards.info/ns/isbd/terms/contentform/T1002> ;
    skos:definition "Content expressed through line, shape, shading, etc. that is perceived to be static and in three dimensions."@en ;
    skos:inScheme <http://iflastandards.info/ns/isbd/terms/contentformbase> ;
    skos:prefLabel "image (still ; 3-dimensional)"@en .

<http://iflastandards.info/ns/isbd/terms/contentformbase/T1006> a skos:Concept ;
    reg:identifier <http://metadataregistry.org/concepts/8683> ;
    reg:status <http://metadataregistry.org/uri/RegStatus/1001> ;
    skos:broadMatch <http://iflastandards.info/ns/isbd/terms/contentform/T1009> ;
    skos:definition "Content expressed through written words, symbols and numbers, and intended to be perceived through sight."@en ;
    skos:inScheme <http://iflastandards.info/ns/isbd/terms/contentformbase> ;
    skos:prefLabel "text (visual)"@en .

<http://iflastandards.info/ns/isbd/terms/contentformbase/T1007> a skos:Concept ;
    reg:identifier <http://metadataregistry.org/concepts/8684> ;
    reg:status <http://metadataregistry.org/uri/RegStatus/1001> ;
    skos:broadMatch <http://iflastandards.info/ns/isbd/terms/contentform/T1004> ;
    skos:definition "Content expressed through ordered tones or sounds in succession, in combination, and in temporal relationships to produce a composition, and through a notational system for artistic purposes intended to be perceived visually."@en ;
    skos:inScheme <http://iflastandards.info/ns/isbd/terms/contentformbase> ;
    skos:prefLabel "music (notated)"@en .

<http://iflastandards.info/ns/isbd/terms/contentformbase/T1008> a skos:Concept ;
    reg:identifier <http://metadataregistry.org/concepts/8685> ;
    reg:status <http://metadataregistry.org/uri/RegStatus/1001> ;
    skos:broadMatch <http://iflastandards.info/ns/isbd/terms/contentform/T1003> ;
    skos:definition "Content expressed through motion, i.e. the act or process of changing the position of an object or person, and through a notational system for artistic purposes intended to be perceived visually."@en ;
    skos:inScheme <http://iflastandards.info/ns/isbd/terms/contentformbase> ;
    skos:prefLabel "movement (notated)"@en .

<http://iflastandards.info/ns/isbd/terms/contentformbase/T1009> a skos:Concept ;
    reg:identifier <http://metadataregistry.org/concepts/8686> ;
    reg:status <http://metadataregistry.org/uri/RegStatus/1001> ;
    skos:broadMatch <http://iflastandards.info/ns/isbd/terms/contentform/T1002> ;
    skos:definition "Content expressed through line, shape, shading, etc. that is perceived to be static and in two dimensions, and intended to be perceived through touch."@en ;
    skos:inScheme <http://iflastandards.info/ns/isbd/terms/contentformbase> ;
    skos:prefLabel "image (still ; 2-dimensional ; tactile)"@en .

<http://iflastandards.info/ns/isbd/terms/contentformbase/T1010> a skos:Concept ;
    reg:identifier <http://metadataregistry.org/concepts/8687> ;
    reg:status <http://metadataregistry.org/uri/RegStatus/1001> ;
    skos:broadMatch <http://iflastandards.info/ns/isbd/terms/contentform/T1005> ;
    skos:definition "Content expressed through three-dimensional material, either naturally occurring entities, or human-made/machine-manufactured artefacts, and intended to be perceived through touch."@en ;
    skos:inScheme <http://iflastandards.info/ns/isbd/terms/contentformbase> ;
    skos:prefLabel "object (tactile)"@en .

<http://iflastandards.info/ns/isbd/terms/contentformbase/T1011> a skos:Concept ;
    reg:identifier <http://metadataregistry.org/concepts/8688> ;
    reg:status <http://metadataregistry.org/uri/RegStatus/1001> ;
    skos:broadMatch <http://iflastandards.info/ns/isbd/terms/contentform/T1009> ;
    skos:definition "Content expressed through written words, symbols and numbers, and intended to be perceived through touch."@en ;
    skos:inScheme <http://iflastandards.info/ns/isbd/terms/contentformbase> ;
    skos:prefLabel "text (tactile)"@en .

<http://iflastandards.info/ns/isbd/terms/contentformbase/T1012> a skos:Concept ;
    reg:identifier <http://metadataregistry.org/concepts/8689> ;
    reg:status <http://metadataregistry.org/uri/RegStatus/1001> ;
    skos:broadMatch <http://iflastandards.info/ns/isbd/terms/contentform/T1004> ;
    skos:definition "Content expressed through ordered tones or sounds in succession, in combination, and in temporal relationships to produce a composition, and through a notational system for artistic purposes intended to be perceived through touch."@en ;
    skos:inScheme <http://iflastandards.info/ns/isbd/terms/contentformbase> ;
    skos:prefLabel "music (notated ; tactile)"@en .

<http://iflastandards.info/ns/isbd/terms/contentformbase/T1013> a skos:Concept ;
    reg:identifier <http://metadataregistry.org/concepts/8690> ;
    reg:status <http://metadataregistry.org/uri/RegStatus/1001> ;
    skos:broadMatch <http://iflastandards.info/ns/isbd/terms/contentform/T1003> ;
    skos:definition "Content expressed through motion, i.e. the act or process of changing the position of an object or person, and through a notational system for artistic purposes intended to be perceived through touch."@en ;
    skos:inScheme <http://iflastandards.info/ns/isbd/terms/contentformbase> ;
    skos:prefLabel "movement (notated ; tactile)"@en .

<http://iflastandards.info/ns/isbd/terms/contentformbase> a skos:ConceptScheme ;
    dc:title "ISBD Content Form Qualified Base" .

<http://metadataregistry.org/uri/RegStatus/1001> a skos:Concept ;
    skos:prefLabel "Published"@en .

